@prefix core:        <https://www.opengis.net/ont/citygml/core/> .
@prefix gen:         <https://www.opengis.net/ont/citygml/generics/> .
@prefix iso19136-bt: <http://def.isotc211.org/iso19136/2007/BasicTypes#> .
@prefix iso19150-2:  <http://def.isotc211.org/iso19150/-2/2012/base#> .
@prefix owl:         <http://www.w3.org/2002/07/owl#> .
@prefix rdf:         <http://www.w3.org/1999/02/22-rdf-syntax-ns#> .
@prefix rdfs:        <http://www.w3.org/2000/01/rdf-schema#> .
@prefix sc:          <http://shapechange.net/resources/ont/base#> .
@prefix skos:        <http://www.w3.org/2004/02/skos/core#> .
@prefix xsd:         <http://www.w3.org/2001/XMLSchema#> .

gen:ADEOfGenericOccupiedSpace
        rdf:type               owl:Class;
        rdfs:label             "ADEOfGenericOccupiedSpace"@en;
        iso19150-2:isAbstract  true;
        skos:definition        "ADEOfGenericOccupiedSpace acts as a hook to define properties within an ADE that are to be added to a GenericOccupiedSpace."@en .

<https://www.opengis.net/ont/citygml/generics>
        rdf:type         owl:Ontology;
        rdfs:label       "Generics"@en;
        owl:imports      <http://shapechange.net/resources/ont/base> , <https://www.opengis.net/ont/citygml/core> , <http://def.isotc211.org/iso19150/-2/2012/base>;
        skos:definition  "The Generics module supports application-specific extensions to the CityGML conceptual model. These extensions may be used to model and exchange additional attributes and features not covered by the predefined thematic classes of CityGML. Generic extensions shall only be used if appropriate thematic classes or attributes are not provided by any other CityGML module."@en .

gen:GenericThematicSurfaceClassValue
        rdf:type         owl:Class;
        rdfs:label       "GenericThematicSurfaceClassValue"@en;
        rdfs:subClassOf  skos:Concept;
        skos:definition  "GenericThematicSurfaceClassValue is a code list used to further classify a GenericThematicSurface."@en .

gen:ADEOfGenericUnoccupiedSpace
        rdf:type               owl:Class;
        rdfs:label             "ADEOfGenericUnoccupiedSpace"@en;
        iso19150-2:isAbstract  true;
        skos:definition        "ADEOfGenericUnoccupiedSpace acts as a hook to define properties within an ADE that are to be added to a GenericUnoccupiedSpace."@en .

gen:adeOfGenericOccupiedSpace
        rdf:type         owl:ObjectProperty;
        rdfs:label       "adeOfGenericOccupiedSpace"@en;
        rdfs:range       gen:ADEOfGenericOccupiedSpace;
        skos:definition  "Augments the GenericOccupiedSpace with properties defined in an ADE."@en .

gen:GenericOccupiedSpace
        rdf:type         owl:Class;
        rdfs:label       "GenericOccupiedSpace"@en;
        rdfs:subClassOf  core:AbstractOccupiedSpace;
        rdfs:subClassOf  [ rdf:type           owl:Restriction;
                           owl:allValuesFrom  gen:ADEOfGenericOccupiedSpace;
                           owl:onProperty     gen:adeOfGenericOccupiedSpace
                         ];
        rdfs:subClassOf  [ rdf:type           owl:Restriction;
                           owl:allValuesFrom  gen:GenericOccupiedSpaceUsageValue;
                           owl:onProperty     gen:GenericOccupiedSpace.usage
                         ];
        rdfs:subClassOf  [ rdf:type           owl:Restriction;
                           owl:allValuesFrom  gen:GenericOccupiedSpaceFunctionValue;
                           owl:onProperty     gen:GenericOccupiedSpace.function
                         ];
        rdfs:subClassOf  [ rdf:type           owl:Restriction;
                           owl:allValuesFrom  gen:GenericOccupiedSpaceClassValue;
                           owl:onProperty     gen:GenericOccupiedSpace.class
                         ];
        rdfs:subClassOf  [ rdf:type                     owl:Restriction;
                           owl:maxQualifiedCardinality  "1"^^xsd:nonNegativeInteger;
                           owl:onClass                  gen:GenericOccupiedSpaceClassValue;
                           owl:onProperty               gen:GenericOccupiedSpace.class
                         ];
        skos:definition  "A GenericOccupiedSpace is a space that is not represented by any explicitly modelled AbstractOccupiedSpace subclass within CityGML."@en .

gen:StringAttribute  rdf:type  owl:Class;
        rdfs:label       "StringAttribute"@en;
        rdfs:subClassOf  core:AbstractGenericAttribute;
        rdfs:subClassOf  [ rdf:type           owl:Restriction;
                           owl:allValuesFrom  xsd:string;
                           owl:onProperty     gen:StringAttribute.value
                         ];
        rdfs:subClassOf  [ rdf:type                  owl:Restriction;
                           owl:onClass               xsd:string;
                           owl:onProperty            gen:StringAttribute.value;
                           owl:qualifiedCardinality  "1"^^xsd:nonNegativeInteger
                         ];
        rdfs:subClassOf  [ rdf:type           owl:Restriction;
                           owl:allValuesFrom  xsd:string;
                           owl:onProperty     gen:StringAttribute.name
                         ];
        rdfs:subClassOf  [ rdf:type                  owl:Restriction;
                           owl:onClass               xsd:string;
                           owl:onProperty            gen:StringAttribute.name;
                           owl:qualifiedCardinality  "1"^^xsd:nonNegativeInteger
                         ];
        skos:definition  "StringAttribute is a data type used to define generic attributes of type \"String\"."@en .

gen:GenericOccupiedSpaceFunctionValue
        rdf:type         owl:Class;
        rdfs:label       "GenericOccupiedSpaceFunctionValue"@en;
        rdfs:subClassOf  skos:Concept;
        skos:definition  "GenericOccupiedSpaceFunctionValue is a code list that enumerates the different purposes of a GenericOccupiedSpace."@en .

gen:UriAttribute.name
        rdf:type         owl:DatatypeProperty;
        rdfs:domain      gen:UriAttribute;
        rdfs:label       "name"@en;
        rdfs:range       xsd:string;
        skos:definition  "Specifies the name of the UriAttribute."@en .

gen:MeasureAttribute.value
        rdf:type         owl:DatatypeProperty;
        rdfs:domain      gen:MeasureAttribute;
        rdfs:label       "value"@en;
        rdfs:range       sc:Measure;
        skos:definition  "Specifies the value of the MeasureAttribute. The value is of type \"Measure\", which can additionally provide the units of measure. [cf. ISO 19103]"@en .

gen:IntAttribute.name
        rdf:type         owl:DatatypeProperty;
        rdfs:domain      gen:IntAttribute;
        rdfs:label       "name"@en;
        rdfs:range       xsd:string;
        skos:definition  "Specifies the name of the IntAttribute."@en .

gen:GenericUnoccupiedSpaceClassValue
        rdf:type         owl:Class;
        rdfs:label       "GenericUnoccupiedSpaceClassValue"@en;
        rdfs:subClassOf  skos:Concept;
        skos:definition  "GenericUnoccupiedSpaceClassValue is a code list used to further classify a GenericUnoccupiedSpace."@en .

gen:GenericThematicSurface.function
        rdf:type         owl:ObjectProperty;
        rdfs:domain      gen:GenericThematicSurface;
        rdfs:label       "function"@en;
        rdfs:range       gen:GenericThematicSurfaceFunctionValue;
        skos:definition  "Specifies the intended purposes of the GenericThematicSurface."@en .

gen:GenericThematicSurfaceFunctionValue
        rdf:type         owl:Class;
        rdfs:label       "GenericThematicSurfaceFunctionValue"@en;
        rdfs:subClassOf  skos:Concept;
        skos:definition  "GenericThematicSurfaceFunctionValue is a code list that enumerates the different purposes of a GenericThematicSurface."@en .

gen:DateAttribute.value
        rdf:type         owl:DatatypeProperty;
        rdfs:domain      gen:DateAttribute;
        rdfs:label       "value"@en;
        rdfs:range       xsd:date;
        skos:definition  "Specifies the \"Date\" value."@en .

gen:ADEOfGenericLogicalSpace
        rdf:type               owl:Class;
        rdfs:label             "ADEOfGenericLogicalSpace"@en;
        iso19150-2:isAbstract  true;
        skos:definition        "ADEOfGenericLogicalSpace acts as a hook to define properties within an ADE that are to be added to a GenericLogicalSpace."@en .

gen:GenericThematicSurface.class
        rdf:type         owl:ObjectProperty;
        rdfs:domain      gen:GenericThematicSurface;
        rdfs:label       "class"@en;
        rdfs:range       gen:GenericThematicSurfaceClassValue;
        skos:definition  "Indicates the specific type of the GenericThematicSurface."@en .

gen:GenericOccupiedSpace.class
        rdf:type         owl:ObjectProperty;
        rdfs:domain      gen:GenericOccupiedSpace;
        rdfs:label       "class"@en;
        rdfs:range       gen:GenericOccupiedSpaceClassValue;
        skos:definition  "Indicates the specific type of the GenericOccupiedSpace."@en .

gen:MeasureAttribute.name
        rdf:type         owl:DatatypeProperty;
        rdfs:domain      gen:MeasureAttribute;
        rdfs:label       "name"@en;
        rdfs:range       xsd:string;
        skos:definition  "Specifies the name of the MeasureAttribute."@en .

gen:GenericThematicSurface
        rdf:type         owl:Class;
        rdfs:label       "GenericThematicSurface"@en;
        rdfs:subClassOf  core:AbstractThematicSurface;
        rdfs:subClassOf  [ rdf:type           owl:Restriction;
                           owl:allValuesFrom  gen:ADEOfGenericThematicSurface;
                           owl:onProperty     gen:adeOfGenericThematicSurface
                         ];
        rdfs:subClassOf  [ rdf:type           owl:Restriction;
                           owl:allValuesFrom  gen:GenericThematicSurfaceUsageValue;
                           owl:onProperty     gen:GenericThematicSurface.usage
                         ];
        rdfs:subClassOf  [ rdf:type           owl:Restriction;
                           owl:allValuesFrom  gen:GenericThematicSurfaceFunctionValue;
                           owl:onProperty     gen:GenericThematicSurface.function
                         ];
        rdfs:subClassOf  [ rdf:type           owl:Restriction;
                           owl:allValuesFrom  gen:GenericThematicSurfaceClassValue;
                           owl:onProperty     gen:GenericThematicSurface.class
                         ];
        rdfs:subClassOf  [ rdf:type                     owl:Restriction;
                           owl:maxQualifiedCardinality  "1"^^xsd:nonNegativeInteger;
                           owl:onClass                  gen:GenericThematicSurfaceClassValue;
                           owl:onProperty               gen:GenericThematicSurface.class
                         ];
        skos:definition  "A GenericThematicSurface is a surface that is not represented by any explicitly modelled AbstractThematicSurface subclass within CityGML."@en .

gen:adeOfGenericUnoccupiedSpace
        rdf:type         owl:ObjectProperty;
        rdfs:label       "adeOfGenericUnoccupiedSpace"@en;
        rdfs:range       gen:ADEOfGenericUnoccupiedSpace;
        skos:definition  "Augments the GenericUnoccupiedSpace with properties defined in an ADE."@en .

gen:StringAttribute.name
        rdf:type         owl:DatatypeProperty;
        rdfs:domain      gen:StringAttribute;
        rdfs:label       "name"@en;
        rdfs:range       xsd:string;
        skos:definition  "Specifies the name of the StringAttribute."@en .

gen:genericAttribute  rdf:type  owl:ObjectProperty;
        rdfs:label       "genericAttribute"@en;
        rdfs:range       core:AbstractGenericAttribute;
        skos:definition  "Relates to the generic attributes that are part of the GenericAttributeSet."@en .

gen:IntAttribute  rdf:type  owl:Class;
        rdfs:label       "IntAttribute"@en;
        rdfs:subClassOf  core:AbstractGenericAttribute;
        rdfs:subClassOf  [ rdf:type           owl:Restriction;
                           owl:allValuesFrom  xsd:integer;
                           owl:onProperty     gen:IntAttribute.value
                         ];
        rdfs:subClassOf  [ rdf:type                  owl:Restriction;
                           owl:onClass               xsd:integer;
                           owl:onProperty            gen:IntAttribute.value;
                           owl:qualifiedCardinality  "1"^^xsd:nonNegativeInteger
                         ];
        rdfs:subClassOf  [ rdf:type           owl:Restriction;
                           owl:allValuesFrom  xsd:string;
                           owl:onProperty     gen:IntAttribute.name
                         ];
        rdfs:subClassOf  [ rdf:type                  owl:Restriction;
                           owl:onClass               xsd:string;
                           owl:onProperty            gen:IntAttribute.name;
                           owl:qualifiedCardinality  "1"^^xsd:nonNegativeInteger
                         ];
        skos:definition  "IntAttribute is a data type used to define generic attributes of type \"Integer\"."@en .

gen:DoubleAttribute.name
        rdf:type         owl:DatatypeProperty;
        rdfs:domain      gen:DoubleAttribute;
        rdfs:label       "name"@en;
        rdfs:range       xsd:string;
        skos:definition  "Specifies the name of the DoubleAttribute."@en .

gen:GenericLogicalSpace.usage
        rdf:type         owl:ObjectProperty;
        rdfs:domain      gen:GenericLogicalSpace;
        rdfs:label       "usage"@en;
        rdfs:range       gen:GenericLogicalSpaceUsageValue;
        skos:definition  "Specifies the actual uses of the GenericLogicalSpace."@en .

gen:adeOfGenericLogicalSpace
        rdf:type         owl:ObjectProperty;
        rdfs:label       "adeOfGenericLogicalSpace"@en;
        rdfs:range       gen:ADEOfGenericLogicalSpace;
        skos:definition  "Augments the GenericLogicalSpace with properties defined in an ADE."@en .

gen:GenericLogicalSpace.function
        rdf:type         owl:ObjectProperty;
        rdfs:domain      gen:GenericLogicalSpace;
        rdfs:label       "function"@en;
        rdfs:range       gen:GenericLogicalSpaceFunctionValue;
        skos:definition  "Specifies the intended purposes of the GenericLogicalSpace."@en .

gen:GenericLogicalSpaceFunctionValue
        rdf:type         owl:Class;
        rdfs:label       "GenericLogicalSpaceFunctionValue"@en;
        rdfs:subClassOf  skos:Concept;
        skos:definition  "GenericLogicalSpaceFunctionValue is a code list that enumerates the different purposes of a GenericLogicalSpace."@en .

gen:codeSpace  rdf:type  owl:DatatypeProperty;
        rdfs:label       "codeSpace"@en;
        rdfs:range       xsd:anyURI;
        skos:definition  "Associates the GenericAttributeSet with an authority that maintains the collection of generic attributes."@en .

gen:ADEOfGenericThematicSurface
        rdf:type               owl:Class;
        rdfs:label             "ADEOfGenericThematicSurface"@en;
        iso19150-2:isAbstract  true;
        skos:definition        "ADEOfGenericThematicSurface acts as a hook to define properties within an ADE that are to be added to a GenericThematicSurface."@en .

gen:adeOfGenericThematicSurface
        rdf:type         owl:ObjectProperty;
        rdfs:label       "adeOfGenericThematicSurface"@en;
        rdfs:range       gen:ADEOfGenericThematicSurface;
        skos:definition  "Augments the GenericThematicSurface with properties defined in an ADE."@en .

gen:DateAttribute.name
        rdf:type         owl:DatatypeProperty;
        rdfs:domain      gen:DateAttribute;
        rdfs:label       "name"@en;
        rdfs:range       xsd:string;
        skos:definition  "Specifies the name of the DateAttribute."@en .

gen:GenericUnoccupiedSpaceFunctionValue
        rdf:type         owl:Class;
        rdfs:label       "GenericUnoccupiedSpaceFunctionValue"@en;
        rdfs:subClassOf  skos:Concept;
        skos:definition  "GenericUnoccupiedSpaceFunctionValue is a code list that enumerates the different purposes of a GenericUnoccupiedSpace."@en .

gen:IntAttribute.value
        rdf:type         owl:DatatypeProperty;
        rdfs:domain      gen:IntAttribute;
        rdfs:label       "value"@en;
        rdfs:range       xsd:integer;
        skos:definition  "Specifies the \"Integer\" value."@en .

gen:MeasureAttribute  rdf:type  owl:Class;
        rdfs:label       "MeasureAttribute"@en;
        rdfs:subClassOf  core:AbstractGenericAttribute;
        rdfs:subClassOf  [ rdf:type           owl:Restriction;
                           owl:allValuesFrom  sc:Measure;
                           owl:onProperty     gen:MeasureAttribute.value
                         ];
        rdfs:subClassOf  [ rdf:type                  owl:Restriction;
                           owl:onClass               sc:Measure;
                           owl:onProperty            gen:MeasureAttribute.value;
                           owl:qualifiedCardinality  "1"^^xsd:nonNegativeInteger
                         ];
        rdfs:subClassOf  [ rdf:type           owl:Restriction;
                           owl:allValuesFrom  xsd:string;
                           owl:onProperty     gen:MeasureAttribute.name
                         ];
        rdfs:subClassOf  [ rdf:type                  owl:Restriction;
                           owl:onClass               xsd:string;
                           owl:onProperty            gen:MeasureAttribute.name;
                           owl:qualifiedCardinality  "1"^^xsd:nonNegativeInteger
                         ];
        skos:definition  "MeasureAttribute is a data type used to define generic attributes of type \"Measure\"."@en .

gen:GenericAttributeSet.name
        rdf:type         owl:DatatypeProperty;
        rdfs:domain      gen:GenericAttributeSet;
        rdfs:label       "name"@en;
        rdfs:range       xsd:string;
        skos:definition  "Specifies the name of the GenericAttributeSet."@en .

gen:GenericUnoccupiedSpace.usage
        rdf:type         owl:ObjectProperty;
        rdfs:domain      gen:GenericUnoccupiedSpace;
        rdfs:label       "usage"@en;
        rdfs:range       gen:GenericUnoccupiedSpaceUsageValue;
        skos:definition  "Specifies the actual uses of the GenericUnoccupiedSpace."@en .

gen:GenericLogicalSpaceUsageValue
        rdf:type         owl:Class;
        rdfs:label       "GenericLogicalSpaceUsageValue"@en;
        rdfs:subClassOf  skos:Concept;
        skos:definition  "GenericLogicalSpaceUsageValue is a code list that enumerates the different uses of a GenericLogicalSpace."@en .

gen:CodeAttribute.value
        rdf:type         owl:ObjectProperty;
        rdfs:domain      gen:CodeAttribute;
        rdfs:label       "value"@en;
        rdfs:range       iso19136-bt:Code;
        skos:definition  "Specifies the \"Code\" value."@en .

gen:GenericUnoccupiedSpace.function
        rdf:type         owl:ObjectProperty;
        rdfs:domain      gen:GenericUnoccupiedSpace;
        rdfs:label       "function"@en;
        rdfs:range       gen:GenericUnoccupiedSpaceFunctionValue;
        skos:definition  "Specifies the intended purposes of the GenericUnoccupiedSpace."@en .

gen:GenericOccupiedSpaceUsageValue
        rdf:type         owl:Class;
        rdfs:label       "GenericOccupiedSpaceUsageValue"@en;
        rdfs:subClassOf  skos:Concept;
        skos:definition  "GenericOccupiedSpaceUsageValue is a code list that enumerates the different uses of a GenericOccupiedSpace."@en .

gen:GenericLogicalSpace.class
        rdf:type         owl:ObjectProperty;
        rdfs:domain      gen:GenericLogicalSpace;
        rdfs:label       "class"@en;
        rdfs:range       gen:GenericLogicalSpaceClassValue;
        skos:definition  "Indicates the specific type of the GenericLogicalSpace."@en .

gen:DoubleAttribute.value
        rdf:type         owl:DatatypeProperty;
        rdfs:domain      gen:DoubleAttribute;
        rdfs:label       "value"@en;
        rdfs:range       xsd:double;
        skos:definition  "Specifies the \"Double\" value."@en .

gen:DoubleAttribute  rdf:type  owl:Class;
        rdfs:label       "DoubleAttribute"@en;
        rdfs:subClassOf  core:AbstractGenericAttribute;
        rdfs:subClassOf  [ rdf:type           owl:Restriction;
                           owl:allValuesFrom  xsd:double;
                           owl:onProperty     gen:DoubleAttribute.value
                         ];
        rdfs:subClassOf  [ rdf:type                  owl:Restriction;
                           owl:onClass               xsd:double;
                           owl:onProperty            gen:DoubleAttribute.value;
                           owl:qualifiedCardinality  "1"^^xsd:nonNegativeInteger
                         ];
        rdfs:subClassOf  [ rdf:type           owl:Restriction;
                           owl:allValuesFrom  xsd:string;
                           owl:onProperty     gen:DoubleAttribute.name
                         ];
        rdfs:subClassOf  [ rdf:type                  owl:Restriction;
                           owl:onClass               xsd:string;
                           owl:onProperty            gen:DoubleAttribute.name;
                           owl:qualifiedCardinality  "1"^^xsd:nonNegativeInteger
                         ];
        skos:definition  "DoubleAttribute is a data type used to define generic attributes of type \"Double\"."@en .

gen:GenericThematicSurfaceUsageValue
        rdf:type         owl:Class;
        rdfs:label       "GenericThematicSurfaceUsageValue"@en;
        rdfs:subClassOf  skos:Concept;
        skos:definition  "GenericThematicSurfaceUsageValue is a code list that enumerates the different uses of a GenericThematicSurface."@en .

gen:GenericLogicalSpace
        rdf:type         owl:Class;
        rdfs:label       "GenericLogicalSpace"@en;
        rdfs:subClassOf  core:AbstractLogicalSpace;
        rdfs:subClassOf  [ rdf:type           owl:Restriction;
                           owl:allValuesFrom  gen:ADEOfGenericLogicalSpace;
                           owl:onProperty     gen:adeOfGenericLogicalSpace
                         ];
        rdfs:subClassOf  [ rdf:type           owl:Restriction;
                           owl:allValuesFrom  gen:GenericLogicalSpaceUsageValue;
                           owl:onProperty     gen:GenericLogicalSpace.usage
                         ];
        rdfs:subClassOf  [ rdf:type           owl:Restriction;
                           owl:allValuesFrom  gen:GenericLogicalSpaceFunctionValue;
                           owl:onProperty     gen:GenericLogicalSpace.function
                         ];
        rdfs:subClassOf  [ rdf:type           owl:Restriction;
                           owl:allValuesFrom  gen:GenericLogicalSpaceClassValue;
                           owl:onProperty     gen:GenericLogicalSpace.class
                         ];
        rdfs:subClassOf  [ rdf:type                     owl:Restriction;
                           owl:maxQualifiedCardinality  "1"^^xsd:nonNegativeInteger;
                           owl:onClass                  gen:GenericLogicalSpaceClassValue;
                           owl:onProperty               gen:GenericLogicalSpace.class
                         ];
        skos:definition  "A GenericLogicalSpace is a space that is not represented by any explicitly modelled AbstractLogicalSpace subclass within CityGML."@en .

gen:UriAttribute.value
        rdf:type         owl:DatatypeProperty;
        rdfs:domain      gen:UriAttribute;
        rdfs:label       "value"@en;
        rdfs:range       xsd:anyURI;
        skos:definition  "Specifies the \"URI\" value."@en .

gen:UriAttribute  rdf:type  owl:Class;
        rdfs:label       "UriAttribute"@en;
        rdfs:subClassOf  core:AbstractGenericAttribute;
        rdfs:subClassOf  [ rdf:type           owl:Restriction;
                           owl:allValuesFrom  xsd:anyURI;
                           owl:onProperty     gen:UriAttribute.value
                         ];
        rdfs:subClassOf  [ rdf:type                  owl:Restriction;
                           owl:onClass               xsd:anyURI;
                           owl:onProperty            gen:UriAttribute.value;
                           owl:qualifiedCardinality  "1"^^xsd:nonNegativeInteger
                         ];
        rdfs:subClassOf  [ rdf:type           owl:Restriction;
                           owl:allValuesFrom  xsd:string;
                           owl:onProperty     gen:UriAttribute.name
                         ];
        rdfs:subClassOf  [ rdf:type                  owl:Restriction;
                           owl:onClass               xsd:string;
                           owl:onProperty            gen:UriAttribute.name;
                           owl:qualifiedCardinality  "1"^^xsd:nonNegativeInteger
                         ];
        skos:definition  "UriAttribute is a data type used to define generic attributes of type \"URI\"."@en .

gen:GenericUnoccupiedSpace
        rdf:type         owl:Class;
        rdfs:label       "GenericUnoccupiedSpace"@en;
        rdfs:subClassOf  core:AbstractUnoccupiedSpace;
        rdfs:subClassOf  [ rdf:type           owl:Restriction;
                           owl:allValuesFrom  gen:ADEOfGenericUnoccupiedSpace;
                           owl:onProperty     gen:adeOfGenericUnoccupiedSpace
                         ];
        rdfs:subClassOf  [ rdf:type           owl:Restriction;
                           owl:allValuesFrom  gen:GenericUnoccupiedSpaceUsageValue;
                           owl:onProperty     gen:GenericUnoccupiedSpace.usage
                         ];
        rdfs:subClassOf  [ rdf:type           owl:Restriction;
                           owl:allValuesFrom  gen:GenericUnoccupiedSpaceFunctionValue;
                           owl:onProperty     gen:GenericUnoccupiedSpace.function
                         ];
        rdfs:subClassOf  [ rdf:type           owl:Restriction;
                           owl:allValuesFrom  gen:GenericUnoccupiedSpaceClassValue;
                           owl:onProperty     gen:GenericUnoccupiedSpace.class
                         ];
        rdfs:subClassOf  [ rdf:type                     owl:Restriction;
                           owl:maxQualifiedCardinality  "1"^^xsd:nonNegativeInteger;
                           owl:onClass                  gen:GenericUnoccupiedSpaceClassValue;
                           owl:onProperty               gen:GenericUnoccupiedSpace.class
                         ];
        skos:definition  "A GenericUnoccupiedSpace is a space that is not represented by any explicitly modelled AbstractUnoccupiedSpace subclass within CityGML."@en .

gen:GenericAttributeSet
        rdf:type         owl:Class;
        rdfs:label       "GenericAttributeSet"@en;
        rdfs:subClassOf  core:AbstractGenericAttribute;
        rdfs:subClassOf  [ rdf:type           owl:Restriction;
                           owl:allValuesFrom  xsd:string;
                           owl:onProperty     gen:GenericAttributeSet.name
                         ];
        rdfs:subClassOf  [ rdf:type                     owl:Restriction;
                           owl:minQualifiedCardinality  "1"^^xsd:nonNegativeInteger;
                           owl:onClass                  core:AbstractGenericAttribute;
                           owl:onProperty               gen:genericAttribute
                         ];
        rdfs:subClassOf  [ rdf:type                     owl:Restriction;
                           owl:maxQualifiedCardinality  "1"^^xsd:nonNegativeInteger;
                           owl:onClass                  xsd:anyURI;
                           owl:onProperty               gen:codeSpace
                         ];
        rdfs:subClassOf  [ rdf:type                  owl:Restriction;
                           owl:onClass               xsd:string;
                           owl:onProperty            gen:GenericAttributeSet.name;
                           owl:qualifiedCardinality  "1"^^xsd:nonNegativeInteger
                         ];
        rdfs:subClassOf  [ rdf:type           owl:Restriction;
                           owl:allValuesFrom  core:AbstractGenericAttribute;
                           owl:onProperty     gen:genericAttribute
                         ];
        rdfs:subClassOf  [ rdf:type           owl:Restriction;
                           owl:allValuesFrom  xsd:anyURI;
                           owl:onProperty     gen:codeSpace
                         ];
        skos:definition  "A GenericAttributeSet is a named collection of generic attributes."@en .

gen:GenericLogicalSpaceClassValue
        rdf:type         owl:Class;
        rdfs:label       "GenericLogicalSpaceClassValue"@en;
        rdfs:subClassOf  skos:Concept;
        skos:definition  "GenericLogicalSpaceClassValue is a code list used to further classify a GenericLogicalSpace."@en .

gen:GenericOccupiedSpaceClassValue
        rdf:type         owl:Class;
        rdfs:label       "GenericOccupiedSpaceClassValue"@en;
        rdfs:subClassOf  skos:Concept;
        skos:definition  "GenericOccupiedSpaceClassValue is a code list used to further classify a GenericOccupiedSpace."@en .

gen:StringAttribute.value
        rdf:type         owl:DatatypeProperty;
        rdfs:domain      gen:StringAttribute;
        rdfs:label       "value"@en;
        rdfs:range       xsd:string;
        skos:definition  "Specifies the \"String\" value."@en .

gen:GenericThematicSurface.usage
        rdf:type         owl:ObjectProperty;
        rdfs:domain      gen:GenericThematicSurface;
        rdfs:label       "usage"@en;
        rdfs:range       gen:GenericThematicSurfaceUsageValue;
        skos:definition  "Specifies the actual uses of the GenericThematicSurface."@en .

gen:GenericUnoccupiedSpaceUsageValue
        rdf:type         owl:Class;
        rdfs:label       "GenericUnoccupiedSpaceUsageValue"@en;
        rdfs:subClassOf  skos:Concept;
        skos:definition  "GenericUnoccupiedSpaceUsageValue is a code list that enumerates the different uses of a GenericUnoccupiedSpace."@en .

gen:GenericOccupiedSpace.usage
        rdf:type         owl:ObjectProperty;
        rdfs:domain      gen:GenericOccupiedSpace;
        rdfs:label       "usage"@en;
        rdfs:range       gen:GenericOccupiedSpaceUsageValue;
        skos:definition  "Specifies the actual uses of the GenericOccupiedSpace."@en .

gen:CodeAttribute.name
        rdf:type         owl:DatatypeProperty;
        rdfs:domain      gen:CodeAttribute;
        rdfs:label       "name"@en;
        rdfs:range       xsd:string;
        skos:definition  "Specifies the name of the CodeAttribute."@en .

gen:GenericOccupiedSpace.function
        rdf:type         owl:ObjectProperty;
        rdfs:domain      gen:GenericOccupiedSpace;
        rdfs:label       "function"@en;
        rdfs:range       gen:GenericOccupiedSpaceFunctionValue;
        skos:definition  "Specifies the intended purposes of the GenericOccupiedSpace."@en .

gen:GenericUnoccupiedSpace.class
        rdf:type         owl:ObjectProperty;
        rdfs:domain      gen:GenericUnoccupiedSpace;
        rdfs:label       "class"@en;
        rdfs:range       gen:GenericUnoccupiedSpaceClassValue;
        skos:definition  "Indicates the specific type of the GenericUnoccupiedSpace."@en .

gen:CodeAttribute  rdf:type  owl:Class;
        rdfs:label       "CodeAttribute"@en;
        rdfs:subClassOf  core:AbstractGenericAttribute;
        rdfs:subClassOf  [ rdf:type           owl:Restriction;
                           owl:allValuesFrom  iso19136-bt:Code;
                           owl:onProperty     gen:CodeAttribute.value
                         ];
        rdfs:subClassOf  [ rdf:type                  owl:Restriction;
                           owl:onClass               iso19136-bt:Code;
                           owl:onProperty            gen:CodeAttribute.value;
                           owl:qualifiedCardinality  "1"^^xsd:nonNegativeInteger
                         ];
        rdfs:subClassOf  [ rdf:type           owl:Restriction;
                           owl:allValuesFrom  xsd:string;
                           owl:onProperty     gen:CodeAttribute.name
                         ];
        rdfs:subClassOf  [ rdf:type                  owl:Restriction;
                           owl:onClass               xsd:string;
                           owl:onProperty            gen:CodeAttribute.name;
                           owl:qualifiedCardinality  "1"^^xsd:nonNegativeInteger
                         ];
        skos:definition  "CodeAttribute is a data type used to define generic attributes of type \"Code\"."@en .

gen:DateAttribute  rdf:type  owl:Class;
        rdfs:label       "DateAttribute"@en;
        rdfs:subClassOf  core:AbstractGenericAttribute;
        rdfs:subClassOf  [ rdf:type           owl:Restriction;
                           owl:allValuesFrom  xsd:date;
                           owl:onProperty     gen:DateAttribute.value
                         ];
        rdfs:subClassOf  [ rdf:type                  owl:Restriction;
                           owl:onClass               xsd:date;
                           owl:onProperty            gen:DateAttribute.value;
                           owl:qualifiedCardinality  "1"^^xsd:nonNegativeInteger
                         ];
        rdfs:subClassOf  [ rdf:type           owl:Restriction;
                           owl:allValuesFrom  xsd:string;
                           owl:onProperty     gen:DateAttribute.name
                         ];
        rdfs:subClassOf  [ rdf:type                  owl:Restriction;
                           owl:onClass               xsd:string;
                           owl:onProperty            gen:DateAttribute.name;
                           owl:qualifiedCardinality  "1"^^xsd:nonNegativeInteger
                         ];
        skos:definition  "DateAttribute is a data type used to define generic attributes of type \"Date\"."@en .
