@prefix core:       <https://www.opengis.net/ont/citygml/core/> .
@prefix iso19150-2: <http://def.isotc211.org/iso19150/-2/2012/base#> .
@prefix owl:        <http://www.w3.org/2002/07/owl#> .
@prefix rdf:        <http://www.w3.org/1999/02/22-rdf-syntax-ns#> .
@prefix rdfs:       <http://www.w3.org/2000/01/rdf-schema#> .
@prefix sc:         <http://shapechange.net/resources/ont/base#> .
@prefix skos:       <http://www.w3.org/2004/02/skos/core#> .
@prefix veg:        <https://www.opengis.net/ont/citygml/vegetation/> .
@prefix xsd:        <http://www.w3.org/2001/XMLSchema#> .

veg:averageHeight  rdf:type  owl:DatatypeProperty;
        rdfs:label       "averageHeight"@en;
        rdfs:range       sc:Measure;
        skos:definition  "Specifies the average height of the PlantCover."@en .

<https://www.opengis.net/ont/citygml/vegetation>
        rdf:type         owl:Ontology;
        rdfs:label       "Vegetation"@en;
        owl:imports      <https://www.opengis.net/ont/citygml/core> , <http://shapechange.net/resources/ont/base> , <http://def.isotc211.org/iso19150/-2/2012/base>;
        skos:definition  "The Vegetation module supports representation of vegetation objects with vegetation-specific thematic classes. CityGMLâ€™s vegetation model distinguishes between solitary vegetation objects like trees, and vegetation areas which represent biotopes like forests or other plant communities."@en .

veg:PlantCoverUsageValue
        rdf:type         owl:Class;
        rdfs:label       "PlantCoverUsageValue"@en;
        rdfs:subClassOf  skos:Concept;
        skos:definition  "PlantCoverUsageValue is a code list that enumerates the different uses of a PlantCover."@en .

veg:maxRootBallDepth  rdf:type  owl:DatatypeProperty;
        rdfs:label       "maxRootBallDepth"@en;
        rdfs:range       sc:Measure;
        skos:definition  "Specifies the vertical distance between the lowest point of the SolitaryVegetationObject's root ball and the terrain surface."@en .

veg:SolitaryVegetationObject
        rdf:type         owl:Class;
        rdfs:label       "SolitaryVegetationObject"@en;
        rdfs:subClassOf  veg:AbstractVegetationObject;
        rdfs:subClassOf  [ rdf:type           owl:Restriction;
                           owl:allValuesFrom  veg:PlantCoverClassValue;
                           owl:onProperty     veg:class
                         ];
        rdfs:subClassOf  [ rdf:type           owl:Restriction;
                           owl:allValuesFrom  sc:Measure;
                           owl:onProperty     veg:maxRootBallDepth
                         ];
        rdfs:subClassOf  [ rdf:type           owl:Restriction;
                           owl:allValuesFrom  veg:ADEOfSolitaryVegetationObject;
                           owl:onProperty     veg:adeOfSolitaryVegetationObject
                         ];
        rdfs:subClassOf  [ rdf:type           owl:Restriction;
                           owl:allValuesFrom  sc:Measure;
                           owl:onProperty     veg:height
                         ];
        rdfs:subClassOf  [ rdf:type                     owl:Restriction;
                           owl:maxQualifiedCardinality  "1"^^xsd:nonNegativeInteger;
                           owl:onClass                  veg:SpeciesValue;
                           owl:onProperty               veg:species
                         ];
        rdfs:subClassOf  [ rdf:type                     owl:Restriction;
                           owl:maxQualifiedCardinality  "1"^^xsd:nonNegativeInteger;
                           owl:onClass                  sc:Measure;
                           owl:onProperty               veg:maxRootBallDepth
                         ];
        rdfs:subClassOf  [ rdf:type           owl:Restriction;
                           owl:allValuesFrom  veg:PlantCoverFunctionValue;
                           owl:onProperty     veg:function
                         ];
        rdfs:subClassOf  [ rdf:type                     owl:Restriction;
                           owl:maxQualifiedCardinality  "1"^^xsd:nonNegativeInteger;
                           owl:onClass                  sc:Measure;
                           owl:onProperty               veg:trunkDiameter
                         ];
        rdfs:subClassOf  [ rdf:type                     owl:Restriction;
                           owl:maxQualifiedCardinality  "1"^^xsd:nonNegativeInteger;
                           owl:onClass                  sc:Measure;
                           owl:onProperty               veg:height
                         ];
        rdfs:subClassOf  [ rdf:type           owl:Restriction;
                           owl:allValuesFrom  sc:Measure;
                           owl:onProperty     veg:crownDiameter
                         ];
        rdfs:subClassOf  [ rdf:type           owl:Restriction;
                           owl:allValuesFrom  sc:Measure;
                           owl:onProperty     veg:trunkDiameter
                         ];
        rdfs:subClassOf  [ rdf:type                     owl:Restriction;
                           owl:maxQualifiedCardinality  "1"^^xsd:nonNegativeInteger;
                           owl:onClass                  sc:Measure;
                           owl:onProperty               veg:crownDiameter
                         ];
        rdfs:subClassOf  [ rdf:type           owl:Restriction;
                           owl:allValuesFrom  sc:Measure;
                           owl:onProperty     veg:rootBallDiameter
                         ];
        rdfs:subClassOf  [ rdf:type           owl:Restriction;
                           owl:allValuesFrom  veg:SpeciesValue;
                           owl:onProperty     veg:species
                         ];
        rdfs:subClassOf  [ rdf:type           owl:Restriction;
                           owl:allValuesFrom  veg:PlantCoverUsageValue;
                           owl:onProperty     veg:usage
                         ];
        rdfs:subClassOf  [ rdf:type                     owl:Restriction;
                           owl:maxQualifiedCardinality  "1"^^xsd:nonNegativeInteger;
                           owl:onClass                  veg:PlantCoverClassValue;
                           owl:onProperty               veg:class
                         ];
        rdfs:subClassOf  [ rdf:type                     owl:Restriction;
                           owl:maxQualifiedCardinality  "1"^^xsd:nonNegativeInteger;
                           owl:onClass                  sc:Measure;
                           owl:onProperty               veg:rootBallDiameter
                         ];
        skos:definition  "A SolitaryVegetationObject represents individual vegetation objects, e.g. trees or bushes."@en .

veg:usage  rdf:type      owl:ObjectProperty;
        rdfs:label       "usage"@en;
        rdfs:range       veg:PlantCoverUsageValue;
        skos:definition  "Specifies the actual uses of the PlantCover."@en .

veg:SpeciesValue  rdf:type  owl:Class;
        rdfs:label       "SpeciesValue"@en;
        rdfs:subClassOf  skos:Concept;
        skos:definition  "A SpeciesValue is a code list that enumerates the species of a SolitaryVegetationObject."@en .

veg:adeOfSolitaryVegetationObject
        rdf:type         owl:ObjectProperty;
        rdfs:label       "adeOfSolitaryVegetationObject"@en;
        rdfs:range       veg:ADEOfSolitaryVegetationObject;
        skos:definition  "Augments the SolitaryVegetationObject with properties defined in an ADE."@en .

veg:adeOfPlantCover  rdf:type  owl:ObjectProperty;
        rdfs:label       "adeOfPlantCover"@en;
        rdfs:range       veg:ADEOfPlantCover;
        skos:definition  "Augments the PlantCover with properties defined in an ADE."@en .

veg:adeOfAbstractVegetationObject
        rdf:type         owl:ObjectProperty;
        rdfs:label       "adeOfAbstractVegetationObject"@en;
        rdfs:range       veg:ADEOfAbstractVegetationObject;
        skos:definition  "Augments AbstractVegetationObject with properties defined in an ADE."@en .

veg:height  rdf:type     owl:DatatypeProperty;
        rdfs:label       "height"@en;
        rdfs:range       sc:Measure;
        skos:definition  "Distance between the highest point of the vegetation object and the lowest point of the terrain at the bottom of the object."@en .

veg:SolitaryVegetationObjectFunctionValue
        rdf:type         owl:Class;
        rdfs:label       "SolitaryVegetationObjectFunctionValue"@en;
        rdfs:subClassOf  skos:Concept;
        skos:definition  "SolitaryVegetationObjectFunctionValue is a code list that enumerates the different purposes of a SolitaryVegetationObject."@en .

veg:PlantCoverClassValue
        rdf:type         owl:Class;
        rdfs:label       "PlantCoverClassValue"@en;
        rdfs:subClassOf  skos:Concept;
        skos:definition  "PlantCoverClassValue is a code list used to further classify a PlantCover."@en .

veg:minHeight  rdf:type  owl:DatatypeProperty;
        rdfs:label       "minHeight"@en;
        rdfs:range       sc:Measure;
        skos:definition  "Specifies the minimum height of the PlantCover."@en .

veg:SolitaryVegetationObjectUsageValue
        rdf:type         owl:Class;
        rdfs:label       "SolitaryVegetationObjectUsageValue"@en;
        rdfs:subClassOf  skos:Concept;
        skos:definition  "SolitaryVegetationObjectUsageValue is a code list that enumerates the different uses of a SolitaryVegetationObject."@en .

veg:AbstractVegetationObject
        rdf:type               owl:Class;
        rdfs:label             "AbstractVegetationObject"@en;
        rdfs:subClassOf        core:AbstractOccupiedSpace;
        rdfs:subClassOf        [ rdf:type           owl:Restriction;
                                 owl:allValuesFrom  veg:ADEOfAbstractVegetationObject;
                                 owl:onProperty     veg:adeOfAbstractVegetationObject
                               ];
        iso19150-2:isAbstract  true;
        skos:definition        "AbstractVegetationObject is the abstract superclass for all kinds of vegetation objects."@en .

veg:function  rdf:type   owl:ObjectProperty;
        rdfs:label       "function"@en;
        rdfs:range       veg:PlantCoverFunctionValue;
        skos:definition  "Specifies the intended purposes of the PlantCover."@en .

veg:ADEOfSolitaryVegetationObject
        rdf:type               owl:Class;
        rdfs:label             "ADEOfSolitaryVegetationObject"@en;
        iso19150-2:isAbstract  true;
        skos:definition        "ADEOfSolitaryVegetationObject acts as a hook to define properties within an ADE that are to be added to a SolitaryVegetationObject."@en .

veg:class  rdf:type      owl:ObjectProperty;
        rdfs:label       "class"@en;
        rdfs:range       veg:PlantCoverClassValue;
        skos:definition  "Indicates the specific type of the PlantCover."@en .

veg:ADEOfAbstractVegetationObject
        rdf:type               owl:Class;
        rdfs:label             "ADEOfAbstractVegetationObject"@en;
        iso19150-2:isAbstract  true;
        skos:definition        "ADEOfAbstractVegetationObject acts as a hook to define properties within an ADE that are to be added to AbstractVegetationObject."@en .

veg:PlantCoverFunctionValue
        rdf:type         owl:Class;
        rdfs:label       "PlantCoverFunctionValue"@en;
        rdfs:subClassOf  skos:Concept;
        skos:definition  "PlantCoverFunctionValue is a code list that enumerates the different purposes of a PlantCover."@en .

veg:ADEOfPlantCover  rdf:type  owl:Class;
        rdfs:label             "ADEOfPlantCover"@en;
        iso19150-2:isAbstract  true;
        skos:definition        "ADEOfPlantCover acts as a hook to define properties within an ADE that are to be added to a PlantCover."@en .

veg:SolitaryVegetationObjectClassValue
        rdf:type         owl:Class;
        rdfs:label       "SolitaryVegetationObjectClassValue"@en;
        rdfs:subClassOf  skos:Concept;
        skos:definition  "SolitaryVegetationObjectClassValue is a code list used to further classify a SolitaryVegetationObject."@en .

veg:maxHeight  rdf:type  owl:DatatypeProperty;
        rdfs:label       "maxHeight"@en;
        rdfs:range       sc:Measure;
        skos:definition  "Specifies the maximum height of the PlantCover."@en .

veg:trunkDiameter  rdf:type  owl:DatatypeProperty;
        rdfs:label       "trunkDiameter"@en;
        rdfs:range       sc:Measure;
        skos:definition  "Specifies the diameter of the SolitaryCityObject's trunk."@en .

veg:crownDiameter  rdf:type  owl:DatatypeProperty;
        rdfs:label       "crownDiameter"@en;
        rdfs:range       sc:Measure;
        skos:definition  "Specifies the diameter of the SolitaryCityObject's crown."@en .

veg:species  rdf:type    owl:ObjectProperty;
        rdfs:label       "species"@en;
        rdfs:range       veg:SpeciesValue;
        skos:definition  "Indicates the botanical name of the SolitaryVegetationObject."@en .

veg:rootBallDiameter  rdf:type  owl:DatatypeProperty;
        rdfs:label       "rootBallDiameter"@en;
        rdfs:range       sc:Measure;
        skos:definition  "Specifies the diameter of the SolitaryCityObject's root ball."@en .

veg:PlantCover  rdf:type  owl:Class;
        rdfs:label        "PlantCover"@en;
        rdfs:subClassOf   veg:AbstractVegetationObject;
        rdfs:subClassOf   [ rdf:type           owl:Restriction;
                            owl:allValuesFrom  veg:PlantCoverUsageValue;
                            owl:onProperty     veg:usage
                          ];
        rdfs:subClassOf   [ rdf:type           owl:Restriction;
                            owl:allValuesFrom  sc:Measure;
                            owl:onProperty     veg:averageHeight
                          ];
        rdfs:subClassOf   [ rdf:type           owl:Restriction;
                            owl:allValuesFrom  sc:Measure;
                            owl:onProperty     veg:minHeight
                          ];
        rdfs:subClassOf   [ rdf:type           owl:Restriction;
                            owl:allValuesFrom  veg:ADEOfPlantCover;
                            owl:onProperty     veg:adeOfPlantCover
                          ];
        rdfs:subClassOf   [ rdf:type           owl:Restriction;
                            owl:allValuesFrom  veg:PlantCoverFunctionValue;
                            owl:onProperty     veg:function
                          ];
        rdfs:subClassOf   [ rdf:type                     owl:Restriction;
                            owl:maxQualifiedCardinality  "1"^^xsd:nonNegativeInteger;
                            owl:onClass                  sc:Measure;
                            owl:onProperty               veg:maxHeight
                          ];
        rdfs:subClassOf   [ rdf:type                     owl:Restriction;
                            owl:maxQualifiedCardinality  "1"^^xsd:nonNegativeInteger;
                            owl:onClass                  veg:PlantCoverClassValue;
                            owl:onProperty               veg:class
                          ];
        rdfs:subClassOf   [ rdf:type           owl:Restriction;
                            owl:allValuesFrom  sc:Measure;
                            owl:onProperty     veg:maxHeight
                          ];
        rdfs:subClassOf   [ rdf:type           owl:Restriction;
                            owl:allValuesFrom  veg:PlantCoverClassValue;
                            owl:onProperty     veg:class
                          ];
        rdfs:subClassOf   [ rdf:type                     owl:Restriction;
                            owl:maxQualifiedCardinality  "1"^^xsd:nonNegativeInteger;
                            owl:onClass                  sc:Measure;
                            owl:onProperty               veg:minHeight
                          ];
        rdfs:subClassOf   [ rdf:type                     owl:Restriction;
                            owl:maxQualifiedCardinality  "1"^^xsd:nonNegativeInteger;
                            owl:onClass                  sc:Measure;
                            owl:onProperty               veg:averageHeight
                          ];
        owl:disjointWith  veg:SolitaryVegetationObject;
        skos:definition   "A PlantCover represents a space covered by vegetation."@en .
