@prefix brid:       <https://www.opengis.net/ont/citygml/bridge/> .
@prefix con:        <https://www.opengis.net/ont/citygml/construction/> .
@prefix core:       <https://www.opengis.net/ont/citygml/core/> .
@prefix iso19150-2: <http://def.isotc211.org/iso19150/-2/2012/base#> .
@prefix owl:        <http://www.w3.org/2002/07/owl#> .
@prefix rdf:        <http://www.w3.org/1999/02/22-rdf-syntax-ns#> .
@prefix rdfs:       <http://www.w3.org/2000/01/rdf-schema#> .
@prefix skos:       <http://www.w3.org/2004/02/skos/core#> .
@prefix xsd:        <http://www.w3.org/2001/XMLSchema#> .

brid:adeOfBridgeFurniture
        rdf:type         owl:ObjectProperty;
        rdfs:label       "adeOfBridgeFurniture"@en;
        rdfs:range       brid:ADEOfBridgeFurniture;
        skos:definition  "Augments the BridgeFurniture with properties defined in an ADE."@en .

brid:BridgeConstructiveElementClassValue
        rdf:type         owl:Class;
        rdfs:label       "BridgeConstructiveElementClassValue"@en;
        rdfs:subClassOf  skos:Concept;
        skos:definition  "BridgeConstructiveElementClassValue is a code list used to further classify a BridgeConstructiveElement."@en .

brid:BridgeFurniture  rdf:type  owl:Class;
        rdfs:label       "BridgeFurniture"@en;
        rdfs:subClassOf  con:AbstractFurniture;
        rdfs:subClassOf  [ rdf:type           owl:Restriction;
                           owl:allValuesFrom  brid:ADEOfBridgeFurniture;
                           owl:onProperty     brid:adeOfBridgeFurniture
                         ];
        rdfs:subClassOf  [ rdf:type           owl:Restriction;
                           owl:allValuesFrom  brid:BridgeFurnitureUsageValue;
                           owl:onProperty     brid:BridgeFurniture.usage
                         ];
        rdfs:subClassOf  [ rdf:type           owl:Restriction;
                           owl:allValuesFrom  brid:BridgeFurnitureFunctionValue;
                           owl:onProperty     brid:BridgeFurniture.function
                         ];
        rdfs:subClassOf  [ rdf:type           owl:Restriction;
                           owl:allValuesFrom  brid:BridgeFurnitureClassValue;
                           owl:onProperty     brid:BridgeFurniture.class
                         ];
        rdfs:subClassOf  [ rdf:type                     owl:Restriction;
                           owl:maxQualifiedCardinality  "1"^^xsd:nonNegativeInteger;
                           owl:onClass                  brid:BridgeFurnitureClassValue;
                           owl:onProperty               brid:BridgeFurniture.class
                         ];
        skos:definition  "A BridgeFurniture is an equipment for occupant use, usually not fixed to the bridge. [cf. ISO 6707-1]"@en .

brid:BridgeInstallation.class
        rdf:type         owl:ObjectProperty;
        rdfs:domain      brid:BridgeInstallation;
        rdfs:label       "class"@en;
        rdfs:range       brid:BridgeInstallationClassValue;
        skos:definition  "Indicates the specific type of the BridgeInstallation."@en .

brid:BridgeRoomUsageValue
        rdf:type         owl:Class;
        rdfs:label       "BridgeRoomUsageValue"@en;
        rdfs:subClassOf  skos:Concept;
        skos:definition  "BridgeRoomUsageValue is a code list that enumerates the different uses of a BridgeRoom."@en .

brid:bridgeRoom  rdf:type  owl:ObjectProperty;
        rdfs:label       "bridgeRoom"@en;
        rdfs:range       brid:BridgeRoom;
        skos:definition  "Relates the rooms to the Bridge or BridgePart."@en .

brid:BridgeInstallationUsageValue
        rdf:type         owl:Class;
        rdfs:label       "BridgeInstallationUsageValue"@en;
        rdfs:subClassOf  skos:Concept;
        skos:definition  "BridgeInstallationUsageValue is a code list that enumerates the different uses of a BridgeInstallation."@en .

brid:BridgeRoom.function
        rdf:type         owl:ObjectProperty;
        rdfs:domain      brid:BridgeRoom;
        rdfs:label       "function"@en;
        rdfs:range       brid:BridgeRoomFunctionValue;
        skos:definition  "Specifies the intended purposes of the BridgeRoom."@en .

brid:ADEOfAbstractBridge
        rdf:type               owl:Class;
        rdfs:label             "ADEOfAbstractBridge"@en;
        iso19150-2:isAbstract  true;
        skos:definition        "ADEOfAbstractBridge acts as a hook to define properties within an ADE that are to be added to AbstractBridge."@en .

brid:adeOfAbstractBridge
        rdf:type         owl:ObjectProperty;
        rdfs:label       "adeOfAbstractBridge"@en;
        rdfs:range       brid:ADEOfAbstractBridge;
        skos:definition  "Augments AbstractBridge with properties defined in an ADE."@en .

brid:BridgeFunctionValue
        rdf:type         owl:Class;
        rdfs:label       "BridgeFunctionValue"@en;
        rdfs:subClassOf  skos:Concept;
        skos:definition  "BridgeFunctionValue is a code list that enumerates the different purposes of a Bridge."@en .

brid:boundary  rdf:type  owl:ObjectProperty;
        rdfs:label       "boundary"@en;
        rdfs:range       core:AbstractThematicSurface;
        skos:definition  "Relates to the surfaces that bound the BridgeRoom. This relation is inherited from the Core module."@en .

brid:BridgeConstructiveElement.usage
        rdf:type         owl:ObjectProperty;
        rdfs:domain      brid:BridgeConstructiveElement;
        rdfs:label       "usage"@en;
        rdfs:range       brid:BridgeConstructiveElementUsageValue;
        skos:definition  "Specifies the actual uses of the BridgeConstructiveElement."@en .

brid:AbstractBridge.function
        rdf:type         owl:ObjectProperty;
        rdfs:domain      brid:AbstractBridge;
        rdfs:label       "function"@en;
        rdfs:range       brid:BridgeFunctionValue;
        skos:definition  "Specifies the intended purposes of the Bridge or BridgePart."@en .

brid:ADEOfBridgeRoom  rdf:type  owl:Class;
        rdfs:label             "ADEOfBridgeRoom"@en;
        iso19150-2:isAbstract  true;
        skos:definition        "ADEOfBridgeRoom acts as a hook to define properties within an ADE that are to be added to a BridgeRoom."@en .

brid:BridgeConstructiveElement.class
        rdf:type         owl:ObjectProperty;
        rdfs:domain      brid:BridgeConstructiveElement;
        rdfs:label       "class"@en;
        rdfs:range       brid:BridgeConstructiveElementClassValue;
        skos:definition  "Indicates the specific type of the BridgeConstructiveElement."@en .

brid:ADEOfBridgeFurniture
        rdf:type               owl:Class;
        rdfs:label             "ADEOfBridgeFurniture"@en;
        iso19150-2:isAbstract  true;
        skos:definition        "ADEOfBridgeFurniture acts as a hook to define properties within an ADE that are to be added to a BridgeFurniture."@en .

brid:BridgeRoomClassValue
        rdf:type         owl:Class;
        rdfs:label       "BridgeRoomClassValue"@en;
        rdfs:subClassOf  skos:Concept;
        skos:definition  "BridgeRoomClassValue is a code list used to further classify a BridgeRoom."@en .

brid:ADEOfBridgeConstructiveElement
        rdf:type               owl:Class;
        rdfs:label             "ADEOfBridgeConstructiveElement"@en;
        iso19150-2:isAbstract  true;
        skos:definition        "ADEOfBridgeConstructiveElement acts as a hook to define properties within an ADE that are to be added to a BridgeConstructiveElement."@en .

brid:BridgeInstallation.function
        rdf:type         owl:ObjectProperty;
        rdfs:domain      brid:BridgeInstallation;
        rdfs:label       "function"@en;
        rdfs:range       brid:BridgeInstallationFunctionValue;
        skos:definition  "Specifies the intended purposes of the BridgeInstallation."@en .

brid:ADEOfBridgePart  rdf:type  owl:Class;
        rdfs:label             "ADEOfBridgePart"@en;
        iso19150-2:isAbstract  true;
        skos:definition        "ADEOfBridgePart acts as a hook to define properties within an ADE that are to be added to a BridgePart."@en .

brid:isMovable  rdf:type  owl:DatatypeProperty;
        rdfs:label       "isMovable"@en;
        rdfs:range       xsd:boolean;
        skos:definition  "Indicates whether the Bridge or BridgePart can be moved to allow for watercraft to pass."@en .

brid:BridgeFurniture.function
        rdf:type         owl:ObjectProperty;
        rdfs:domain      brid:BridgeFurniture;
        rdfs:label       "function"@en;
        rdfs:range       brid:BridgeFurnitureFunctionValue;
        skos:definition  "Specifies the intended purposes of the BridgeFurniture."@en .

brid:BridgeFurnitureFunctionValue
        rdf:type         owl:Class;
        rdfs:label       "BridgeFurnitureFunctionValue"@en;
        rdfs:subClassOf  skos:Concept;
        skos:definition  "BridgeFurnitureFunctionValue is a code list that enumerates the different purposes of a BridgeFurniture."@en .

brid:adeOfBridge  rdf:type  owl:ObjectProperty;
        rdfs:label       "adeOfBridge"@en;
        rdfs:range       brid:ADEOfBridge;
        skos:definition  "Augments the Bridge with properties defined in an ADE."@en .

brid:BridgeUsageValue
        rdf:type         owl:Class;
        rdfs:label       "BridgeUsageValue"@en;
        rdfs:subClassOf  skos:Concept;
        skos:definition  "BridgeUsageValue is a code list that enumerates the different uses of a Bridge."@en .

brid:BridgeInstallationClassValue
        rdf:type         owl:Class;
        rdfs:label       "BridgeInstallationClassValue"@en;
        rdfs:subClassOf  skos:Concept;
        skos:definition  "BridgeInstallationClassValue is a code list used to further classify a BridgeInstallation."@en .

brid:AbstractBridge.usage
        rdf:type         owl:ObjectProperty;
        rdfs:domain      brid:AbstractBridge;
        rdfs:label       "usage"@en;
        rdfs:range       brid:BridgeUsageValue;
        skos:definition  "Specifies the actual uses of the Bridge or BridgePart."@en .

brid:BridgeRoomFunctionValue
        rdf:type         owl:Class;
        rdfs:label       "BridgeRoomFunctionValue"@en;
        rdfs:subClassOf  skos:Concept;
        skos:definition  "BridgeRoomFunctionValue is a code list that enumerates the different purposes of a BridgeRoom."@en .

brid:BridgePart  rdf:type  owl:Class;
        rdfs:label       "BridgePart"@en;
        rdfs:subClassOf  brid:AbstractBridge;
        rdfs:subClassOf  [ rdf:type           owl:Restriction;
                           owl:allValuesFrom  brid:ADEOfBridgePart;
                           owl:onProperty     brid:adeOfBridgePart
                         ];
        skos:definition  "A BridgePart is a physical or functional subdivision of a Bridge. It would be considered a Bridge, if it were not part of a collection of other BridgeParts."@en .

brid:Bridge  rdf:type     owl:Class;
        rdfs:label        "Bridge"@en;
        rdfs:subClassOf   brid:AbstractBridge;
        rdfs:subClassOf   [ rdf:type           owl:Restriction;
                            owl:allValuesFrom  brid:ADEOfBridge;
                            owl:onProperty     brid:adeOfBridge
                          ];
        rdfs:subClassOf   [ rdf:type           owl:Restriction;
                            owl:allValuesFrom  brid:BridgePart;
                            owl:onProperty     brid:bridgePart
                          ];
        owl:disjointWith  brid:BridgePart;
        skos:definition   "A Bridge represents a structure that affords the passage of pedestrians, animals, vehicles, and service(s) above obstacles or between two points at a height above ground. [cf. ISO 6707-1]"@en .

brid:bridgeConstructiveElement
        rdf:type         owl:ObjectProperty;
        rdfs:label       "bridgeConstructiveElement"@en;
        rdfs:range       brid:BridgeConstructiveElement;
        skos:definition  "Relates the constructive elements to the Bridge or BridgePart."@en .

brid:BridgeRoom.usage
        rdf:type         owl:ObjectProperty;
        rdfs:domain      brid:BridgeRoom;
        rdfs:label       "usage"@en;
        rdfs:range       brid:BridgeRoomUsageValue;
        skos:definition  "Specifies the actual uses of the BridgeRoom."@en .

brid:BridgeFurniture.usage
        rdf:type         owl:ObjectProperty;
        rdfs:domain      brid:BridgeFurniture;
        rdfs:label       "usage"@en;
        rdfs:range       brid:BridgeFurnitureUsageValue;
        skos:definition  "Specifies the actual uses of the BridgeFurniture."@en .

brid:ADEOfBridge  rdf:type     owl:Class;
        rdfs:label             "ADEOfBridge"@en;
        iso19150-2:isAbstract  true;
        skos:definition        "ADEOfBridge acts as a hook to define properties within an ADE that are to be added to a Bridge."@en .

brid:BridgeConstructiveElementFunctionValue
        rdf:type         owl:Class;
        rdfs:label       "BridgeConstructiveElementFunctionValue"@en;
        rdfs:subClassOf  skos:Concept;
        skos:definition  "BridgeConstructiveElementFunctionValue is a code list that enumerates the different purposes of a BridgeConstructiveElement."@en .

brid:BridgeFurnitureUsageValue
        rdf:type         owl:Class;
        rdfs:label       "BridgeFurnitureUsageValue"@en;
        rdfs:subClassOf  skos:Concept;
        skos:definition  "BridgeFurnitureUsageValue is a code list that enumerates the different uses of a BridgeFurniture."@en .

brid:ADEOfBridgeInstallation
        rdf:type               owl:Class;
        rdfs:label             "ADEOfBridgeInstallation"@en;
        iso19150-2:isAbstract  true;
        skos:definition        "ADEOfBridgeInstallation acts as a hook to define properties within an ADE that are to be added to a BridgeInstallation."@en .

brid:AbstractBridge  rdf:type  owl:Class;
        rdfs:label             "AbstractBridge"@en;
        rdfs:subClassOf        con:AbstractConstruction;
        rdfs:subClassOf        [ rdf:type           owl:Restriction;
                                 owl:allValuesFrom  brid:BridgeConstructiveElement;
                                 owl:onProperty     brid:bridgeConstructiveElement
                               ];
        rdfs:subClassOf        [ rdf:type           owl:Restriction;
                                 owl:allValuesFrom  brid:BridgeRoom;
                                 owl:onProperty     brid:bridgeRoom
                               ];
        rdfs:subClassOf        [ rdf:type                     owl:Restriction;
                                 owl:maxQualifiedCardinality  "1"^^xsd:nonNegativeInteger;
                                 owl:onClass                  brid:BridgeClassValue;
                                 owl:onProperty               brid:AbstractBridge.class
                               ];
        rdfs:subClassOf        [ rdf:type           owl:Restriction;
                                 owl:allValuesFrom  core:Address;
                                 owl:onProperty     brid:address
                               ];
        rdfs:subClassOf        [ rdf:type           owl:Restriction;
                                 owl:allValuesFrom  brid:BridgeUsageValue;
                                 owl:onProperty     brid:AbstractBridge.usage
                               ];
        rdfs:subClassOf        [ rdf:type                     owl:Restriction;
                                 owl:maxQualifiedCardinality  "1"^^xsd:nonNegativeInteger;
                                 owl:onClass                  xsd:boolean;
                                 owl:onProperty               brid:isMovable
                               ];
        rdfs:subClassOf        [ rdf:type           owl:Restriction;
                                 owl:allValuesFrom  brid:ADEOfAbstractBridge;
                                 owl:onProperty     brid:adeOfAbstractBridge
                               ];
        rdfs:subClassOf        [ rdf:type           owl:Restriction;
                                 owl:allValuesFrom  brid:BridgeClassValue;
                                 owl:onProperty     brid:AbstractBridge.class
                               ];
        rdfs:subClassOf        [ rdf:type           owl:Restriction;
                                 owl:allValuesFrom  xsd:boolean;
                                 owl:onProperty     brid:isMovable
                               ];
        rdfs:subClassOf        [ rdf:type           owl:Restriction;
                                 owl:allValuesFrom  brid:BridgeInstallation;
                                 owl:onProperty     brid:AbstractBridge.bridgeInstallation
                               ];
        rdfs:subClassOf        [ rdf:type           owl:Restriction;
                                 owl:allValuesFrom  brid:BridgeFurniture;
                                 owl:onProperty     brid:AbstractBridge.bridgeFurniture
                               ];
        rdfs:subClassOf        [ rdf:type           owl:Restriction;
                                 owl:allValuesFrom  brid:BridgeFunctionValue;
                                 owl:onProperty     brid:AbstractBridge.function
                               ];
        iso19150-2:isAbstract  true;
        skos:definition        "AbstractBridge is an abstract superclass representing the common attributes and associations of the classes Bridge and BridgePart."@en .

brid:BridgeRoom  rdf:type  owl:Class;
        rdfs:label       "BridgeRoom"@en;
        rdfs:subClassOf  core:AbstractUnoccupiedSpace;
        rdfs:subClassOf  [ rdf:type           owl:Restriction;
                           owl:allValuesFrom  brid:BridgeRoomFunctionValue;
                           owl:onProperty     brid:BridgeRoom.function
                         ];
        rdfs:subClassOf  [ rdf:type           owl:Restriction;
                           owl:allValuesFrom  brid:BridgeRoomClassValue;
                           owl:onProperty     brid:BridgeRoom.class
                         ];
        rdfs:subClassOf  [ rdf:type           owl:Restriction;
                           owl:allValuesFrom  brid:BridgeRoomUsageValue;
                           owl:onProperty     brid:BridgeRoom.usage
                         ];
        rdfs:subClassOf  [ rdf:type           owl:Restriction;
                           owl:allValuesFrom  core:AbstractThematicSurface;
                           owl:onProperty     brid:boundary
                         ];
        rdfs:subClassOf  [ rdf:type                     owl:Restriction;
                           owl:maxQualifiedCardinality  "1"^^xsd:nonNegativeInteger;
                           owl:onClass                  brid:BridgeRoomClassValue;
                           owl:onProperty               brid:BridgeRoom.class
                         ];
        rdfs:subClassOf  [ rdf:type           owl:Restriction;
                           owl:allValuesFrom  brid:BridgeInstallation;
                           owl:onProperty     brid:BridgeRoom.bridgeInstallation
                         ];
        rdfs:subClassOf  [ rdf:type           owl:Restriction;
                           owl:allValuesFrom  brid:BridgeFurniture;
                           owl:onProperty     brid:BridgeRoom.bridgeFurniture
                         ];
        rdfs:subClassOf  [ rdf:type           owl:Restriction;
                           owl:allValuesFrom  brid:ADEOfBridgeRoom;
                           owl:onProperty     brid:adeOfBridgeRoom
                         ];
        skos:definition  "A BridgeRoom is a space within a Bridge or BridgePart intended for human occupancy (e.g. a place of work or recreation) and/or containment (storage) of animals or things. A BridgeRoom is bounded physically and/or virtually (e.g. by ClosureSurfaces or GenericSurfaces)."@en .

brid:BridgeClassValue
        rdf:type         owl:Class;
        rdfs:label       "BridgeClassValue"@en;
        rdfs:subClassOf  skos:Concept;
        skos:definition  "BridgeClassValue is a code list used to further classify a Bridge."@en .

brid:BridgeInstallation.usage
        rdf:type         owl:ObjectProperty;
        rdfs:domain      brid:BridgeInstallation;
        rdfs:label       "usage"@en;
        rdfs:range       brid:BridgeInstallationUsageValue;
        skos:definition  "Specifies the actual uses of the BridgeInstallation."@en .

brid:BridgeConstructiveElement.function
        rdf:type         owl:ObjectProperty;
        rdfs:domain      brid:BridgeConstructiveElement;
        rdfs:label       "function"@en;
        rdfs:range       brid:BridgeConstructiveElementFunctionValue;
        skos:definition  "Specifies the intended purposes of the BridgeConstructiveElement."@en .

brid:adeOfBridgePart  rdf:type  owl:ObjectProperty;
        rdfs:label       "adeOfBridgePart"@en;
        rdfs:range       brid:ADEOfBridgePart;
        skos:definition  "Augments the BridgePart with properties defined in an ADE."@en .

brid:BridgeConstructiveElementUsageValue
        rdf:type         owl:Class;
        rdfs:label       "BridgeConstructiveElementUsageValue"@en;
        rdfs:subClassOf  skos:Concept;
        skos:definition  "BridgeConstructiveElementUsageValue is a code list that enumerates the different uses of a BridgeConstructiveElement."@en .

brid:BridgeConstructiveElement
        rdf:type         owl:Class;
        rdfs:label       "BridgeConstructiveElement"@en;
        rdfs:subClassOf  con:AbstractConstructiveElement;
        rdfs:subClassOf  [ rdf:type           owl:Restriction;
                           owl:allValuesFrom  brid:ADEOfBridgeConstructiveElement;
                           owl:onProperty     brid:adeOfBridgeConstructiveElement
                         ];
        rdfs:subClassOf  [ rdf:type           owl:Restriction;
                           owl:allValuesFrom  brid:BridgeConstructiveElementUsageValue;
                           owl:onProperty     brid:BridgeConstructiveElement.usage
                         ];
        rdfs:subClassOf  [ rdf:type           owl:Restriction;
                           owl:allValuesFrom  brid:BridgeConstructiveElementFunctionValue;
                           owl:onProperty     brid:BridgeConstructiveElement.function
                         ];
        rdfs:subClassOf  [ rdf:type           owl:Restriction;
                           owl:allValuesFrom  brid:BridgeConstructiveElementClassValue;
                           owl:onProperty     brid:BridgeConstructiveElement.class
                         ];
        rdfs:subClassOf  [ rdf:type                     owl:Restriction;
                           owl:maxQualifiedCardinality  "1"^^xsd:nonNegativeInteger;
                           owl:onClass                  brid:BridgeConstructiveElementClassValue;
                           owl:onProperty               brid:BridgeConstructiveElement.class
                         ];
        skos:definition  "A BridgeConstructiveElement is an element of a bridge which is essential from a structural point of view. Examples are pylons, anchorages, slabs, beams."@en .

brid:BridgeInstallationFunctionValue
        rdf:type         owl:Class;
        rdfs:label       "BridgeInstallationFunctionValue"@en;
        rdfs:subClassOf  skos:Concept;
        skos:definition  "BridgeInstallationFunctionValue is a code list that enumerates the different purposes of a BridgeInstallation."@en .

brid:AbstractBridge.class
        rdf:type         owl:ObjectProperty;
        rdfs:domain      brid:AbstractBridge;
        rdfs:label       "class"@en;
        rdfs:range       brid:BridgeClassValue;
        skos:definition  "Indicates the specific type of the Bridge or BridgePart."@en .

brid:BridgeRoom.bridgeFurniture
        rdf:type         owl:ObjectProperty;
        rdfs:domain      brid:BridgeRoom;
        rdfs:label       "bridgeFurniture"@en;
        rdfs:range       brid:BridgeFurniture;
        skos:definition  "Relates the furniture objects to the BridgeRoom."@en .

brid:address  rdf:type   owl:ObjectProperty;
        rdfs:label       "address"@en;
        rdfs:range       core:Address;
        skos:definition  "Relates the addresses to the Bridge or BridgePart."@en .

brid:BridgeFurnitureClassValue
        rdf:type         owl:Class;
        rdfs:label       "BridgeFurnitureClassValue"@en;
        rdfs:subClassOf  skos:Concept;
        skos:definition  "BridgeFurnitureClassValue is a code list used to further classify a BridgeFurniture."@en .

brid:adeOfBridgeConstructiveElement
        rdf:type         owl:ObjectProperty;
        rdfs:label       "adeOfBridgeConstructiveElement"@en;
        rdfs:range       brid:ADEOfBridgeConstructiveElement;
        skos:definition  "Augments the BridgeConstructiveElement with properties defined in an ADE."@en .

<https://www.opengis.net/ont/citygml/bridge>
        rdf:type         owl:Ontology;
        rdfs:label       "Bridge"@en;
        owl:imports      <https://www.opengis.net/ont/citygml/construction> , <https://www.opengis.net/ont/citygml/core> , <http://def.isotc211.org/iso19150/-2/2012/base>;
        skos:definition  "The Bridge module supports representation of thematic and spatial aspects of bridges, bridge parts, bridge installations, and interior bridge structures."@en .

brid:BridgeFurniture.class
        rdf:type         owl:ObjectProperty;
        rdfs:domain      brid:BridgeFurniture;
        rdfs:label       "class"@en;
        rdfs:range       brid:BridgeFurnitureClassValue;
        skos:definition  "Indicates the specific type of the BridgeFurniture."@en .

brid:BridgeRoom.class
        rdf:type         owl:ObjectProperty;
        rdfs:domain      brid:BridgeRoom;
        rdfs:label       "class"@en;
        rdfs:range       brid:BridgeRoomClassValue;
        skos:definition  "Indicates the specific type of the BridgeRoom."@en .

brid:AbstractBridge.bridgeInstallation
        rdf:type         owl:ObjectProperty;
        rdfs:domain      brid:AbstractBridge;
        rdfs:label       "bridgeInstallation"@en;
        rdfs:range       brid:BridgeInstallation;
        skos:definition  "Relates the installation objects to the Bridge or BridgePart."@en .

brid:adeOfBridgeRoom  rdf:type  owl:ObjectProperty;
        rdfs:label       "adeOfBridgeRoom"@en;
        rdfs:range       brid:ADEOfBridgeRoom;
        skos:definition  "Augments the BridgeRoom with properties defined in an ADE."@en .

brid:bridgePart  rdf:type  owl:ObjectProperty;
        rdfs:label       "bridgePart"@en;
        rdfs:range       brid:BridgePart;
        skos:definition  "Relates the bridge parts to the Bridge."@en .

brid:BridgeInstallation
        rdf:type         owl:Class;
        rdfs:label       "BridgeInstallation"@en;
        rdfs:subClassOf  con:AbstractInstallation;
        rdfs:subClassOf  [ rdf:type           owl:Restriction;
                           owl:allValuesFrom  brid:ADEOfBridgeInstallation;
                           owl:onProperty     brid:adeOfBridgeInstallation
                         ];
        rdfs:subClassOf  [ rdf:type           owl:Restriction;
                           owl:allValuesFrom  brid:BridgeInstallationUsageValue;
                           owl:onProperty     brid:BridgeInstallation.usage
                         ];
        rdfs:subClassOf  [ rdf:type           owl:Restriction;
                           owl:allValuesFrom  brid:BridgeInstallationFunctionValue;
                           owl:onProperty     brid:BridgeInstallation.function
                         ];
        rdfs:subClassOf  [ rdf:type           owl:Restriction;
                           owl:allValuesFrom  brid:BridgeInstallationClassValue;
                           owl:onProperty     brid:BridgeInstallation.class
                         ];
        rdfs:subClassOf  [ rdf:type                     owl:Restriction;
                           owl:maxQualifiedCardinality  "1"^^xsd:nonNegativeInteger;
                           owl:onClass                  brid:BridgeInstallationClassValue;
                           owl:onProperty               brid:BridgeInstallation.class
                         ];
        skos:definition  "A BridgeInstallation is a permanent part of a Bridge (inside and/or outside) which does not have the significance of a BridgePart. In contrast to BridgeConstructiveElements, a BridgeInstallation is not essential from a structural point of view. Examples are stairs, antennas or railways."@en .

brid:AbstractBridge.bridgeFurniture
        rdf:type         owl:ObjectProperty;
        rdfs:domain      brid:AbstractBridge;
        rdfs:label       "bridgeFurniture"@en;
        rdfs:range       brid:BridgeFurniture;
        skos:definition  "Relates the furniture objects to the Bridge or BridgePart."@en .

brid:adeOfBridgeInstallation
        rdf:type         owl:ObjectProperty;
        rdfs:label       "adeOfBridgeInstallation"@en;
        rdfs:range       brid:ADEOfBridgeInstallation;
        skos:definition  "Augments the BridgeInstallation with properties defined in an ADE."@en .

brid:BridgeRoom.bridgeInstallation
        rdf:type         owl:ObjectProperty;
        rdfs:domain      brid:BridgeRoom;
        rdfs:label       "bridgeInstallation"@en;
        rdfs:range       brid:BridgeInstallation;
        skos:definition  "Relates to the installation objects to the BridgeRoom."@en .
