@prefix iso19150-2: <http://def.isotc211.org/iso19150/-2/2012/base#> .
@prefix owl:   <http://www.w3.org/2002/07/owl#> .
@prefix rdf:   <http://www.w3.org/1999/02/22-rdf-syntax-ns#> .
@prefix xsd:   <http://www.w3.org/2001/XMLSchema#> .
@prefix skos:  <http://www.w3.org/2004/02/skos/core#> .
@prefix rdfs:  <http://www.w3.org/2000/01/rdf-schema#> .
@prefix lunom: <http://inspire.ec.europa.eu/ont/lunom#> .

lunom:HILUCSPercentage.hilucsValue
        a                owl:ObjectProperty ;
        rdfs:domain      lunom:HILUCSPercentage ;
        rdfs:range       skos:Concept ;
        rdfs:seeAlso     <http://inspire.ec.europa.eu/codeList/HILUCSValue> ;
        skos:definition  "HILUCS category for this HILUCS percentage."@en .

lunom:SpecificPercentage
        a                owl:Class ;
        rdfs:label       "specific percentage"@en ;
        skos:definition  "Percentage of land use object that is covered by this specific presence."@en .

lunom:SpecificPercentage.specificValue
        a                owl:ObjectProperty ;
        rdfs:domain      lunom:SpecificPercentage ;
        rdfs:range       skos:Concept ;
        skos:definition  "specific value category for this specific percentage."@en .

<http://inspire.ec.europa.eu/ont/lunom>
        a                owl:Ontology ;
        rdfs:label       "land use nomenclature"@en ;
        owl:imports      <http://www.w3.org/2004/02/skos/core> , <http://def.isotc211.org/iso19150/-2/2012/base> ;
        owl:versionIRI   "http://inspire.ec.europa.eu/ont/lunom/4.0" ;
        owl:versionInfo  "4.0" .

lunom:percentage  a      owl:DatatypeProperty ;
        rdfs:comment     "NOTE The percentage is according to the socio-economic importance of the use. In section 5.2.1.1.2. examples of the use of percentages are given."@en ;
        rdfs:range       xsd:integer ;
        skos:definition  "Percentage of land use object that is covered by a specific presence."@en .

lunom:HILUCSPercentage
        a                owl:Class ;
        rdfs:comment     "NOTE1:The percentage is according to the socio-economic or functional importance of the use.\r\n\r\nNOTE2:examples are provided in the narrative description part of the data specification."@en ;
        rdfs:label       "HILUCS percentage"@en ;
        skos:definition  "Percentage of land use object that is covered by this HILUCS presence."@en .
