@prefix app:           <https://www.opengis.net/ont/citygml/appearance/> .
@prefix bldg:          <https://www.opengis.net/ont/citygml/building/> .
@prefix brid:          <https://www.opengis.net/ont/citygml/bridge/> .
@prefix con:           <https://www.opengis.net/ont/citygml/construction/> .
@prefix core:          <https://www.opengis.net/ont/citygml/core/> .
@prefix dem:           <https://www.opengis.net/ont/citygml/relief/> .
@prefix doc:           <https://www.opengis.net/ont/citygml/document/> .
@prefix dyn:           <https://www.opengis.net/ont/citygml/dynamizer/> .
@prefix frn:           <https://www.opengis.net/ont/citygml/cityfurniture/> .
@prefix gen:           <https://www.opengis.net/ont/citygml/generics/> .
@prefix gmlowl:        <http://www.opengis.net/ont/gml#> .
@prefix grp:           <https://www.opengis.net/ont/citygml/cityobjectgroup/> .
@prefix iso19109:      <http://def.isotc211.org/iso19109/2015/GeneralFeatureModel#> .
@prefix iso19111-2019: <http://def.isotc211.org/iso19111/2019/CoordinateReferenceSystems#> .
@prefix iso19136-bt:   <http://def.isotc211.org/iso19136/2007/BasicTypes#> .
@prefix iso19150-2:    <http://def.isotc211.org/iso19150/-2/2012/base#> .
@prefix luse:          <https://www.opengis.net/ont/citygml/landuse/> .
@prefix owl:           <http://www.w3.org/2002/07/owl#> .
@prefix rdf:           <http://www.w3.org/1999/02/22-rdf-syntax-ns#> .
@prefix rdfs:          <http://www.w3.org/2000/01/rdf-schema#> .
@prefix skos:          <http://www.w3.org/2004/02/skos/core#> .
@prefix tran:          <https://www.opengis.net/ont/citygml/transportation/> .
@prefix tun:           <https://www.opengis.net/ont/citygml/tunnel/> .
@prefix veg:           <https://www.opengis.net/ont/citygml/vegetation/> .
@prefix wksp:          <https://www.opengis.net/ont/citygml/workspace/> .
@prefix wtr:           <https://www.opengis.net/ont/citygml/waterbody/> .
@prefix xsd:           <http://www.w3.org/2001/XMLSchema#> .

core:volume  rdf:type    owl:ObjectProperty;
        rdfs:label       "volume"@en;
        rdfs:range       core:QualifiedVolume;
        skos:definition  "Specifies qualified volumes related to the space."@en .

core:MimeTypeValue  rdf:type  owl:Class;
        rdfs:label       "MimeTypeValue"@en;
        rdfs:subClassOf  skos:Concept;
        skos:definition  "MimeTypeValue is a code list used to specify the MIME type of a referenced resource."@en .

core:RelativeToWater  rdf:type  rdfs:Datatype;
        rdfs:label       "RelativeToWater"@en;
        owl:oneOf        ( "entirelyAboveWaterSurface" "substantiallyAboveWaterSurface" "substantiallyAboveAndBelowWaterSurface" "substantiallyBelowWaterSurface" "entirelyBelowWaterSurface" "temporarilyAboveAndBelowWaterSurface" );
        skos:definition  "RelativeToWater enumerates the spatial relations of a city object relative to the water surface in a qualitative way."@en .

core:AbstractThematicSurface.lod0MultiSurface
        rdf:type         owl:ObjectProperty;
        rdfs:domain      core:AbstractThematicSurface;
        rdfs:label       "lod0MultiSurface"@en;
        rdfs:range       gmlowl:MultiSurface;
        skos:definition  "Relates to a 3D MultiSurface geometry that represents the thematic surface in Level of Detail 0."@en .

core:adeOfAbstractVersion
        rdf:type         owl:ObjectProperty;
        rdfs:label       "adeOfAbstractVersion"@en;
        rdfs:range       core:ADEOfAbstractVersion;
        skos:definition  "Augments AbstractVersion with properties defined in an ADE."@en .

core:targetResource  rdf:type  owl:DatatypeProperty;
        rdfs:label       "targetResource"@en;
        rdfs:range       xsd:anyURI;
        skos:definition  "Specifies the URI that points to the object in the external information system."@en .

core:TopologicalRelationTypeValue
        rdf:type         owl:Class;
        rdfs:label       "TopologicalRelationTypeValue"@en;
        rdfs:subClassOf  skos:Concept;
        skos:definition  "TopologicalRelationTypeValue is a code list used to classify topological city object relations."@en .

core:QualifiedVolume  rdf:type  owl:Class;
        rdfs:label       "QualifiedVolume"@en;
        rdfs:subClassOf  [ rdf:type           owl:Restriction;
                           owl:allValuesFrom  core:QualifiedVolumeTypeValue;
                           owl:onProperty     core:typeOfVolume
                         ];
        rdfs:subClassOf  [ rdf:type                  owl:Restriction;
                           owl:onClass               core:QualifiedVolumeTypeValue;
                           owl:onProperty            core:typeOfVolume;
                           owl:qualifiedCardinality  "1"^^xsd:nonNegativeInteger
                         ];
        rdfs:subClassOf  [ rdf:type           owl:Restriction;
                           owl:allValuesFrom  core:QualifiedVolume;
                           owl:onProperty     core:volume
                         ];
        rdfs:subClassOf  [ rdf:type                  owl:Restriction;
                           owl:onClass               core:QualifiedVolume;
                           owl:onProperty            core:volume;
                           owl:qualifiedCardinality  "1"^^xsd:nonNegativeInteger
                         ];
        skos:definition  "QualifiedVolume is an application-dependent measure of the volume of a space."@en .

core:area  rdf:type      owl:ObjectProperty;
        rdfs:label       "area"@en;
        rdfs:range       core:QualifiedArea;
        skos:definition  "Specifies qualified areas related to the space."@en .

core:ADEOfAbstractOccupiedSpace
        rdf:type               owl:Class;
        rdfs:label             "ADEOfAbstractOccupiedSpace"@en;
        iso19150-2:isAbstract  true;
        skos:definition        "ADEOfAbstractOccupiedSpace acts as a hook to define properties within an ADE that are to be added to AbstractOccupiedSpace."@en .

core:validFrom  rdf:type  owl:DatatypeProperty;
        rdfs:label       "validFrom"@en;
        rdfs:range       xsd:dateTime;
        skos:definition  "Indicates the date at which a CityGML feature started to exist in the real world."@en .

core:AbstractCityObject.dynamizer
        rdf:type         owl:ObjectProperty;
        rdfs:domain      core:AbstractCityObject;
        rdfs:label       "dynamizer"@en;
        rdfs:range       core:AbstractDynamizer;
        skos:definition  "Relates Dynamizer objects to the city object. These allow timeseries data to override static attribute values of the city object."@en .

core:ADEOfClosureSurface
        rdf:type               owl:Class;
        rdfs:label             "ADEOfClosureSurface"@en;
        iso19150-2:isAbstract  true;
        skos:definition        "ADEOfClosureSurface acts as a hook to define properties within an ADE that are to be added to a ClosureSurface."@en .

[ rdf:type     owl:AllDisjointClasses;
  owl:members  ( gen:CodeAttribute gen:DateAttribute gen:DoubleAttribute gen:GenericAttributeSet gen:IntAttribute gen:MeasureAttribute gen:StringAttribute gen:UriAttribute )
] .

core:ID  rdf:type        owl:Class;
        rdfs:label       "ID"@en;
        skos:definition  "ID is a basic type that represents a unique identifier."@en .

core:ImplicitGeometry
        rdf:type         owl:Class;
        rdfs:label       "ImplicitGeometry"@en;
        rdfs:subClassOf  [ rdf:type           owl:Restriction;
                           owl:allValuesFrom  xsd:anyURI;
                           owl:onProperty     core:libraryObject
                         ];
        rdfs:subClassOf  [ rdf:type                     owl:Restriction;
                           owl:maxQualifiedCardinality  "1"^^xsd:nonNegativeInteger;
                           owl:onClass                  xsd:anyURI;
                           owl:onProperty               core:libraryObject
                         ];
        rdfs:subClassOf  [ rdf:type           owl:Restriction;
                           owl:allValuesFrom  core:TransformationMatrix4x4;
                           owl:onProperty     core:transformationMatrix
                         ];
        rdfs:subClassOf  [ rdf:type                  owl:Restriction;
                           owl:onClass               gmlowl:Point;
                           owl:onProperty            core:ImplicitGeometry.referencePoint;
                           owl:qualifiedCardinality  "1"^^xsd:nonNegativeInteger
                         ];
        rdfs:subClassOf  [ rdf:type                     owl:Restriction;
                           owl:maxQualifiedCardinality  "1"^^xsd:nonNegativeInteger;
                           owl:onClass                  gmlowl:AbstractGeometry;
                           owl:onProperty               core:ImplicitGeometry.relativeGeometry
                         ];
        rdfs:subClassOf  [ rdf:type           owl:Restriction;
                           owl:allValuesFrom  core:ID;
                           owl:onProperty     core:objectID
                         ];
        rdfs:subClassOf  [ rdf:type           owl:Restriction;
                           owl:allValuesFrom  core:MimeTypeValue;
                           owl:onProperty     core:mimeType
                         ];
        rdfs:subClassOf  [ rdf:type                  owl:Restriction;
                           owl:onClass               core:TransformationMatrix4x4;
                           owl:onProperty            core:transformationMatrix;
                           owl:qualifiedCardinality  "1"^^xsd:nonNegativeInteger
                         ];
        rdfs:subClassOf  [ rdf:type           owl:Restriction;
                           owl:allValuesFrom  gmlowl:AbstractGeometry;
                           owl:onProperty     core:ImplicitGeometry.relativeGeometry
                         ];
        rdfs:subClassOf  [ rdf:type                  owl:Restriction;
                           owl:onClass               core:ID;
                           owl:onProperty            core:objectID;
                           owl:qualifiedCardinality  "1"^^xsd:nonNegativeInteger
                         ];
        rdfs:subClassOf  [ rdf:type           owl:Restriction;
                           owl:allValuesFrom  core:AbstractAppearance;
                           owl:onProperty     core:ImplicitGeometry.appearance
                         ];
        rdfs:subClassOf  [ rdf:type           owl:Restriction;
                           owl:allValuesFrom  gmlowl:Point;
                           owl:onProperty     core:ImplicitGeometry.referencePoint
                         ];
        rdfs:subClassOf  [ rdf:type                     owl:Restriction;
                           owl:maxQualifiedCardinality  "1"^^xsd:nonNegativeInteger;
                           owl:onClass                  core:MimeTypeValue;
                           owl:onProperty               core:mimeType
                         ];
        skos:definition  "ImplicitGeometry is a geometry representation where the shape is stored only once as a prototypical geometry. Examples are a tree or other vegetation object, a traffic light or a traffic sign. This prototypic geometry object can be re-used or referenced many times, wherever the corresponding feature occurs in the 3D city model."@en .

core:TransformationMatrix2x2
        rdf:type         owl:Class;
        rdfs:label       "TransformationMatrix2x2"@en;
        rdfs:subClassOf  core:DoubleList;
        skos:definition  "TransformationMatrix2x2 is a 2 by 2 matrix represented as a list of four double values in row major order."@en .

core:AbstractSpace.lod2Solid
        rdf:type         owl:ObjectProperty;
        rdfs:domain      core:AbstractSpace;
        rdfs:label       "lod2Solid"@en;
        rdfs:range       gmlowl:Solid;
        skos:definition  "Relates to a 3D Solid geometry that represents the space in Level of Detail 2."@en .

core:AbstractSpace.lod0MultiSurface
        rdf:type         owl:ObjectProperty;
        rdfs:domain      core:AbstractSpace;
        rdfs:label       "lod0MultiSurface"@en;
        rdfs:range       gmlowl:MultiSurface;
        skos:definition  "Relates to a 3D MultiSurface geometry that represents the space in Level of Detail 0."@en .

core:occupantType  rdf:type  owl:ObjectProperty;
        rdfs:label       "occupantType"@en;
        rdfs:range       core:OccupantTypeValue;
        skos:definition  "Indicates the specific type of the occupants that are contained by a feature."@en .

core:adeOfAbstractFeature
        rdf:type         owl:ObjectProperty;
        rdfs:label       "adeOfAbstractFeature"@en;
        rdfs:range       core:ADEOfAbstractFeature;
        skos:definition  "Augments AbstractFeature with properties defined in an ADE."@en .

core:name  rdf:type      owl:DatatypeProperty;
        rdfs:label       "name"@en;
        rdfs:range       xsd:Name;
        skos:definition  "Specifies the name of the feature."@en .

core:adeOfAbstractAppearance
        rdf:type         owl:ObjectProperty;
        rdfs:label       "adeOfAbstractAppearance"@en;
        rdfs:range       core:ADEOfAbstractAppearance;
        skos:definition  "Augments AbstractAppearance with properties defined in an ADE."@en .

core:adeOfAbstractUnoccupiedSpace
        rdf:type         owl:ObjectProperty;
        rdfs:label       "adeOfAbstractUnoccupiedSpace"@en;
        rdfs:range       core:ADEOfAbstractUnoccupiedSpace;
        skos:definition  "Augments AbstractUnoccupiedSpace with properties defined in an ADE."@en .

core:numberOfOccupants
        rdf:type         owl:DatatypeProperty;
        rdfs:label       "numberOfOccupants"@en;
        rdfs:range       xsd:integer;
        skos:definition  "Indicates the number of occupants contained by a feature."@en .

core:informationSystem
        rdf:type         owl:DatatypeProperty;
        rdfs:label       "informationSystem"@en;
        rdfs:range       xsd:anyURI;
        skos:definition  "Specifies the URI that points to the external information system."@en .

core:CityObjectRelation.genericAttribute
        rdf:type         owl:ObjectProperty;
        rdfs:domain      core:CityObjectRelation;
        rdfs:label       "genericAttribute"@en;
        rdfs:range       core:AbstractGenericAttribute;
        skos:definition  "Relates generic attributes to the CityObjectRelation."@en .

core:description  rdf:type  owl:DatatypeProperty;
        rdfs:label       "description"@en;
        rdfs:range       xsd:string;
        skos:definition  "Provides further information on the feature."@en .

core:ADEOfAbstractVersion
        rdf:type               owl:Class;
        rdfs:label             "ADEOfAbstractVersion"@en;
        iso19150-2:isAbstract  true;
        skos:definition        "ADEOfAbstractVersion acts as a hook to define properties within an ADE that are to be added to AbstractVersion."@en .

core:TransformationMatrix3x4
        rdf:type         owl:Class;
        rdfs:label       "TransformationMatrix3x4"@en;
        rdfs:subClassOf  core:DoubleList;
        skos:definition  "TransformationMatrix3x4 is a 3 by 4 matrix represented as a list of twelve double values in row major order."@en .

core:AbstractSpace.lod1Solid
        rdf:type         owl:ObjectProperty;
        rdfs:domain      core:AbstractSpace;
        rdfs:label       "lod1Solid"@en;
        rdfs:range       gmlowl:Solid;
        skos:definition  "Relates to a 3D Solid geometry that represents the space in Level of Detail 1."@en .

core:adeOfAbstractThematicSurface
        rdf:type         owl:ObjectProperty;
        rdfs:label       "adeOfAbstractThematicSurface"@en;
        rdfs:range       core:ADEOfAbstractThematicSurface;
        skos:definition  "Augments AbstractThematicSurface with properties defined in an ADE."@en .

core:ADEOfAbstractDynamizer
        rdf:type               owl:Class;
        rdfs:label             "ADEOfAbstractDynamizer"@en;
        iso19150-2:isAbstract  true;
        skos:definition        "ADEOfAbstractDynamizer acts as a hook to define properties within an ADE that are to be added to AbstractDynamizer."@en .

core:ADEOfAbstractVersionTransition
        rdf:type               owl:Class;
        rdfs:label             "ADEOfAbstractVersionTransition"@en;
        iso19150-2:isAbstract  true;
        skos:definition        "ADEOfAbstractVersionTransition acts as a hook to define properties within an ADE that are to be added to AbstractVersionTransition."@en .

core:AbstractVersion  rdf:type  owl:Class;
        rdfs:label             "AbstractVersion"@en;
        rdfs:subClassOf        core:AbstractFeatureWithLifespan;
        rdfs:subClassOf        [ rdf:type           owl:Restriction;
                                 owl:allValuesFrom  core:ADEOfAbstractVersion;
                                 owl:onProperty     core:adeOfAbstractVersion
                               ];
        iso19150-2:isAbstract  true;
        skos:definition        "AbstractVersion is the abstract superclass to represent Version objects."@en .

core:cityObjectMember
        rdf:type         owl:ObjectProperty;
        rdfs:label       "cityObjectMember"@en;
        rdfs:range       core:AbstractCityObject;
        skos:definition  "Specifies the city objects that are part of the CityModel."@en .

core:AbstractOccupiedSpace
        rdf:type               owl:Class;
        rdfs:label             "AbstractOccupiedSpace"@en;
        rdfs:subClassOf        core:AbstractPhysicalSpace;
        rdfs:subClassOf        [ rdf:type           owl:Restriction;
                                 owl:allValuesFrom  core:ImplicitGeometry;
                                 owl:onProperty     core:AbstractOccupiedSpace.lod3ImplicitRepresentation
                               ];
        rdfs:subClassOf        [ rdf:type                     owl:Restriction;
                                 owl:maxQualifiedCardinality  "1"^^xsd:nonNegativeInteger;
                                 owl:onClass                  core:ImplicitGeometry;
                                 owl:onProperty               core:AbstractOccupiedSpace.lod2ImplicitRepresentation
                               ];
        rdfs:subClassOf        [ rdf:type           owl:Restriction;
                                 owl:allValuesFrom  core:ImplicitGeometry;
                                 owl:onProperty     core:AbstractOccupiedSpace.lod1ImplicitRepresentation
                               ];
        rdfs:subClassOf        [ rdf:type           owl:Restriction;
                                 owl:allValuesFrom  core:ADEOfAbstractOccupiedSpace;
                                 owl:onProperty     core:adeOfAbstractOccupiedSpace
                               ];
        rdfs:subClassOf        [ rdf:type                     owl:Restriction;
                                 owl:maxQualifiedCardinality  "1"^^xsd:nonNegativeInteger;
                                 owl:onClass                  core:ImplicitGeometry;
                                 owl:onProperty               core:AbstractOccupiedSpace.lod1ImplicitRepresentation
                               ];
        rdfs:subClassOf        [ rdf:type                     owl:Restriction;
                                 owl:maxQualifiedCardinality  "1"^^xsd:nonNegativeInteger;
                                 owl:onClass                  core:ImplicitGeometry;
                                 owl:onProperty               core:AbstractOccupiedSpace.lod3ImplicitRepresentation
                               ];
        rdfs:subClassOf        [ rdf:type           owl:Restriction;
                                 owl:allValuesFrom  core:ImplicitGeometry;
                                 owl:onProperty     core:AbstractOccupiedSpace.lod2ImplicitRepresentation
                               ];
        iso19150-2:isAbstract  true;
        owl:disjointWith       core:AbstractUnoccupiedSpace;
        skos:definition        "AbstractOccupiedSpace is the abstract superclass for all types of physically occupied spaces. Occupied space refers to spaces that are partially or entirely filled with matter."@en .

core:AbstractDynamizer
        rdf:type               owl:Class;
        rdfs:label             "AbstractDynamizer"@en;
        rdfs:subClassOf        core:AbstractFeatureWithLifespan;
        rdfs:subClassOf        [ rdf:type           owl:Restriction;
                                 owl:allValuesFrom  core:ADEOfAbstractDynamizer;
                                 owl:onProperty     core:adeOfAbstractDynamizer
                               ];
        iso19150-2:isAbstract  true;
        skos:definition        "AbstractDynamizer is the abstract superclass to represent Dynamizer objects."@en .

core:AbstractAppearance
        rdf:type               owl:Class;
        rdfs:label             "AbstractAppearance"@en;
        rdfs:subClassOf        core:AbstractFeatureWithLifespan;
        rdfs:subClassOf        [ rdf:type           owl:Restriction;
                                 owl:allValuesFrom  core:ADEOfAbstractAppearance;
                                 owl:onProperty     core:adeOfAbstractAppearance
                               ];
        iso19150-2:isAbstract  true;
        skos:definition        "AbstractAppearance is the abstract superclass to represent any kind of appearance objects."@en .

core:adeOfCityModel  rdf:type  owl:ObjectProperty;
        rdfs:label       "adeOfCityModel"@en;
        rdfs:range       core:ADEOfCityModel;
        skos:definition  "Augments the CityModel with properties defined in an ADE."@en .

core:AbstractThematicSurface.lod1MultiSurface
        rdf:type         owl:ObjectProperty;
        rdfs:domain      core:AbstractThematicSurface;
        rdfs:label       "lod1MultiSurface"@en;
        rdfs:range       gmlowl:MultiSurface;
        skos:definition  "Relates to a 3D MultiSurface geometry that represents the thematic surface in Level of Detail 1."@en .

core:AbstractCityObject.appearance
        rdf:type         owl:ObjectProperty;
        rdfs:domain      core:AbstractCityObject;
        rdfs:label       "appearance"@en;
        rdfs:range       core:AbstractAppearance;
        skos:definition  "Relates appearances to the city object."@en .

core:adeOfAddress  rdf:type  owl:ObjectProperty;
        rdfs:label       "adeOfAddress"@en;
        rdfs:range       core:ADEOfAddress;
        skos:definition  "Augments the Address with properties defined in an ADE."@en .

core:adeOfClosureSurface
        rdf:type         owl:ObjectProperty;
        rdfs:label       "adeOfClosureSurface"@en;
        rdfs:range       core:ADEOfClosureSurface;
        skos:definition  "Augments the ClosureSurface with properties defined in an ADE."@en .

core:adeOfAbstractOccupiedSpace
        rdf:type         owl:ObjectProperty;
        rdfs:label       "adeOfAbstractOccupiedSpace"@en;
        rdfs:range       core:ADEOfAbstractOccupiedSpace;
        skos:definition  "Augments AbstractOccupiedSpace with properties defined in an ADE."@en .

core:NilReason  rdf:type  owl:Class;
        rdfs:label       "NilReason"@en;
        rdfs:subClassOf  [ rdf:type     owl:Class;
                           owl:unionOf  ( [ rdf:type            owl:Class;
                                            owl:intersectionOf  ( [ rdf:type                  owl:Restriction;
                                                                    owl:onClass               core:NilReasonEnumeration;
                                                                    owl:onProperty            core:nilReasonEnumeration;
                                                                    owl:qualifiedCardinality  "1"^^xsd:nonNegativeInteger
                                                                  ]
                                                                  [ rdf:type         owl:Restriction;
                                                                    owl:cardinality  "0"^^xsd:nonNegativeInteger;
                                                                    owl:onProperty   core:uRI
                                                                  ]
                                                                )
                                          ]
                                          [ rdf:type            owl:Class;
                                            owl:intersectionOf  ( [ rdf:type         owl:Restriction;
                                                                    owl:cardinality  "0"^^xsd:nonNegativeInteger;
                                                                    owl:onProperty   core:nilReasonEnumeration
                                                                  ]
                                                                  [ rdf:type                  owl:Restriction;
                                                                    owl:onClass               xsd:anyURI;
                                                                    owl:onProperty            core:uRI;
                                                                    owl:qualifiedCardinality  "1"^^xsd:nonNegativeInteger
                                                                  ]
                                                                )
                                          ]
                                        )
                         ];
        rdfs:subClassOf  [ rdf:type           owl:Restriction;
                           owl:allValuesFrom  xsd:anyURI;
                           owl:onProperty     core:uRI
                         ];
        rdfs:subClassOf  [ rdf:type           owl:Restriction;
                           owl:allValuesFrom  core:NilReasonEnumeration;
                           owl:onProperty     core:nilReasonEnumeration
                         ];
        skos:definition  "NilReason is a union type that allows for choosing between two different types of nil reason."@en .

core:ImplicitGeometry.relativeGeometry
        rdf:type         owl:ObjectProperty;
        rdfs:domain      core:ImplicitGeometry;
        rdfs:label       "relativeGeometry"@en;
        rdfs:range       gmlowl:AbstractGeometry;
        skos:definition  "Relates to a prototypical geometry in a local coordinate system stored inline with the city model."@en .

core:DoubleOrNilReasonList
        rdf:type         owl:Class;
        rdfs:label       "DoubleOrNilReasonList"@en;
        rdfs:subClassOf  [ rdf:type           owl:Restriction;
                           owl:allValuesFrom  xsd:double;
                           owl:onProperty     core:list
                         ];
        rdfs:subClassOf  [ rdf:type                  owl:Restriction;
                           owl:onClass               xsd:double;
                           owl:onProperty            core:list;
                           owl:qualifiedCardinality  "1"^^xsd:nonNegativeInteger
                         ];
        skos:definition  "DoubleOrNilReasonList is a basic type that represents a list of double values and/or nil reasons."@en .

core:validTo  rdf:type   owl:DatatypeProperty;
        rdfs:label       "validTo"@en;
        rdfs:range       xsd:dateTime;
        skos:definition  "Indicates the date at which a CityGML feature ended to exist in the real world."@en .

core:CityObjectRelation.relatedTo
        rdf:type         owl:ObjectProperty;
        rdfs:domain      core:CityObjectRelation;
        rdfs:label       "relatedTo"@en;
        rdfs:range       core:AbstractCityObject;
        skos:definition  "Relates other city objects to the city object. It also describes how the city objects are related to each other."@en .

core:CityModel  rdf:type  owl:Class;
        rdfs:label       "CityModel"@en;
        rdfs:subClassOf  core:AbstractFeatureWithLifespan;
        rdfs:subClassOf  [ rdf:type           owl:Restriction;
                           owl:allValuesFrom  core:ADEOfCityModel;
                           owl:onProperty     core:adeOfCityModel
                         ];
        rdfs:subClassOf  [ rdf:type           owl:Restriction;
                           owl:allValuesFrom  core:CityModelMember;
                           owl:onProperty     core:CityModel.cityModelMember
                         ];
        rdfs:subClassOf  [ rdf:type           owl:Restriction;
                           owl:allValuesFrom  iso19111-2019:EngineeringCRS;
                           owl:onProperty     core:engineeringCRS
                         ];
        rdfs:subClassOf  [ rdf:type                     owl:Restriction;
                           owl:maxQualifiedCardinality  "1"^^xsd:nonNegativeInteger;
                           owl:onClass                  iso19111-2019:EngineeringCRS;
                           owl:onProperty               core:engineeringCRS
                         ];
        skos:definition  "CityModel is the container for all objects belonging to a city model."@en .

core:adeOfAbstractSpace
        rdf:type         owl:ObjectProperty;
        rdfs:label       "adeOfAbstractSpace"@en;
        rdfs:range       core:ADEOfAbstractSpace;
        skos:definition  "Augments AbstractSpace with properties defined in an ADE."@en .

core:AbstractThematicSurface.lod0MultiCurve
        rdf:type         owl:ObjectProperty;
        rdfs:domain      core:AbstractThematicSurface;
        rdfs:label       "lod0MultiCurve"@en;
        rdfs:range       gmlowl:MultiCurve;
        skos:definition  "Relates to a 3D MultiCurve geometry that represents the thematic surface in Level of Detail 0."@en .

core:adeOfAbstractDynamizer
        rdf:type         owl:ObjectProperty;
        rdfs:label       "adeOfAbstractDynamizer"@en;
        rdfs:range       core:ADEOfAbstractDynamizer;
        skos:definition  "Augments AbstractDynamizer with properties defined in an ADE."@en .

core:DoubleList  rdf:type  owl:Class;
        rdfs:label       "DoubleList"@en;
        rdfs:subClassOf  [ rdf:type           owl:Restriction;
                           owl:allValuesFrom  xsd:double;
                           owl:onProperty     core:list
                         ];
        rdfs:subClassOf  [ rdf:type                  owl:Restriction;
                           owl:onClass               xsd:double;
                           owl:onProperty            core:list;
                           owl:qualifiedCardinality  "1"^^xsd:nonNegativeInteger
                         ];
        skos:definition  "DoubleList is an ordered sequence of double values."@en .

core:CityObjectRelation
        rdf:type         owl:Class;
        rdfs:label       "CityObjectRelation"@en;
        rdfs:subClassOf  [ rdf:type           owl:Restriction;
                           owl:allValuesFrom  core:AbstractCityObject;
                           owl:onProperty     core:CityObjectRelation.relatedTo
                         ];
        rdfs:subClassOf  [ rdf:type                  owl:Restriction;
                           owl:onClass               core:AbstractCityObject;
                           owl:onProperty            core:CityObjectRelation.relatedTo;
                           owl:qualifiedCardinality  "1"^^xsd:nonNegativeInteger
                         ];
        rdfs:subClassOf  [ rdf:type           owl:Restriction;
                           owl:allValuesFrom  core:RelationTypeValue;
                           owl:onProperty     core:relationType
                         ];
        rdfs:subClassOf  [ rdf:type                  owl:Restriction;
                           owl:onClass               core:RelationTypeValue;
                           owl:onProperty            core:relationType;
                           owl:qualifiedCardinality  "1"^^xsd:nonNegativeInteger
                         ];
        rdfs:subClassOf  [ rdf:type           owl:Restriction;
                           owl:allValuesFrom  core:AbstractGenericAttribute;
                           owl:onProperty     core:CityObjectRelation.genericAttribute
                         ];
        skos:definition  "CityObjectRelation represents a specific relation from the city object in which the relation is included to another city object."@en .

core:ADEOfAbstractFeature
        rdf:type               owl:Class;
        rdfs:label             "ADEOfAbstractFeature"@en;
        iso19150-2:isAbstract  true;
        skos:definition        "ADEOfAbstractFeature acts as a hook to define properties within an ADE that are to be added to AbstractFeature."@en .

core:CityModelMember  rdf:type  owl:Class;
        rdfs:label       "CityModelMember"@en;
        rdfs:subClassOf  [ rdf:type     owl:Class;
                           owl:unionOf  ( [ rdf:type            owl:Class;
                                            owl:intersectionOf  ( [ rdf:type                  owl:Restriction;
                                                                    owl:onClass               core:AbstractCityObject;
                                                                    owl:onProperty            core:cityObjectMember;
                                                                    owl:qualifiedCardinality  "1"^^xsd:nonNegativeInteger
                                                                  ]
                                                                  [ rdf:type         owl:Restriction;
                                                                    owl:cardinality  "0"^^xsd:nonNegativeInteger;
                                                                    owl:onProperty   core:appearanceMember
                                                                  ]
                                                                  [ rdf:type         owl:Restriction;
                                                                    owl:cardinality  "0"^^xsd:nonNegativeInteger;
                                                                    owl:onProperty   core:versionMember
                                                                  ]
                                                                  [ rdf:type         owl:Restriction;
                                                                    owl:cardinality  "0"^^xsd:nonNegativeInteger;
                                                                    owl:onProperty   core:versionTransitionMember
                                                                  ]
                                                                  [ rdf:type         owl:Restriction;
                                                                    owl:cardinality  "0"^^xsd:nonNegativeInteger;
                                                                    owl:onProperty   core:featureMember
                                                                  ]
                                                                )
                                          ]
                                          [ rdf:type            owl:Class;
                                            owl:intersectionOf  ( [ rdf:type         owl:Restriction;
                                                                    owl:cardinality  "0"^^xsd:nonNegativeInteger;
                                                                    owl:onProperty   core:cityObjectMember
                                                                  ]
                                                                  [ rdf:type                  owl:Restriction;
                                                                    owl:onClass               core:AbstractAppearance;
                                                                    owl:onProperty            core:appearanceMember;
                                                                    owl:qualifiedCardinality  "1"^^xsd:nonNegativeInteger
                                                                  ]
                                                                  [ rdf:type         owl:Restriction;
                                                                    owl:cardinality  "0"^^xsd:nonNegativeInteger;
                                                                    owl:onProperty   core:versionMember
                                                                  ]
                                                                  [ rdf:type         owl:Restriction;
                                                                    owl:cardinality  "0"^^xsd:nonNegativeInteger;
                                                                    owl:onProperty   core:versionTransitionMember
                                                                  ]
                                                                  [ rdf:type         owl:Restriction;
                                                                    owl:cardinality  "0"^^xsd:nonNegativeInteger;
                                                                    owl:onProperty   core:featureMember
                                                                  ]
                                                                )
                                          ]
                                          [ rdf:type            owl:Class;
                                            owl:intersectionOf  ( [ rdf:type         owl:Restriction;
                                                                    owl:cardinality  "0"^^xsd:nonNegativeInteger;
                                                                    owl:onProperty   core:cityObjectMember
                                                                  ]
                                                                  [ rdf:type         owl:Restriction;
                                                                    owl:cardinality  "0"^^xsd:nonNegativeInteger;
                                                                    owl:onProperty   core:appearanceMember
                                                                  ]
                                                                  [ rdf:type                  owl:Restriction;
                                                                    owl:onClass               core:AbstractVersion;
                                                                    owl:onProperty            core:versionMember;
                                                                    owl:qualifiedCardinality  "1"^^xsd:nonNegativeInteger
                                                                  ]
                                                                  [ rdf:type         owl:Restriction;
                                                                    owl:cardinality  "0"^^xsd:nonNegativeInteger;
                                                                    owl:onProperty   core:versionTransitionMember
                                                                  ]
                                                                  [ rdf:type         owl:Restriction;
                                                                    owl:cardinality  "0"^^xsd:nonNegativeInteger;
                                                                    owl:onProperty   core:featureMember
                                                                  ]
                                                                )
                                          ]
                                          [ rdf:type            owl:Class;
                                            owl:intersectionOf  ( [ rdf:type         owl:Restriction;
                                                                    owl:cardinality  "0"^^xsd:nonNegativeInteger;
                                                                    owl:onProperty   core:cityObjectMember
                                                                  ]
                                                                  [ rdf:type         owl:Restriction;
                                                                    owl:cardinality  "0"^^xsd:nonNegativeInteger;
                                                                    owl:onProperty   core:appearanceMember
                                                                  ]
                                                                  [ rdf:type         owl:Restriction;
                                                                    owl:cardinality  "0"^^xsd:nonNegativeInteger;
                                                                    owl:onProperty   core:versionMember
                                                                  ]
                                                                  [ rdf:type                  owl:Restriction;
                                                                    owl:onClass               core:AbstractVersionTransition;
                                                                    owl:onProperty            core:versionTransitionMember;
                                                                    owl:qualifiedCardinality  "1"^^xsd:nonNegativeInteger
                                                                  ]
                                                                  [ rdf:type         owl:Restriction;
                                                                    owl:cardinality  "0"^^xsd:nonNegativeInteger;
                                                                    owl:onProperty   core:featureMember
                                                                  ]
                                                                )
                                          ]
                                          [ rdf:type            owl:Class;
                                            owl:intersectionOf  ( [ rdf:type         owl:Restriction;
                                                                    owl:cardinality  "0"^^xsd:nonNegativeInteger;
                                                                    owl:onProperty   core:cityObjectMember
                                                                  ]
                                                                  [ rdf:type         owl:Restriction;
                                                                    owl:cardinality  "0"^^xsd:nonNegativeInteger;
                                                                    owl:onProperty   core:appearanceMember
                                                                  ]
                                                                  [ rdf:type         owl:Restriction;
                                                                    owl:cardinality  "0"^^xsd:nonNegativeInteger;
                                                                    owl:onProperty   core:versionMember
                                                                  ]
                                                                  [ rdf:type         owl:Restriction;
                                                                    owl:cardinality  "0"^^xsd:nonNegativeInteger;
                                                                    owl:onProperty   core:versionTransitionMember
                                                                  ]
                                                                  [ rdf:type                  owl:Restriction;
                                                                    owl:onClass               core:AbstractFeature;
                                                                    owl:onProperty            core:featureMember;
                                                                    owl:qualifiedCardinality  "1"^^xsd:nonNegativeInteger
                                                                  ]
                                                                )
                                          ]
                                        )
                         ];
        rdfs:subClassOf  [ rdf:type           owl:Restriction;
                           owl:allValuesFrom  core:AbstractFeature;
                           owl:onProperty     core:featureMember
                         ];
        rdfs:subClassOf  [ rdf:type           owl:Restriction;
                           owl:allValuesFrom  core:AbstractVersionTransition;
                           owl:onProperty     core:versionTransitionMember
                         ];
        rdfs:subClassOf  [ rdf:type           owl:Restriction;
                           owl:allValuesFrom  core:AbstractVersion;
                           owl:onProperty     core:versionMember
                         ];
        rdfs:subClassOf  [ rdf:type           owl:Restriction;
                           owl:allValuesFrom  core:AbstractAppearance;
                           owl:onProperty     core:appearanceMember
                         ];
        rdfs:subClassOf  [ rdf:type           owl:Restriction;
                           owl:allValuesFrom  core:AbstractCityObject;
                           owl:onProperty     core:cityObjectMember
                         ];
        skos:definition  "CityModelMember is a union type that enumerates the different types of objects that can occur as members of a city model."@en .

core:AbstractSpace.lod0Point
        rdf:type         owl:ObjectProperty;
        rdfs:domain      core:AbstractSpace;
        rdfs:label       "lod0Point"@en;
        rdfs:range       gmlowl:Point;
        skos:definition  "Relates to a 3D Point geometry that represents the space in Level of Detail 0."@en .

core:AbstractCityObject
        rdf:type               owl:Class;
        rdfs:label             "AbstractCityObject"@en;
        rdfs:subClassOf        core:AbstractFeatureWithLifespan;
        rdfs:subClassOf        [ rdf:type                     owl:Restriction;
                                 owl:maxQualifiedCardinality  "1"^^xsd:nonNegativeInteger;
                                 owl:onClass                  core:RelativeToTerrain;
                                 owl:onProperty               core:relativeToTerrain
                               ];
        rdfs:subClassOf        [ rdf:type           owl:Restriction;
                                 owl:allValuesFrom  core:ExternalReference;
                                 owl:onProperty     core:AbstractCityObject.externalReference
                               ];
        rdfs:subClassOf        [ rdf:type           owl:Restriction;
                                 owl:allValuesFrom  core:CityObjectRelation;
                                 owl:onProperty     core:AbstractCityObject.relatedTo
                               ];
        rdfs:subClassOf        [ rdf:type           owl:Restriction;
                                 owl:allValuesFrom  core:ADEOfAbstractCityObject;
                                 owl:onProperty     core:adeOfAbstractCityObject
                               ];
        rdfs:subClassOf        [ rdf:type           owl:Restriction;
                                 owl:allValuesFrom  core:AbstractAppearance;
                                 owl:onProperty     core:AbstractCityObject.appearance
                               ];
        rdfs:subClassOf        [ rdf:type           owl:Restriction;
                                 owl:allValuesFrom  core:AbstractDynamizer;
                                 owl:onProperty     core:AbstractCityObject.dynamizer
                               ];
        rdfs:subClassOf        [ rdf:type           owl:Restriction;
                                 owl:allValuesFrom  core:AbstractGenericAttribute;
                                 owl:onProperty     core:AbstractCityObject.genericAttribute
                               ];
        rdfs:subClassOf        [ rdf:type           owl:Restriction;
                                 owl:allValuesFrom  core:AbstractCityObject;
                                 owl:onProperty     core:AbstractCityObject.generalizesTo
                               ];
        rdfs:subClassOf        [ rdf:type           owl:Restriction;
                                 owl:allValuesFrom  core:RelativeToTerrain;
                                 owl:onProperty     core:relativeToTerrain
                               ];
        rdfs:subClassOf        [ rdf:type           owl:Restriction;
                                 owl:allValuesFrom  core:RelativeToWater;
                                 owl:onProperty     core:relativeToWater
                               ];
        rdfs:subClassOf        [ rdf:type                     owl:Restriction;
                                 owl:maxQualifiedCardinality  "1"^^xsd:nonNegativeInteger;
                                 owl:onClass                  core:RelativeToWater;
                                 owl:onProperty               core:relativeToWater
                               ];
        iso19150-2:isAbstract  true;
        skos:definition        "AbstractCityObject is the abstract superclass of all thematic classes within the CityGML Conceptual Model."@en .

core:SpaceType  rdf:type  rdfs:Datatype;
        rdfs:label       "SpaceType"@en;
        owl:oneOf        ( "closed" "open" "semiOpen" );
        skos:definition  "SpaceType is an enumeration that characterises a space according to its closure properties."@en .

core:appearanceMember
        rdf:type         owl:ObjectProperty;
        rdfs:label       "appearanceMember"@en;
        rdfs:range       core:AbstractAppearance;
        skos:definition  "Specifies the appearances of the CityModel."@en .

core:engineeringCRS  rdf:type  owl:ObjectProperty;
        rdfs:label       "engineeringCRS"@en;
        rdfs:range       iso19111-2019:EngineeringCRS;
        skos:definition  "Specifies the local engineering coordinate reference system of the CityModel that can be provided inline the CityModel instead of referencing a well-known CRS definition. The definition of an engineering CRS requires an anchor point which relates the origin of the local coordinate system to a point on the earth’s surface in order to facilitate the transformation of coordinates from the local engineering CRS."@en .

core:ADEOfAddress  rdf:type    owl:Class;
        rdfs:label             "ADEOfAddress"@en;
        iso19150-2:isAbstract  true;
        skos:definition        "ADEOfAddress acts as a hook to define properties within an ADE that are to be added to an Address."@en .

core:Address.multiPoint
        rdf:type         owl:ObjectProperty;
        rdfs:domain      core:Address;
        rdfs:label       "multiPoint"@en;
        rdfs:range       gmlowl:MultiPoint;
        skos:definition  "Relates to the MultiPoint geometry of the Address. The geometry relates the address spatially to a city object."@en .

core:ADEOfAbstractPointCloud
        rdf:type               owl:Class;
        rdfs:label             "ADEOfAbstractPointCloud"@en;
        iso19150-2:isAbstract  true;
        skos:definition        "ADEOfAbstractPointCloud acts as a hook to define properties within an ADE that are to be added to AbstractPointCloud."@en .

core:adeOfAbstractLogicalSpace
        rdf:type         owl:ObjectProperty;
        rdfs:label       "adeOfAbstractLogicalSpace"@en;
        rdfs:range       core:ADEOfAbstractLogicalSpace;
        skos:definition  "Augments AbstractLogicalSpace with properties defined in an ADE."@en .

core:value  rdf:type     owl:DatatypeProperty;
        rdfs:label       "value"@en;
        rdfs:range       xsd:double;
        skos:definition  "Specifies the double value."@en .

core:AbstractPhysicalSpace.lod2TerrainIntersectionCurve
        rdf:type         owl:ObjectProperty;
        rdfs:domain      core:AbstractPhysicalSpace;
        rdfs:label       "lod2TerrainIntersectionCurve"@en;
        rdfs:range       gmlowl:MultiCurve;
        skos:definition  "Relates to a 3D MultiCurve geometry that represents the terrain intersection curve of the physical space in Level of Detail 2."@en .

core:DoubleBetween0and1List
        rdf:type         owl:Class;
        rdfs:label       "DoubleBetween0and1List"@en;
        rdfs:subClassOf  [ rdf:type           owl:Restriction;
                           owl:allValuesFrom  xsd:double;
                           owl:onProperty     core:list
                         ];
        rdfs:subClassOf  [ rdf:type                  owl:Restriction;
                           owl:onClass               xsd:double;
                           owl:onProperty            core:list;
                           owl:qualifiedCardinality  "1"^^xsd:nonNegativeInteger
                         ];
        skos:definition  "DoubleBetween0and1List is a basic type that represents a list of double values greater or equal than 0 and less or equal than 1. The type is used for color encoding, for example."@en .

core:AbstractCityObject.genericAttribute
        rdf:type         owl:ObjectProperty;
        rdfs:domain      core:AbstractCityObject;
        rdfs:label       "genericAttribute"@en;
        rdfs:range       core:AbstractGenericAttribute;
        skos:definition  "Relates generic attributes to the city object."@en .

core:ADEOfAbstractSpaceBoundary
        rdf:type               owl:Class;
        rdfs:label             "ADEOfAbstractSpaceBoundary"@en;
        iso19150-2:isAbstract  true;
        skos:definition        "ADEOfAbstractSpaceBoundary acts as a hook to define properties within an ADE that are to be added to AbstractSpaceBoundary."@en .

core:AbstractThematicSurface.lod2MultiSurface
        rdf:type         owl:ObjectProperty;
        rdfs:domain      core:AbstractThematicSurface;
        rdfs:label       "lod2MultiSurface"@en;
        rdfs:range       gmlowl:MultiSurface;
        skos:definition  "Relates to a 3D MultiSurface geometry that represents the thematic surface in Level of Detail 2."@en .

core:adeOfAbstractVersionTransition
        rdf:type         owl:ObjectProperty;
        rdfs:label       "adeOfAbstractVersionTransition"@en;
        rdfs:range       core:ADEOfAbstractVersionTransition;
        skos:definition  "Augments AbstractVersionTransition with properties defined in an ADE."@en .

core:ADEOfAbstractSpace
        rdf:type               owl:Class;
        rdfs:label             "ADEOfAbstractSpace"@en;
        iso19150-2:isAbstract  true;
        skos:definition        "ADEOfAbstractSpace acts as a hook to define properties within an ADE that are to be added to AbstractSpace."@en .

core:terminationDate  rdf:type  owl:DatatypeProperty;
        rdfs:label       "terminationDate"@en;
        rdfs:range       xsd:dateTime;
        skos:definition  "Indicates the date at which a CityGML feature was removed from the CityModel."@en .

core:ImplicitGeometry.referencePoint
        rdf:type         owl:ObjectProperty;
        rdfs:domain      core:ImplicitGeometry;
        rdfs:label       "referencePoint"@en;
        rdfs:range       gmlowl:Point;
        skos:definition  "Relates to a 3D Point geometry that represents the base point of the object in the world coordinate system."@en .

core:list  rdf:type      owl:DatatypeProperty;
        rdfs:label       "list"@en;
        rdfs:range       xsd:double;
        skos:definition  "Specifies the list of double values."@en .

core:nilReasonEnumeration
        rdf:type         owl:ObjectProperty;
        rdfs:label       "nilReasonEnumeration"@en;
        rdfs:range       core:NilReasonEnumeration;
        skos:definition  "Indicates a nil reason that is provided in a code list."@en .

core:OtherRelationTypeValue
        rdf:type         owl:Class;
        rdfs:label       "OtherRelationTypeValue"@en;
        rdfs:subClassOf  skos:Concept;
        skos:definition  "OtherRelationTypeValue is a code list used to classify other types of city object relations."@en .

<https://www.opengis.net/ont/citygml/core>
        rdf:type         owl:Ontology;
        rdfs:label       "Core"@en;
        owl:imports      <https://www.opengis.net/ont/citygml/waterbody> , <https://www.opengis.net/ont/citygml/landuse> , <https://www.opengis.net/ont/citygml/tunnel> , <https://www.opengis.net/ont/citygml/bridge> , <https://www.opengis.net/ont/citygml/document> , <https://www.opengis.net/ont/citygml/cityobjectgroup> , <https://www.opengis.net/ont/citygml/vegetation> , <https://www.opengis.net/ont/citygml/relief> , <https://www.opengis.net/ont/citygml/appearance> , <http://www.opengis.net/ont/gml> , <http://def.isotc211.org/iso19150/-2/2012/base> , <https://www.opengis.net/ont/citygml/construction> , <https://www.opengis.net/ont/citygml/generics> , <https://www.opengis.net/ont/citygml/transportation> , <https://www.opengis.net/ont/citygml/workspace> , <https://www.opengis.net/ont/citygml/cityfurniture> , <https://www.opengis.net/ont/citygml/building> , <https://www.opengis.net/ont/citygml/dynamizer>;
        skos:definition  "The Core module defines the basic components of the CityGML conceptual model. This includes abstract base classes that define the core properties of more specialized thematic classes defined in other modules as well as concrete classes that are common to other modules, for example basic data types."@en .

[ rdf:type     owl:AllDisjointClasses;
  owl:members  ( frn:CityFurniture con:AbstractConstruction con:AbstractConstructiveElement con:AbstractFillingElement con:AbstractFurniture con:AbstractInstallation gen:GenericOccupiedSpace veg:AbstractVegetationObject wtr:WaterBody )
] .

core:AbstractFeatureWithLifespan
        rdf:type               owl:Class;
        rdfs:label             "AbstractFeatureWithLifespan"@en;
        rdfs:subClassOf        core:AbstractFeature;
        rdfs:subClassOf        [ rdf:type                     owl:Restriction;
                                 owl:maxQualifiedCardinality  "1"^^xsd:nonNegativeInteger;
                                 owl:onClass                  xsd:dateTime;
                                 owl:onProperty               core:creationDate
                               ];
        rdfs:subClassOf        [ rdf:type           owl:Restriction;
                                 owl:allValuesFrom  xsd:dateTime;
                                 owl:onProperty     core:creationDate
                               ];
        rdfs:subClassOf        [ rdf:type                     owl:Restriction;
                                 owl:maxQualifiedCardinality  "1"^^xsd:nonNegativeInteger;
                                 owl:onClass                  xsd:dateTime;
                                 owl:onProperty               core:terminationDate
                               ];
        rdfs:subClassOf        [ rdf:type                     owl:Restriction;
                                 owl:maxQualifiedCardinality  "1"^^xsd:nonNegativeInteger;
                                 owl:onClass                  xsd:dateTime;
                                 owl:onProperty               core:validFrom
                               ];
        rdfs:subClassOf        [ rdf:type           owl:Restriction;
                                 owl:allValuesFrom  xsd:dateTime;
                                 owl:onProperty     core:validTo
                               ];
        rdfs:subClassOf        [ rdf:type           owl:Restriction;
                                 owl:allValuesFrom  core:ADEOfAbstractFeatureWithLifespan;
                                 owl:onProperty     core:adeOfAbstractFeatureWithLifespan
                               ];
        rdfs:subClassOf        [ rdf:type           owl:Restriction;
                                 owl:allValuesFrom  xsd:dateTime;
                                 owl:onProperty     core:terminationDate
                               ];
        rdfs:subClassOf        [ rdf:type           owl:Restriction;
                                 owl:allValuesFrom  xsd:dateTime;
                                 owl:onProperty     core:validFrom
                               ];
        rdfs:subClassOf        [ rdf:type                     owl:Restriction;
                                 owl:maxQualifiedCardinality  "1"^^xsd:nonNegativeInteger;
                                 owl:onClass                  xsd:dateTime;
                                 owl:onProperty               core:validTo
                               ];
        iso19150-2:isAbstract  true;
        skos:definition        "AbstractFeatureWithLifespan is the base class for all CityGML features. This class allows the optional specification of the real-world and database times for the existence of each feature."@en .

core:ADEOfAbstractUnoccupiedSpace
        rdf:type               owl:Class;
        rdfs:label             "ADEOfAbstractUnoccupiedSpace"@en;
        iso19150-2:isAbstract  true;
        skos:definition        "ADEOfAbstractUnoccupiedSpace acts as a hook to define properties within an ADE that are to be added to AbstractUnoccupiedSpace."@en .

core:AbstractSpace.lod2MultiSurface
        rdf:type         owl:ObjectProperty;
        rdfs:domain      core:AbstractSpace;
        rdfs:label       "lod2MultiSurface"@en;
        rdfs:range       gmlowl:MultiSurface;
        skos:definition  "Relates to a 3D MultiSurface geometry that represents the space in Level of Detail 2."@en .

core:AbstractPhysicalSpace.lod1TerrainIntersectionCurve
        rdf:type         owl:ObjectProperty;
        rdfs:domain      core:AbstractPhysicalSpace;
        rdfs:label       "lod1TerrainIntersectionCurve"@en;
        rdfs:range       gmlowl:MultiCurve;
        skos:definition  "Relates to a 3D MultiCurve geometry that represents the terrain intersection curve of the physical space in Level of Detail 1."@en .

core:AbstractCityObject.relatedTo
        rdf:type         owl:ObjectProperty;
        rdfs:domain      core:AbstractCityObject;
        rdfs:label       "relatedTo"@en;
        rdfs:range       core:CityObjectRelation;
        skos:definition  "Relates other city objects to the city object. It also describes how the city objects are related to each other."@en .

core:QualifiedAreaTypeValue
        rdf:type         owl:Class;
        rdfs:label       "QualifiedAreaTypeValue"@en;
        rdfs:subClassOf  skos:Concept;
        skos:definition  "QualifiedAreaTypeValue is a code list used to specify area types."@en .

core:versionTransitionMember
        rdf:type         owl:ObjectProperty;
        rdfs:label       "versionTransitionMember"@en;
        rdfs:range       core:AbstractVersionTransition;
        skos:definition  "Specifies the transitions between the different versions of the CityModel."@en .

core:AbstractPhysicalSpace.lod3TerrainIntersectionCurve
        rdf:type         owl:ObjectProperty;
        rdfs:domain      core:AbstractPhysicalSpace;
        rdfs:label       "lod3TerrainIntersectionCurve"@en;
        rdfs:range       gmlowl:MultiCurve;
        skos:definition  "Relates to a 3D MultiCurve geometry that represents the terrain intersection curve of the physical space in Level of Detail 3."@en .

core:AbstractUnoccupiedSpace
        rdf:type               owl:Class;
        rdfs:label             "AbstractUnoccupiedSpace"@en;
        rdfs:subClassOf        core:AbstractPhysicalSpace;
        rdfs:subClassOf        [ rdf:type           owl:Restriction;
                                 owl:allValuesFrom  core:ADEOfAbstractUnoccupiedSpace;
                                 owl:onProperty     core:adeOfAbstractUnoccupiedSpace
                               ];
        iso19150-2:isAbstract  true;
        skos:definition        "AbstractUnoccupiedSpace is the abstract superclass for all types of physically unoccupied spaces. Unoccupied space refers to spaces that are entirely or mostly free of matter."@en .

core:OccupantTypeValue
        rdf:type         owl:Class;
        rdfs:label       "OccupantTypeValue"@en;
        rdfs:subClassOf  skos:Concept;
        skos:definition  "OccupantTypeValue is a code list used to classify occupants."@en .

core:AbstractSpace.lod3MultiCurve
        rdf:type         owl:ObjectProperty;
        rdfs:domain      core:AbstractSpace;
        rdfs:label       "lod3MultiCurve"@en;
        rdfs:range       gmlowl:MultiCurve;
        skos:definition  "Relates to a 3D MultiCurve geometry that represents the space in Level of Detail 3."@en .

[ rdf:type     owl:AllDisjointClasses;
  owl:members  ( bldg:AbstractBuildingSubdivision grp:CityObjectGroup gen:GenericLogicalSpace )
] .

core:versionMember  rdf:type  owl:ObjectProperty;
        rdfs:label       "versionMember"@en;
        rdfs:range       core:AbstractVersion;
        skos:definition  "Specifies the different versions of the CityModel."@en .

core:ADEOfAbstractLogicalSpace
        rdf:type               owl:Class;
        rdfs:label             "ADEOfAbstractLogicalSpace"@en;
        iso19150-2:isAbstract  true;
        skos:definition        "ADEOfAbstractLogicalSpace acts as a hook to define properties within an ADE that are to be added to AbstractLogicalSpace."@en .

core:featureID  rdf:type  owl:ObjectProperty;
        rdfs:label       "featureID"@en;
        rdfs:range       core:ID;
        skos:definition  "Specifies the unique identifier of the feature that is valid in the instance document within which it occurs."@en .

core:AbstractSpaceBoundary
        rdf:type               owl:Class;
        rdfs:label             "AbstractSpaceBoundary"@en;
        rdfs:subClassOf        core:AbstractCityObject;
        rdfs:subClassOf        [ rdf:type           owl:Restriction;
                                 owl:allValuesFrom  core:ADEOfAbstractSpaceBoundary;
                                 owl:onProperty     core:adeOfAbstractSpaceBoundary
                               ];
        iso19150-2:isAbstract  true;
        skos:definition        "AbstractSpaceBoundary is the abstract superclass for all types of space boundaries. A space boundary is an entity with areal extent in the real world. Space boundaries are objects that bound a Space. They also realize the contact between adjacent spaces."@en .

core:relativeToTerrain
        rdf:type         owl:ObjectProperty;
        rdfs:label       "relativeToTerrain"@en;
        rdfs:range       core:RelativeToTerrain;
        skos:definition  "Describes the vertical position of the city object relative to the surrounding terrain."@en .

core:AbstractFeature  rdf:type  owl:Class;
        rdfs:label             "AbstractFeature"@en;
        rdfs:subClassOf        iso19109:AnyFeature;
        rdfs:subClassOf        [ rdf:type                     owl:Restriction;
                                 owl:maxQualifiedCardinality  "1"^^xsd:nonNegativeInteger;
                                 owl:onClass                  rdfs:Resource;
                                 owl:onProperty               core:identifier
                               ];
        rdfs:subClassOf        [ rdf:type                  owl:Restriction;
                                 owl:onClass               core:ID;
                                 owl:onProperty            core:featureID;
                                 owl:qualifiedCardinality  "1"^^xsd:nonNegativeInteger
                               ];
        rdfs:subClassOf        [ rdf:type           owl:Restriction;
                                 owl:allValuesFrom  rdfs:Resource;
                                 owl:onProperty     core:identifier
                               ];
        rdfs:subClassOf        [ rdf:type           owl:Restriction;
                                 owl:allValuesFrom  core:ID;
                                 owl:onProperty     core:featureID
                               ];
        rdfs:subClassOf        [ rdf:type                     owl:Restriction;
                                 owl:maxQualifiedCardinality  "1"^^xsd:nonNegativeInteger;
                                 owl:onClass                  xsd:string;
                                 owl:onProperty               core:description
                               ];
        rdfs:subClassOf        [ rdf:type           owl:Restriction;
                                 owl:allValuesFrom  xsd:string;
                                 owl:onProperty     core:description
                               ];
        rdfs:subClassOf        [ rdf:type           owl:Restriction;
                                 owl:allValuesFrom  xsd:Name;
                                 owl:onProperty     core:name
                               ];
        rdfs:subClassOf        [ rdf:type           owl:Restriction;
                                 owl:allValuesFrom  core:ADEOfAbstractFeature;
                                 owl:onProperty     core:adeOfAbstractFeature
                               ];
        iso19150-2:isAbstract  true;
        skos:definition        "AbstractFeature is the abstract superclass of all feature types within the CityGML Conceptual Model."@en .

core:AbstractSpace  rdf:type   owl:Class;
        rdfs:label             "AbstractSpace"@en;
        rdfs:subClassOf        core:AbstractCityObject;
        rdfs:subClassOf        [ rdf:type           owl:Restriction;
                                 owl:allValuesFrom  gmlowl:MultiSurface;
                                 owl:onProperty     core:AbstractSpace.lod2MultiSurface
                               ];
        rdfs:subClassOf        [ rdf:type                     owl:Restriction;
                                 owl:maxQualifiedCardinality  "1"^^xsd:nonNegativeInteger;
                                 owl:onClass                  gmlowl:MultiCurve;
                                 owl:onProperty               core:AbstractSpace.lod2MultiCurve
                               ];
        rdfs:subClassOf        [ rdf:type           owl:Restriction;
                                 owl:allValuesFrom  gmlowl:Solid;
                                 owl:onProperty     core:AbstractSpace.lod3Solid
                               ];
        rdfs:subClassOf        [ rdf:type                     owl:Restriction;
                                 owl:maxQualifiedCardinality  "1"^^xsd:nonNegativeInteger;
                                 owl:onClass                  gmlowl:Solid;
                                 owl:onProperty               core:AbstractSpace.lod2Solid
                               ];
        rdfs:subClassOf        [ rdf:type           owl:Restriction;
                                 owl:allValuesFrom  gmlowl:Solid;
                                 owl:onProperty     core:AbstractSpace.lod1Solid
                               ];
        rdfs:subClassOf        [ rdf:type           owl:Restriction;
                                 owl:allValuesFrom  core:QualifiedVolume;
                                 owl:onProperty     core:volume
                               ];
        rdfs:subClassOf        [ rdf:type                     owl:Restriction;
                                 owl:maxQualifiedCardinality  "1"^^xsd:nonNegativeInteger;
                                 owl:onClass                  gmlowl:Point;
                                 owl:onProperty               core:AbstractSpace.lod0Point
                               ];
        rdfs:subClassOf        [ rdf:type           owl:Restriction;
                                 owl:allValuesFrom  gmlowl:MultiSurface;
                                 owl:onProperty     core:AbstractSpace.lod0MultiSurface
                               ];
        rdfs:subClassOf        [ rdf:type           owl:Restriction;
                                 owl:allValuesFrom  core:AbstractSpaceBoundary;
                                 owl:onProperty     core:AbstractSpace.boundary
                               ];
        rdfs:subClassOf        [ rdf:type           owl:Restriction;
                                 owl:allValuesFrom  gmlowl:MultiCurve;
                                 owl:onProperty     core:AbstractSpace.lod2MultiCurve
                               ];
        rdfs:subClassOf        [ rdf:type           owl:Restriction;
                                 owl:allValuesFrom  core:ADEOfAbstractSpace;
                                 owl:onProperty     core:adeOfAbstractSpace
                               ];
        rdfs:subClassOf        [ rdf:type                     owl:Restriction;
                                 owl:maxQualifiedCardinality  "1"^^xsd:nonNegativeInteger;
                                 owl:onClass                  gmlowl:MultiCurve;
                                 owl:onProperty               core:AbstractSpace.lod3MultiCurve
                               ];
        rdfs:subClassOf        [ rdf:type                     owl:Restriction;
                                 owl:maxQualifiedCardinality  "1"^^xsd:nonNegativeInteger;
                                 owl:onClass                  gmlowl:Solid;
                                 owl:onProperty               core:AbstractSpace.lod3Solid
                               ];
        rdfs:subClassOf        [ rdf:type           owl:Restriction;
                                 owl:allValuesFrom  gmlowl:Point;
                                 owl:onProperty     core:AbstractSpace.lod0Point
                               ];
        rdfs:subClassOf        [ rdf:type                     owl:Restriction;
                                 owl:maxQualifiedCardinality  "1"^^xsd:nonNegativeInteger;
                                 owl:onClass                  core:SpaceType;
                                 owl:onProperty               core:spaceType
                               ];
        rdfs:subClassOf        [ rdf:type                     owl:Restriction;
                                 owl:maxQualifiedCardinality  "1"^^xsd:nonNegativeInteger;
                                 owl:onClass                  gmlowl:MultiSurface;
                                 owl:onProperty               core:AbstractSpace.lod2MultiSurface
                               ];
        rdfs:subClassOf        [ rdf:type           owl:Restriction;
                                 owl:allValuesFrom  core:QualifiedArea;
                                 owl:onProperty     core:area
                               ];
        rdfs:subClassOf        [ rdf:type           owl:Restriction;
                                 owl:allValuesFrom  gmlowl:MultiCurve;
                                 owl:onProperty     core:AbstractSpace.lod3MultiCurve
                               ];
        rdfs:subClassOf        [ rdf:type                     owl:Restriction;
                                 owl:maxQualifiedCardinality  "1"^^xsd:nonNegativeInteger;
                                 owl:onClass                  gmlowl:MultiCurve;
                                 owl:onProperty               core:AbstractSpace.lod0MultiCurve
                               ];
        rdfs:subClassOf        [ rdf:type           owl:Restriction;
                                 owl:allValuesFrom  gmlowl:MultiCurve;
                                 owl:onProperty     core:AbstractSpace.lod0MultiCurve
                               ];
        rdfs:subClassOf        [ rdf:type           owl:Restriction;
                                 owl:allValuesFrom  gmlowl:Solid;
                                 owl:onProperty     core:AbstractSpace.lod2Solid
                               ];
        rdfs:subClassOf        [ rdf:type           owl:Restriction;
                                 owl:allValuesFrom  core:SpaceType;
                                 owl:onProperty     core:spaceType
                               ];
        rdfs:subClassOf        [ rdf:type           owl:Restriction;
                                 owl:allValuesFrom  gmlowl:MultiSurface;
                                 owl:onProperty     core:AbstractSpace.lod3MultiSurface
                               ];
        rdfs:subClassOf        [ rdf:type                     owl:Restriction;
                                 owl:maxQualifiedCardinality  "1"^^xsd:nonNegativeInteger;
                                 owl:onClass                  gmlowl:MultiSurface;
                                 owl:onProperty               core:AbstractSpace.lod0MultiSurface
                               ];
        rdfs:subClassOf        [ rdf:type                     owl:Restriction;
                                 owl:maxQualifiedCardinality  "1"^^xsd:nonNegativeInteger;
                                 owl:onClass                  gmlowl:Solid;
                                 owl:onProperty               core:AbstractSpace.lod1Solid
                               ];
        rdfs:subClassOf        [ rdf:type                     owl:Restriction;
                                 owl:maxQualifiedCardinality  "1"^^xsd:nonNegativeInteger;
                                 owl:onClass                  gmlowl:MultiSurface;
                                 owl:onProperty               core:AbstractSpace.lod3MultiSurface
                               ];
        iso19150-2:isAbstract  true;
        owl:disjointWith       core:AbstractSpaceBoundary;
        skos:definition        "AbstractSpace is the abstract superclass for all types of spaces. A space is an entity of volumetric extent in the real world."@en .

core:adeOfAbstractSpaceBoundary
        rdf:type         owl:ObjectProperty;
        rdfs:label       "adeOfAbstractSpaceBoundary"@en;
        rdfs:range       core:ADEOfAbstractSpaceBoundary;
        skos:definition  "Augments AbstractSpaceBoundary with properties defined in an ADE."@en .

core:AbstractThematicSurface.lod3MultiSurface
        rdf:type         owl:ObjectProperty;
        rdfs:domain      core:AbstractThematicSurface;
        rdfs:label       "lod3MultiSurface"@en;
        rdfs:range       gmlowl:MultiSurface;
        skos:definition  "Relates to a 3D MultiSurface geometry that represents the thematic surface in Level of Detail 3."@en .

[ rdf:type     owl:AllDisjointClasses;
  owl:members  ( core:AbstractThematicSurface dem:AbstractReliefComponent dem:ReliefFeature )
] .

core:AbstractOccupiedSpace.lod1ImplicitRepresentation
        rdf:type         owl:ObjectProperty;
        rdfs:domain      core:AbstractOccupiedSpace;
        rdfs:label       "lod1ImplicitRepresentation"@en;
        rdfs:range       core:ImplicitGeometry;
        skos:definition  "Relates to an implicit geometry that represents the occupied space in Level of Detail 1."@en .

core:TransformationMatrix4x4
        rdf:type         owl:Class;
        rdfs:label       "TransformationMatrix4x4"@en;
        rdfs:subClassOf  core:DoubleList;
        skos:definition  "TransformationMatrix4x4 is a 4 by 4 matrix represented as a list of sixteen double values in row major order."@en .

core:typeOfVolume  rdf:type  owl:ObjectProperty;
        rdfs:label       "typeOfVolume"@en;
        rdfs:range       core:QualifiedVolumeTypeValue;
        skos:definition  "Indicates the specific type of the QualifiedVolume."@en .

core:DoubleBetween0and1
        rdf:type         owl:Class;
        rdfs:label       "DoubleBetween0and1"@en;
        skos:definition  "DoubleBetween0and1 is a basic type for values, which are greater or equal than 0 and less or equal than 1. The type is used for color encoding, for example."@en .

[ rdf:type     owl:AllDisjointClasses;
  owl:members  ( app:AbstractSurfaceData core:AbstractFeatureWithLifespan core:AbstractPointCloud core:Address dyn:AbstractTimeseries )
] .

core:adeOfAbstractPointCloud
        rdf:type         owl:ObjectProperty;
        rdfs:label       "adeOfAbstractPointCloud"@en;
        rdfs:range       core:ADEOfAbstractPointCloud;
        skos:definition  "Augments AbstractPointCloud with properties defined in an ADE."@en .

[ rdf:type     owl:AllDisjointClasses;
  owl:members  ( con:AbstractConstructionSurface con:AbstractFillingSurface core:ClosureSurface gen:GenericThematicSurface luse:LandUse tran:AuxiliaryTrafficArea tran:HoleSurface tran:Marking tran:TrafficArea wtr:AbstractWaterBoundarySurface )
] .

core:ADEOfAbstractPhysicalSpace
        rdf:type               owl:Class;
        rdfs:label             "ADEOfAbstractPhysicalSpace"@en;
        iso19150-2:isAbstract  true;
        skos:definition        "ADEOfAbstractPhysicalSpace acts as a hook to define properties within an ADE that are to be added to AbstractPhysicalSpace."@en .

core:RelativeToTerrain
        rdf:type         rdfs:Datatype;
        rdfs:label       "RelativeToTerrain"@en;
        owl:oneOf        ( "entirelyAboveTerrain" "substantiallyAboveTerrain" "substantiallyAboveAndBelowTerrain" "substantiallyBelowTerrain" "entirelyBelowTerrain" );
        skos:definition  "RelativeToTerrain enumerates the spatial relations of a city object relative to terrain in a qualitative way."@en .

core:AbstractSpace.boundary
        rdf:type         owl:ObjectProperty;
        rdfs:domain      core:AbstractSpace;
        rdfs:label       "boundary"@en;
        rdfs:range       core:AbstractSpaceBoundary;
        skos:definition  "Relates to surfaces that bound the space."@en .

core:DoubleOrNilReason
        rdf:type         owl:Class;
        rdfs:label       "DoubleOrNilReason"@en;
        rdfs:subClassOf  [ rdf:type     owl:Class;
                           owl:unionOf  ( [ rdf:type            owl:Class;
                                            owl:intersectionOf  ( [ rdf:type                  owl:Restriction;
                                                                    owl:onClass               xsd:double;
                                                                    owl:onProperty            core:value;
                                                                    owl:qualifiedCardinality  "1"^^xsd:nonNegativeInteger
                                                                  ]
                                                                  [ rdf:type         owl:Restriction;
                                                                    owl:cardinality  "0"^^xsd:nonNegativeInteger;
                                                                    owl:onProperty   core:nilReason
                                                                  ]
                                                                )
                                          ]
                                          [ rdf:type            owl:Class;
                                            owl:intersectionOf  ( [ rdf:type         owl:Restriction;
                                                                    owl:cardinality  "0"^^xsd:nonNegativeInteger;
                                                                    owl:onProperty   core:value
                                                                  ]
                                                                  [ rdf:type                  owl:Restriction;
                                                                    owl:onClass               core:NilReason;
                                                                    owl:onProperty            core:nilReason;
                                                                    owl:qualifiedCardinality  "1"^^xsd:nonNegativeInteger
                                                                  ]
                                                                )
                                          ]
                                        )
                         ];
        rdfs:subClassOf  [ rdf:type           owl:Restriction;
                           owl:allValuesFrom  core:NilReason;
                           owl:onProperty     core:nilReason
                         ];
        rdfs:subClassOf  [ rdf:type           owl:Restriction;
                           owl:allValuesFrom  xsd:double;
                           owl:onProperty     core:value
                         ];
        skos:definition  "DoubleOrNilReason is a union type that allows for choosing between a double value and a nil reason."@en .

core:ADEOfAbstractAppearance
        rdf:type               owl:Class;
        rdfs:label             "ADEOfAbstractAppearance"@en;
        iso19150-2:isAbstract  true;
        skos:definition        "ADEOfAbstractAppearance acts as a hook to define properties within an ADE that are to be added to AbstractAppearance."@en .

core:AbstractCityObject.externalReference
        rdf:type         owl:ObjectProperty;
        rdfs:domain      core:AbstractCityObject;
        rdfs:label       "externalReference"@en;
        rdfs:range       core:ExternalReference;
        skos:definition  "References external objects in other information systems that have a relation to the city object."@en .

core:AbstractSpace.lod3MultiSurface
        rdf:type         owl:ObjectProperty;
        rdfs:domain      core:AbstractSpace;
        rdfs:label       "lod3MultiSurface"@en;
        rdfs:range       gmlowl:MultiSurface;
        skos:definition  "Relates to a 3D MultiSurface geometry that represents the space in Level of Detail 3."@en .

core:mimeType  rdf:type  owl:ObjectProperty;
        rdfs:label       "mimeType"@en;
        rdfs:range       core:MimeTypeValue;
        skos:definition  "Specifies the MIME type of the external file that stores the prototypical geometry."@en .

core:typeOfArea  rdf:type  owl:ObjectProperty;
        rdfs:label       "typeOfArea"@en;
        rdfs:range       core:QualifiedAreaTypeValue;
        skos:definition  "Indicates the specific type of the QualifiedArea."@en .

core:ImplicitGeometry.appearance
        rdf:type         owl:ObjectProperty;
        rdfs:domain      core:ImplicitGeometry;
        rdfs:label       "appearance"@en;
        rdfs:range       core:AbstractAppearance;
        skos:definition  "Relates appearances to the ImplicitGeometry."@en .

core:identifier  rdf:type  owl:ObjectProperty;
        rdfs:label       "identifier"@en;
        rdfs:range       rdfs:Resource;
        skos:definition  "Specifies the unique identifier of the feature that is valid globally."@en .

core:AbstractLogicalSpace
        rdf:type               owl:Class;
        rdfs:label             "AbstractLogicalSpace"@en;
        rdfs:subClassOf        core:AbstractSpace;
        rdfs:subClassOf        [ rdf:type           owl:Restriction;
                                 owl:allValuesFrom  core:ADEOfAbstractLogicalSpace;
                                 owl:onProperty     core:adeOfAbstractLogicalSpace
                               ];
        iso19150-2:isAbstract  true;
        owl:disjointWith       core:AbstractPhysicalSpace;
        skos:definition        "AbstractLogicalSpace is the abstract superclass for all types of logical spaces. Logical space refers to spaces that are not bounded by physical surfaces but are defined according to thematic considerations."@en .

core:IntervalValue  rdf:type  owl:Class;
        rdfs:label       "IntervalValue"@en;
        rdfs:subClassOf  skos:Concept;
        skos:definition  "IntervalValue is a code list used to specify a time period."@en .

core:adeOfAbstractFeatureWithLifespan
        rdf:type         owl:ObjectProperty;
        rdfs:label       "adeOfAbstractFeatureWithLifespan"@en;
        rdfs:range       core:ADEOfAbstractFeatureWithLifespan;
        skos:definition  "Augments AbstractFeatureWithLifespan with properties defined in an ADE."@en .

core:featureMember  rdf:type  owl:ObjectProperty;
        rdfs:label       "featureMember"@en;
        rdfs:range       core:AbstractFeature;
        skos:definition  "Specifies the feature objects that are part of the CityModel. It allows to include objects that are not derived from a class defined in the CityGML conceptual model, but from the ISO 19109 class AnyFeature."@en .

core:ADEOfAbstractCityObject
        rdf:type               owl:Class;
        rdfs:label             "ADEOfAbstractCityObject"@en;
        iso19150-2:isAbstract  true;
        skos:definition        "ADEOfAbstractCityObject acts as a hook to define properties within an ADE that are to be added to AbstractCityObject."@en .

core:AbstractCityObject.generalizesTo
        rdf:type         owl:ObjectProperty;
        rdfs:domain      core:AbstractCityObject;
        rdfs:label       "generalizesTo"@en;
        rdfs:range       core:AbstractCityObject;
        skos:definition  "Relates generalized representations of the same real-world object in different Levels of Detail to the city object. The direction of this relation is from the city object to the corresponding generalized city objects."@en .

core:ADEOfAbstractThematicSurface
        rdf:type               owl:Class;
        rdfs:label             "ADEOfAbstractThematicSurface"@en;
        iso19150-2:isAbstract  true;
        skos:definition        "ADEOfAbstractThematicSurface acts as a hook to define properties within an ADE that are to be added to AbstractThematicSurface."@en .

core:transformationMatrix
        rdf:type         owl:ObjectProperty;
        rdfs:label       "transformationMatrix"@en;
        rdfs:range       core:TransformationMatrix4x4;
        skos:definition  "Specifies the mathematical transformation (translation, rotation, and scaling) between the prototypical geometry and the actual spatial position of the object."@en .

core:QualifiedArea  rdf:type  owl:Class;
        rdfs:label       "QualifiedArea"@en;
        rdfs:subClassOf  [ rdf:type           owl:Restriction;
                           owl:allValuesFrom  core:QualifiedAreaTypeValue;
                           owl:onProperty     core:typeOfArea
                         ];
        rdfs:subClassOf  [ rdf:type                  owl:Restriction;
                           owl:onClass               core:QualifiedAreaTypeValue;
                           owl:onProperty            core:typeOfArea;
                           owl:qualifiedCardinality  "1"^^xsd:nonNegativeInteger
                         ];
        rdfs:subClassOf  [ rdf:type           owl:Restriction;
                           owl:allValuesFrom  core:QualifiedArea;
                           owl:onProperty     core:area
                         ];
        rdfs:subClassOf  [ rdf:type                  owl:Restriction;
                           owl:onClass               core:QualifiedArea;
                           owl:onProperty            core:area;
                           owl:qualifiedCardinality  "1"^^xsd:nonNegativeInteger
                         ];
        skos:definition  "QualifiedArea is an application-dependent measure of the area of a space or of a thematic surface."@en .

core:AbstractPhysicalSpace
        rdf:type               owl:Class;
        rdfs:label             "AbstractPhysicalSpace"@en;
        rdfs:subClassOf        core:AbstractSpace;
        rdfs:subClassOf        [ rdf:type           owl:Restriction;
                                 owl:allValuesFrom  gmlowl:MultiCurve;
                                 owl:onProperty     core:AbstractPhysicalSpace.lod1TerrainIntersectionCurve
                               ];
        rdfs:subClassOf        [ rdf:type           owl:Restriction;
                                 owl:allValuesFrom  core:ADEOfAbstractPhysicalSpace;
                                 owl:onProperty     core:adeOfAbstractPhysicalSpace
                               ];
        rdfs:subClassOf        [ rdf:type           owl:Restriction;
                                 owl:allValuesFrom  gmlowl:MultiCurve;
                                 owl:onProperty     core:AbstractPhysicalSpace.lod3TerrainIntersectionCurve
                               ];
        rdfs:subClassOf        [ rdf:type           owl:Restriction;
                                 owl:allValuesFrom  gmlowl:MultiCurve;
                                 owl:onProperty     core:AbstractPhysicalSpace.lod2TerrainIntersectionCurve
                               ];
        rdfs:subClassOf        [ rdf:type                     owl:Restriction;
                                 owl:maxQualifiedCardinality  "1"^^xsd:nonNegativeInteger;
                                 owl:onClass                  gmlowl:MultiCurve;
                                 owl:onProperty               core:AbstractPhysicalSpace.lod1TerrainIntersectionCurve
                               ];
        rdfs:subClassOf        [ rdf:type                     owl:Restriction;
                                 owl:maxQualifiedCardinality  "1"^^xsd:nonNegativeInteger;
                                 owl:onClass                  gmlowl:MultiCurve;
                                 owl:onProperty               core:AbstractPhysicalSpace.lod3TerrainIntersectionCurve
                               ];
        rdfs:subClassOf        [ rdf:type                     owl:Restriction;
                                 owl:maxQualifiedCardinality  "1"^^xsd:nonNegativeInteger;
                                 owl:onClass                  core:AbstractPointCloud;
                                 owl:onProperty               core:AbstractPhysicalSpace.pointCloud
                               ];
        rdfs:subClassOf        [ rdf:type                     owl:Restriction;
                                 owl:maxQualifiedCardinality  "1"^^xsd:nonNegativeInteger;
                                 owl:onClass                  gmlowl:MultiCurve;
                                 owl:onProperty               core:AbstractPhysicalSpace.lod2TerrainIntersectionCurve
                               ];
        rdfs:subClassOf        [ rdf:type           owl:Restriction;
                                 owl:allValuesFrom  core:AbstractPointCloud;
                                 owl:onProperty     core:AbstractPhysicalSpace.pointCloud
                               ];
        iso19150-2:isAbstract  true;
        skos:definition        "AbstractPhysicalSpace is the abstract superclass for all types of physical spaces. Physical space refers to spaces that are fully or partially bounded by physical objects."@en .

core:AbstractOccupiedSpace.lod2ImplicitRepresentation
        rdf:type         owl:ObjectProperty;
        rdfs:domain      core:AbstractOccupiedSpace;
        rdfs:label       "lod2ImplicitRepresentation"@en;
        rdfs:range       core:ImplicitGeometry;
        skos:definition  "Relates to an implicit geometry that represents the occupied space in Level of Detail 2."@en .

core:AbstractThematicSurface
        rdf:type               owl:Class;
        rdfs:label             "AbstractThematicSurface"@en;
        rdfs:subClassOf        core:AbstractSpaceBoundary;
        rdfs:subClassOf        [ rdf:type           owl:Restriction;
                                 owl:allValuesFrom  gmlowl:MultiSurface;
                                 owl:onProperty     core:AbstractThematicSurface.lod3MultiSurface
                               ];
        rdfs:subClassOf        [ rdf:type           owl:Restriction;
                                 owl:allValuesFrom  gmlowl:MultiSurface;
                                 owl:onProperty     core:AbstractThematicSurface.lod1MultiSurface
                               ];
        rdfs:subClassOf        [ rdf:type           owl:Restriction;
                                 owl:allValuesFrom  gmlowl:MultiCurve;
                                 owl:onProperty     core:AbstractThematicSurface.lod0MultiCurve
                               ];
        rdfs:subClassOf        [ rdf:type                     owl:Restriction;
                                 owl:maxQualifiedCardinality  "1"^^xsd:nonNegativeInteger;
                                 owl:onClass                  gmlowl:MultiCurve;
                                 owl:onProperty               core:AbstractThematicSurface.lod0MultiCurve
                               ];
        rdfs:subClassOf        [ rdf:type                     owl:Restriction;
                                 owl:maxQualifiedCardinality  "1"^^xsd:nonNegativeInteger;
                                 owl:onClass                  gmlowl:MultiSurface;
                                 owl:onProperty               core:AbstractThematicSurface.lod0MultiSurface
                               ];
        rdfs:subClassOf        [ rdf:type                     owl:Restriction;
                                 owl:maxQualifiedCardinality  "1"^^xsd:nonNegativeInteger;
                                 owl:onClass                  core:AbstractPointCloud;
                                 owl:onProperty               core:AbstractThematicSurface.pointCloud
                               ];
        rdfs:subClassOf        [ rdf:type           owl:Restriction;
                                 owl:allValuesFrom  gmlowl:MultiSurface;
                                 owl:onProperty     core:AbstractThematicSurface.lod2MultiSurface
                               ];
        rdfs:subClassOf        [ rdf:type           owl:Restriction;
                                 owl:allValuesFrom  core:AbstractPointCloud;
                                 owl:onProperty     core:AbstractThematicSurface.pointCloud
                               ];
        rdfs:subClassOf        [ rdf:type           owl:Restriction;
                                 owl:allValuesFrom  core:ADEOfAbstractThematicSurface;
                                 owl:onProperty     core:adeOfAbstractThematicSurface
                               ];
        rdfs:subClassOf        [ rdf:type                     owl:Restriction;
                                 owl:maxQualifiedCardinality  "1"^^xsd:nonNegativeInteger;
                                 owl:onClass                  gmlowl:MultiSurface;
                                 owl:onProperty               core:AbstractThematicSurface.lod2MultiSurface
                               ];
        rdfs:subClassOf        [ rdf:type                     owl:Restriction;
                                 owl:maxQualifiedCardinality  "1"^^xsd:nonNegativeInteger;
                                 owl:onClass                  gmlowl:MultiSurface;
                                 owl:onProperty               core:AbstractThematicSurface.lod1MultiSurface
                               ];
        rdfs:subClassOf        [ rdf:type           owl:Restriction;
                                 owl:allValuesFrom  gmlowl:MultiSurface;
                                 owl:onProperty     core:AbstractThematicSurface.lod0MultiSurface
                               ];
        rdfs:subClassOf        [ rdf:type                     owl:Restriction;
                                 owl:maxQualifiedCardinality  "1"^^xsd:nonNegativeInteger;
                                 owl:onClass                  gmlowl:MultiSurface;
                                 owl:onProperty               core:AbstractThematicSurface.lod3MultiSurface
                               ];
        rdfs:subClassOf        [ rdf:type           owl:Restriction;
                                 owl:allValuesFrom  core:QualifiedArea;
                                 owl:onProperty     core:area
                               ];
        iso19150-2:isAbstract  true;
        skos:definition        "AbstractThematicSurface is the abstract superclass for all types of thematic surfaces."@en .

core:relationType  rdf:type  owl:ObjectProperty;
        rdfs:label       "relationType"@en;
        rdfs:range       core:RelationTypeValue;
        skos:definition  "Indicates the specific type of the CityObjectRelation."@en .

core:AbstractSpace.lod3Solid
        rdf:type         owl:ObjectProperty;
        rdfs:domain      core:AbstractSpace;
        rdfs:label       "lod3Solid"@en;
        rdfs:range       gmlowl:Solid;
        skos:definition  "Relates to a 3D Solid geometry that represents the space in Level of Detail 3."@en .

core:adeOfAbstractPhysicalSpace
        rdf:type         owl:ObjectProperty;
        rdfs:label       "adeOfAbstractPhysicalSpace"@en;
        rdfs:range       core:ADEOfAbstractPhysicalSpace;
        skos:definition  "Augments AbstractPhysicalSpace with properties defined in an ADE."@en .

core:Occupancy  rdf:type  owl:Class;
        rdfs:label       "Occupancy"@en;
        rdfs:subClassOf  [ rdf:type           owl:Restriction;
                           owl:allValuesFrom  core:OccupantTypeValue;
                           owl:onProperty     core:occupantType
                         ];
        rdfs:subClassOf  [ rdf:type                     owl:Restriction;
                           owl:maxQualifiedCardinality  "1"^^xsd:nonNegativeInteger;
                           owl:onClass                  core:OccupantTypeValue;
                           owl:onProperty               core:occupantType
                         ];
        rdfs:subClassOf  [ rdf:type           owl:Restriction;
                           owl:allValuesFrom  core:IntervalValue;
                           owl:onProperty     core:interval
                         ];
        rdfs:subClassOf  [ rdf:type                     owl:Restriction;
                           owl:maxQualifiedCardinality  "1"^^xsd:nonNegativeInteger;
                           owl:onClass                  core:IntervalValue;
                           owl:onProperty               core:interval
                         ];
        rdfs:subClassOf  [ rdf:type           owl:Restriction;
                           owl:allValuesFrom  xsd:integer;
                           owl:onProperty     core:numberOfOccupants
                         ];
        rdfs:subClassOf  [ rdf:type                  owl:Restriction;
                           owl:onClass               xsd:integer;
                           owl:onProperty            core:numberOfOccupants;
                           owl:qualifiedCardinality  "1"^^xsd:nonNegativeInteger
                         ];
        skos:definition  "Occupancy is an application-dependent indication of what is contained by a feature."@en .

core:AbstractSpace.lod0MultiCurve
        rdf:type         owl:ObjectProperty;
        rdfs:domain      core:AbstractSpace;
        rdfs:label       "lod0MultiCurve"@en;
        rdfs:range       gmlowl:MultiCurve;
        skos:definition  "Relates to a 3D MultiCurve geometry that represents the space in Level of Detail 0."@en .

core:Address.xalAddress
        rdf:type         owl:ObjectProperty;
        rdfs:domain      core:Address;
        rdfs:label       "xalAddress"@en;
        rdfs:range       core:XALAddress;
        skos:definition  "Relates an OASIS address object to the Address."@en .

core:ExternalReference
        rdf:type         owl:Class;
        rdfs:label       "ExternalReference"@en;
        rdfs:subClassOf  [ rdf:type           owl:Restriction;
                           owl:allValuesFrom  core:RelationTypeValue;
                           owl:onProperty     core:relationType
                         ];
        rdfs:subClassOf  [ rdf:type                     owl:Restriction;
                           owl:maxQualifiedCardinality  "1"^^xsd:nonNegativeInteger;
                           owl:onClass                  core:RelationTypeValue;
                           owl:onProperty               core:relationType
                         ];
        rdfs:subClassOf  [ rdf:type           owl:Restriction;
                           owl:allValuesFrom  xsd:anyURI;
                           owl:onProperty     core:informationSystem
                         ];
        rdfs:subClassOf  [ rdf:type                     owl:Restriction;
                           owl:maxQualifiedCardinality  "1"^^xsd:nonNegativeInteger;
                           owl:onClass                  xsd:anyURI;
                           owl:onProperty               core:informationSystem
                         ];
        rdfs:subClassOf  [ rdf:type           owl:Restriction;
                           owl:allValuesFrom  xsd:anyURI;
                           owl:onProperty     core:targetResource
                         ];
        rdfs:subClassOf  [ rdf:type                  owl:Restriction;
                           owl:onClass               xsd:anyURI;
                           owl:onProperty            core:targetResource;
                           owl:qualifiedCardinality  "1"^^xsd:nonNegativeInteger
                         ];
        skos:definition  "ExternalReference is a reference to a corresponding object in another information system, for example in the German cadastre (ALKIS), the German topographic information system (ATKIS), or the OS UK MasterMap®."@en .

core:RelationTypeValue
        rdf:type         owl:Class;
        rdfs:label       "RelationTypeValue"@en;
        rdfs:subClassOf  skos:Concept;
        skos:definition  "RelationTypeValue is a code list used to classify city object relations."@en .

core:ClosureSurface  rdf:type  owl:Class;
        rdfs:label       "ClosureSurface"@en;
        rdfs:subClassOf  core:AbstractThematicSurface;
        rdfs:subClassOf  [ rdf:type           owl:Restriction;
                           owl:allValuesFrom  core:ADEOfClosureSurface;
                           owl:onProperty     core:adeOfClosureSurface
                         ];
        skos:definition  "ClosureSurface is a special type of thematic surface used to close holes in volumetric objects. Closure surfaces are virtual (non-physical) surfaces."@en .

core:ADEOfCityModel  rdf:type  owl:Class;
        rdfs:label             "ADEOfCityModel"@en;
        iso19150-2:isAbstract  true;
        skos:definition        "ADEOfCityModel acts as a hook to define properties within an ADE that are to be added to a CityModel."@en .

core:nilReason  rdf:type  owl:ObjectProperty;
        rdfs:label       "nilReason"@en;
        rdfs:range       core:NilReason;
        skos:definition  "Specifies the nil reason."@en .

core:TemporalRelationTypeValue
        rdf:type         owl:Class;
        rdfs:label       "TemporalRelationTypeValue"@en;
        rdfs:subClassOf  skos:Concept;
        skos:definition  "TemporalRelationTypeValue is a code list used to classify temporal city object relations."@en .

core:QualifiedVolumeTypeValue
        rdf:type         owl:Class;
        rdfs:label       "QualifiedVolumeTypeValue"@en;
        rdfs:subClassOf  skos:Concept;
        skos:definition  "QualifiedVolumeTypeValue is a code list used to specify volume types."@en .

core:NilReasonEnumeration
        rdf:type         owl:Class;
        rdfs:label       "NilReasonEnumeration"@en;
        rdfs:subClassOf  skos:Concept;
        skos:definition  "NilReasonEnumeration is a code list that enumerates the different nil reasons."@en .

core:ADEOfAbstractFeatureWithLifespan
        rdf:type               owl:Class;
        rdfs:label             "ADEOfAbstractFeatureWithLifespan"@en;
        iso19150-2:isAbstract  true;
        skos:definition        "ADEOfAbstractFeatureWithLifespan acts as a hook to define properties within an ADE that are to be added to AbstractFeatureWithLifespan."@en .

core:relativeToWater  rdf:type  owl:ObjectProperty;
        rdfs:label       "relativeToWater"@en;
        rdfs:range       core:RelativeToWater;
        skos:definition  "Describes the vertical position of the city object relative to the surrounding water surface."@en .

[ rdf:type     owl:AllDisjointClasses;
  owl:members  ( core:AbstractAppearance core:AbstractCityObject core:AbstractDynamizer core:AbstractVersion core:AbstractVersionTransition core:CityModel doc:Document wksp:Scenario wksp:Space wksp:Workspace )
] .

core:AbstractGenericAttribute
        rdf:type               owl:Class;
        rdfs:label             "AbstractGenericAttribute"@en;
        iso19150-2:isAbstract  true;
        skos:definition        "AbstractGenericAttribute is the abstract superclass for all types of generic attributes."@en .

core:AbstractSpace.lod2MultiCurve
        rdf:type         owl:ObjectProperty;
        rdfs:domain      core:AbstractSpace;
        rdfs:label       "lod2MultiCurve"@en;
        rdfs:range       gmlowl:MultiCurve;
        skos:definition  "Relates to a 3D MultiCurve geometry that represents the space in Level of Detail 2."@en .

core:AbstractVersionTransition
        rdf:type               owl:Class;
        rdfs:label             "AbstractVersionTransition"@en;
        rdfs:subClassOf        core:AbstractFeatureWithLifespan;
        rdfs:subClassOf        [ rdf:type           owl:Restriction;
                                 owl:allValuesFrom  core:ADEOfAbstractVersionTransition;
                                 owl:onProperty     core:adeOfAbstractVersionTransition
                               ];
        iso19150-2:isAbstract  true;
        skos:definition        "AbstractVersionTransition is the abstract superclass to represent VersionTransition objects."@en .

[ rdf:type     owl:AllDisjointClasses;
  owl:members  ( brid:BridgeRoom bldg:BuildingRoom gen:GenericUnoccupiedSpace tran:AbstractTransportationSpace tran:AuxiliaryTrafficSpace tran:ClearanceSpace tran:Hole tran:TrafficSpace tun:HollowSpace )
] .

core:Address  rdf:type   owl:Class;
        rdfs:label       "Address"@en;
        rdfs:subClassOf  core:AbstractFeature;
        rdfs:subClassOf  [ rdf:type           owl:Restriction;
                           owl:allValuesFrom  core:ADEOfAddress;
                           owl:onProperty     core:adeOfAddress
                         ];
        rdfs:subClassOf  [ rdf:type           owl:Restriction;
                           owl:allValuesFrom  gmlowl:MultiPoint;
                           owl:onProperty     core:Address.multiPoint
                         ];
        rdfs:subClassOf  [ rdf:type                     owl:Restriction;
                           owl:maxQualifiedCardinality  "1"^^xsd:nonNegativeInteger;
                           owl:onClass                  gmlowl:MultiPoint;
                           owl:onProperty               core:Address.multiPoint
                         ];
        rdfs:subClassOf  [ rdf:type           owl:Restriction;
                           owl:allValuesFrom  core:XALAddress;
                           owl:onProperty     core:Address.xalAddress
                         ];
        rdfs:subClassOf  [ rdf:type                  owl:Restriction;
                           owl:onClass               core:XALAddress;
                           owl:onProperty            core:Address.xalAddress;
                           owl:qualifiedCardinality  "1"^^xsd:nonNegativeInteger
                         ];
        skos:definition  "Address represents an address of a city object."@en .

core:libraryObject  rdf:type  owl:DatatypeProperty;
        rdfs:label       "libraryObject"@en;
        rdfs:range       xsd:anyURI;
        skos:definition  "Specifies the URI that points to the prototypical geometry stored in an external file."@en .

core:spaceType  rdf:type  owl:ObjectProperty;
        rdfs:label       "spaceType"@en;
        rdfs:range       core:SpaceType;
        skos:definition  "Specifies the degree of openness of a space."@en .

core:AbstractPointCloud
        rdf:type               owl:Class;
        rdfs:label             "AbstractPointCloud"@en;
        rdfs:subClassOf        core:AbstractFeature;
        rdfs:subClassOf        [ rdf:type           owl:Restriction;
                                 owl:allValuesFrom  core:ADEOfAbstractPointCloud;
                                 owl:onProperty     core:adeOfAbstractPointCloud
                               ];
        iso19150-2:isAbstract  true;
        skos:definition        "AbstractPointCloud is the abstract superclass to represent PointCloud objects."@en .

core:XALAddress  rdf:type  owl:Class;
        rdfs:label       "XALAddress"@en;
        skos:definition  "XALAddress represents address details according to the OASIS xAL standard."@en .

core:objectID  rdf:type  owl:ObjectProperty;
        rdfs:label       "objectID"@en;
        rdfs:range       core:ID;
        skos:definition  "Specifies the unique identifier of the ImplicitGeometry."@en .

core:AbstractPhysicalSpace.pointCloud
        rdf:type         owl:ObjectProperty;
        rdfs:domain      core:AbstractPhysicalSpace;
        rdfs:label       "pointCloud"@en;
        rdfs:range       core:AbstractPointCloud;
        skos:definition  "Relates to a 3D PointCloud that represents the physical space."@en .

core:interval  rdf:type  owl:ObjectProperty;
        rdfs:label       "interval"@en;
        rdfs:range       core:IntervalValue;
        skos:definition  "Indicates the time period the occupants are contained by a feature."@en .

core:IntegerBetween0and3
        rdf:type         owl:Class;
        rdfs:label       "IntegerBetween0and3"@en;
        skos:definition  "IntegerBetween0and3 is a basic type for integer values, which are greater or equal than 0 and less or equal than 3. The type is used for encoding the LOD number."@en .

core:uRI  rdf:type       owl:DatatypeProperty;
        rdfs:label       "URI"@en;
        rdfs:range       xsd:anyURI;
        skos:definition  "Specifies a URI that points to a resource that describes the nil reason."@en .

core:AbstractOccupiedSpace.lod3ImplicitRepresentation
        rdf:type         owl:ObjectProperty;
        rdfs:domain      core:AbstractOccupiedSpace;
        rdfs:label       "lod3ImplicitRepresentation"@en;
        rdfs:range       core:ImplicitGeometry;
        skos:definition  "Relates to an implicit geometry that represents the occupied space in Level of Detail 3."@en .

core:AbstractThematicSurface.pointCloud
        rdf:type         owl:ObjectProperty;
        rdfs:domain      core:AbstractThematicSurface;
        rdfs:label       "pointCloud"@en;
        rdfs:range       core:AbstractPointCloud;
        skos:definition  "Relates to a 3D PointCloud that represents the thematic surface."@en .

core:CityModel.cityModelMember
        rdf:type         owl:ObjectProperty;
        rdfs:domain      core:CityModel;
        rdfs:label       "cityModelMember"@en;
        rdfs:range       core:CityModelMember;
        skos:definition  "Relates to all objects that are part of the CityModel."@en .

core:creationDate  rdf:type  owl:DatatypeProperty;
        rdfs:label       "creationDate"@en;
        rdfs:range       xsd:dateTime;
        skos:definition  "Indicates the date at which a CityGML feature was added to the CityModel."@en .

[ rdf:type     owl:AllDisjointClasses;
  owl:members  ( core:TransformationMatrix2x2 core:TransformationMatrix3x4 core:TransformationMatrix4x4 )
] .

core:adeOfAbstractCityObject
        rdf:type         owl:ObjectProperty;
        rdfs:label       "adeOfAbstractCityObject"@en;
        rdfs:range       core:ADEOfAbstractCityObject;
        skos:definition  "Augments AbstractCityObject with properties defined in an ADE."@en .
