@prefix bldg: <https://www.opengis.net/ont/citygml/building/> .
@prefix brid: <https://www.opengis.net/ont/citygml/bridge/> .
@prefix con: <https://www.opengis.net/ont/citygml/construction/> .
@prefix concode: <https://www.opengis.net/ont/citygml/construction/code/> .
@prefix core: <https://www.opengis.net/ont/citygml/core/> .
@prefix dct: <http://purl.org/dc/terms/> .
@prefix gmlowl: <http://www.opengis.net/ont/gml#> .
@prefix iso19150-2: <http://def.isotc211.org/iso19150/-2/2012/base#> .
@prefix owl: <http://www.w3.org/2002/07/owl#> .
@prefix rdf: <http://www.w3.org/1999/02/22-rdf-syntax-ns#> .
@prefix rdfs: <http://www.w3.org/2000/01/rdf-schema#> .
@prefix sc: <http://shapechange.net/resources/ont/base#> .
@prefix skos: <http://www.w3.org/2004/02/skos/core#> .
@prefix tun: <https://www.opengis.net/ont/citygml/tunnel/> .
@prefix xsd: <http://www.w3.org/2001/XMLSchema#> .

<https://www.opengis.net/ont/citygml/construction> a owl:Ontology ;
    rdfs:label "Construction"@en ;
    owl:imports <http://def.isotc211.org/iso19150/-2/2012/base>,
        <http://shapechange.net/resources/ont/base>,
        <http://www.opengis.net/ont/gml>,
        <https://www.opengis.net/ont/citygml/bridge>,
        <https://www.opengis.net/ont/citygml/building>,
        <https://www.opengis.net/ont/citygml/core>,
        <https://www.opengis.net/ont/citygml/tunnel> ;
    skos:definition "The Construction module supports representation of key elements of different types of constructions. These key elements include construction surfaces (e.g floor and ceiling), windows and doors, constructive elements (e.g. beams and slabs), installations, and furniture."@en .

con:AbstractFurniture a owl:Class ;
    rdfs:label "AbstractFurniture"@en ;
    iso19150-2:isAbstract true ;
    rdfs:subClassOf [ a owl:Restriction ;
            owl:allValuesFrom con:ADEOfAbstractFurniture ;
            owl:onProperty con:adeOfAbstractFurniture ],
        core:AbstractOccupiedSpace ;
    skos:definition "AbstractFurniture is the abstract superclass for the representation of furniture objects of a construction."@en .

con:code a owl:Ontology .

concode:DoorClassValue a skos:ConceptScheme ;
    rdfs:label "DoorClassValue"@en ;
    dct:isFormatOf con:DoorClassValue ;
    skos:definition "DoorClassValue is a code list used to further classify a Door."@en .

concode:DoorFunctionValue a skos:ConceptScheme ;
    rdfs:label "DoorFunctionValue"@en ;
    dct:isFormatOf con:DoorFunctionValue ;
    skos:definition "DoorFunctionValue is a code list that enumerates the different purposes of a Door."@en .

concode:DoorUsageValue a skos:ConceptScheme ;
    rdfs:label "DoorUsageValue"@en ;
    dct:isFormatOf con:DoorUsageValue ;
    skos:definition "DoorUsageValue is a code list that enumerates the different uses of a Door."@en .

concode:ElevationReferenceValue a skos:ConceptScheme ;
    rdfs:label "ElevationReferenceValue"@en ;
    dct:isFormatOf con:ElevationReferenceValue ;
    skos:definition "ElevationReferenceValue is a code list that enumerates the different elevation reference levels used to measure construction heights."@en .

concode:EventValue a skos:ConceptScheme ;
    rdfs:label "EventValue"@en ;
    dct:isFormatOf con:EventValue ;
    skos:definition "EventValue is a code list that enumerates the different events of a construction."@en .

concode:OtherConstructionClassValue a skos:ConceptScheme ;
    rdfs:label "OtherConstructionClassValue"@en ;
    dct:isFormatOf con:OtherConstructionClassValue ;
    skos:definition "OtherConstructionClassValue is a code list used to further classify an OtherConstruction."@en .

concode:OtherConstructionFunctionValue a skos:ConceptScheme ;
    rdfs:label "OtherConstructionFunctionValue"@en ;
    dct:isFormatOf con:OtherConstructionFunctionValue ;
    skos:definition "OtherConstructionFunctionValue is a code list that enumerates the different purposes of an OtherConstruction."@en .

concode:OtherConstructionUsageValue a skos:ConceptScheme ;
    rdfs:label "OtherConstructionUsageValue"@en ;
    dct:isFormatOf con:OtherConstructionUsageValue ;
    skos:definition "OtherConstructionUsageValue is a code list that enumerates the different uses of an OtherConstruction."@en .

concode:WindowClassValue a skos:ConceptScheme ;
    rdfs:label "WindowClassValue"@en ;
    dct:isFormatOf con:WindowClassValue ;
    skos:definition "WindowClassValue is a code list used to further classify a Window."@en .

concode:WindowFunctionValue a skos:ConceptScheme ;
    rdfs:label "WindowFunctionValue"@en ;
    dct:isFormatOf con:WindowFunctionValue ;
    skos:definition "WindowFunctionValue is a code list that enumerates the different purposes of a Window."@en .

concode:WindowUsageValue a skos:ConceptScheme ;
    rdfs:label "WindowUsageValue"@en ;
    dct:isFormatOf con:WindowUsageValue ;
    skos:definition "WindowUsageValue is a code list that enumerates the different uses of a Window."@en .

con:AbstractConstruction.boundary a owl:ObjectProperty ;
    rdfs:label "boundary"@en ;
    rdfs:domain con:AbstractConstruction ;
    rdfs:range core:AbstractThematicSurface ;
    skos:definition "Relates to the surfaces that bound the construction. This relation is inherited from the Core module."@en .

con:AbstractConstructionSurface.fillingSurface a owl:ObjectProperty ;
    rdfs:label "fillingSurface"@en ;
    rdfs:domain con:AbstractConstructionSurface ;
    rdfs:range con:AbstractFillingSurface ;
    skos:definition "Relates to the surfaces that seal the openings of the construction surface."@en .

con:AbstractConstructiveElement.boundary a owl:ObjectProperty ;
    rdfs:label "boundary"@en ;
    rdfs:domain con:AbstractConstructiveElement ;
    rdfs:range core:AbstractThematicSurface ;
    skos:definition "Relates to the surfaces that bound the constructive element. This relation is inherited from the Core module."@en .

con:AbstractConstructiveElement.filling a owl:ObjectProperty ;
    rdfs:label "filling"@en ;
    rdfs:domain con:AbstractConstructiveElement ;
    rdfs:range con:AbstractFillingElement ;
    skos:definition "Relates to the elements that fill the opening of the constructive element."@en .

con:AbstractInstallation a owl:Class ;
    rdfs:label "AbstractInstallation"@en ;
    iso19150-2:isAbstract true ;
    rdfs:subClassOf [ a owl:Restriction ;
            owl:allValuesFrom con:ADEOfAbstractInstallation ;
            owl:onProperty con:adeOfAbstractInstallation ],
        [ a owl:Restriction ;
            owl:allValuesFrom core:AbstractThematicSurface ;
            owl:onProperty con:AbstractInstallation.boundary ],
        [ a owl:Restriction ;
            owl:allValuesFrom con:RelationToConstruction ;
            owl:onProperty con:relationToConstruction ],
        [ a owl:Restriction ;
            owl:maxQualifiedCardinality "1"^^xsd:nonNegativeInteger ;
            owl:onDataRange con:RelationToConstruction ;
            owl:onProperty con:relationToConstruction ],
        core:AbstractOccupiedSpace ;
    skos:definition "AbstractInstallation is the abstract superclass for the representation of installation objects of a construction."@en .

con:AbstractInstallation.boundary a owl:ObjectProperty ;
    rdfs:label "boundary"@en ;
    rdfs:domain con:AbstractInstallation ;
    rdfs:range core:AbstractThematicSurface ;
    skos:definition "Relates to the surfaces that bound the installation. This relation is inherited from the Core module."@en .

con:CeilingSurface a owl:Class ;
    rdfs:label "CeilingSurface"@en ;
    rdfs:subClassOf [ a owl:Restriction ;
            owl:allValuesFrom con:ADEOfCeilingSurface ;
            owl:onProperty con:adeOfCeilingSurface ],
        con:AbstractConstructionSurface ;
    skos:definition "A CeilingSurface is a surface that represents the interior ceiling of a construction. An example is the ceiling of a room."@en .

con:Door.address a owl:ObjectProperty ;
    rdfs:label "address"@en ;
    rdfs:domain con:Door ;
    rdfs:range core:Address ;
    skos:definition "Relates to the addresses that are assigned to the Door."@en .

con:Door.boundary a owl:ObjectProperty ;
    rdfs:label "boundary"@en ;
    rdfs:domain con:Door ;
    rdfs:range con:DoorSurface ;
    skos:definition "Relates to the door surfaces that bound the Door. This relation is inherited from the Core module."@en .

con:DoorSurface.address a owl:ObjectProperty ;
    rdfs:label "address"@en ;
    rdfs:domain con:DoorSurface ;
    rdfs:range core:Address ;
    skos:definition "Relates to the addresses that are assigned to the DoorSurface."@en .

con:FloorSurface a owl:Class ;
    rdfs:label "FloorSurface"@en ;
    rdfs:subClassOf [ a owl:Restriction ;
            owl:allValuesFrom con:ADEOfFloorSurface ;
            owl:onProperty con:adeOfFloorSurface ],
        con:AbstractConstructionSurface ;
    skos:definition "A FloorSurface is surface that represents the interior floor of a construction. An example is the floor of a room."@en .

con:GroundSurface a owl:Class ;
    rdfs:label "GroundSurface"@en ;
    rdfs:subClassOf [ a owl:Restriction ;
            owl:allValuesFrom con:ADEOfGroundSurface ;
            owl:onProperty con:adeOfGroundSurface ],
        con:AbstractConstructionSurface ;
    skos:definition "A GroundSurface is a surface that represents the ground plate of a construction. The polygon defining the ground plate is congruent with the footprint of the construction."@en .

con:InteriorWallSurface a owl:Class ;
    rdfs:label "InteriorWallSurface"@en ;
    rdfs:subClassOf [ a owl:Restriction ;
            owl:allValuesFrom con:ADEOfInteriorWallSurface ;
            owl:onProperty con:adeOfInteriorWallSurface ],
        con:AbstractConstructionSurface ;
    skos:definition "An InteriorWallSurface is a surface that is visible from inside a construction. An example is the wall of a room."@en .

con:OtherConstruction a owl:Class ;
    rdfs:label "OtherConstruction"@en ;
    rdfs:subClassOf [ a owl:Restriction ;
            owl:allValuesFrom con:ADEOfOtherConstruction ;
            owl:onProperty con:adeOfOtherConstruction ],
        [ a owl:Restriction ;
            owl:allValuesFrom con:DoorUsageValue ;
            owl:onProperty con:usage ],
        [ a owl:Restriction ;
            owl:allValuesFrom con:DoorFunctionValue ;
            owl:onProperty con:function ],
        [ a owl:Restriction ;
            owl:allValuesFrom con:DoorClassValue ;
            owl:onProperty con:class ],
        [ a owl:Restriction ;
            owl:maxQualifiedCardinality "1"^^xsd:nonNegativeInteger ;
            owl:onClass con:DoorClassValue ;
            owl:onProperty con:class ],
        con:AbstractConstruction ;
    skos:definition "An OtherConstruction is a construction that is not covered by any of the other subclasses of AbstractConstruction."@en .

con:OtherConstructionClassValue a owl:Class ;
    rdfs:label "OtherConstructionClassValue"@en ;
    rdfs:subClassOf skos:Concept ;
    skos:definition "OtherConstructionClassValue is a code list used to further classify an OtherConstruction."@en .

con:OtherConstructionFunctionValue a owl:Class ;
    rdfs:label "OtherConstructionFunctionValue"@en ;
    rdfs:subClassOf skos:Concept ;
    skos:definition "OtherConstructionFunctionValue is a code list that enumerates the different purposes of an OtherConstruction."@en .

con:OtherConstructionUsageValue a owl:Class ;
    rdfs:label "OtherConstructionUsageValue"@en ;
    rdfs:subClassOf skos:Concept ;
    skos:definition "OtherConstructionUsageValue is a code list that enumerates the different uses of an OtherConstruction."@en .

con:OuterCeilingSurface a owl:Class ;
    rdfs:label "OuterCeilingSurface"@en ;
    rdfs:subClassOf [ a owl:Restriction ;
            owl:allValuesFrom con:ADEOfOuterCeilingSurface ;
            owl:onProperty con:adeOfOuterCeilingSurface ],
        con:AbstractConstructionSurface ;
    skos:definition "An OuterCeilingSurface is a surface that belongs to the outer building shell with the orientation pointing downwards. An example is the ceiling of a loggia."@en .

con:OuterFloorSurface a owl:Class ;
    rdfs:label "OuterFloorSurface"@en ;
    rdfs:subClassOf [ a owl:Restriction ;
            owl:allValuesFrom con:ADEOfOuterFloorSurface ;
            owl:onProperty con:adeOfOuterFloorSurface ],
        con:AbstractConstructionSurface ;
    skos:definition "An OuterFloorSurface is a surface that belongs to the outer construction shell with the orientation pointing upwards. An example is the floor of a loggia."@en .

con:RoofSurface a owl:Class ;
    rdfs:label "RoofSurface"@en ;
    rdfs:subClassOf [ a owl:Restriction ;
            owl:allValuesFrom con:ADEOfRoofSurface ;
            owl:onProperty con:adeOfRoofSurface ],
        con:AbstractConstructionSurface ;
    skos:definition "A RoofSurface is a surface that delimits major roof parts of a construction."@en .

con:WallSurface a owl:Class ;
    rdfs:label "WallSurface"@en ;
    rdfs:subClassOf [ a owl:Restriction ;
            owl:allValuesFrom con:ADEOfWallSurface ;
            owl:onProperty con:adeOfWallSurface ],
        con:AbstractConstructionSurface ;
    skos:definition "A WallSurface is a surface that is part of the building facade visible from the outside."@en .

con:Window.boundary a owl:ObjectProperty ;
    rdfs:label "boundary"@en ;
    rdfs:domain con:Window ;
    rdfs:range con:WindowSurface ;
    skos:definition "Relates to the window surfaces that bound the Window. This relation is inherited from the Core module."@en .

con:WindowClassValue a owl:Class ;
    rdfs:label "WindowClassValue"@en ;
    rdfs:subClassOf skos:Concept ;
    skos:definition "WindowClassValue is a code list used to further classify a Window."@en .

con:WindowFunctionValue a owl:Class ;
    rdfs:label "WindowFunctionValue"@en ;
    rdfs:subClassOf skos:Concept ;
    skos:definition "WindowFunctionValue is a code list that enumerates the different purposes of a Window."@en .

con:WindowUsageValue a owl:Class ;
    rdfs:label "WindowUsageValue"@en ;
    rdfs:subClassOf skos:Concept ;
    skos:definition "WindowUsageValue is a code list that enumerates the different uses of a Window."@en .

con:adeOfAbstractConstruction a owl:ObjectProperty ;
    rdfs:label "adeOfAbstractConstruction"@en ;
    rdfs:range con:ADEOfAbstractConstruction ;
    skos:definition "Augments AbstractConstruction with properties defined in an ADE."@en .

con:adeOfAbstractConstructionSurface a owl:ObjectProperty ;
    rdfs:label "adeOfAbstractConstructionSurface"@en ;
    rdfs:range con:ADEOfAbstractConstructionSurface ;
    skos:definition "Augments AbstractConstructionSurface with properties defined in an ADE."@en .

con:adeOfAbstractConstructiveElement a owl:ObjectProperty ;
    rdfs:label "adeOfAbstractConstructiveElement"@en ;
    rdfs:range con:ADEOfAbstractConstructiveElement ;
    skos:definition "Augments AbstractConstructiveElement with properties defined in an ADE."@en .

con:adeOfAbstractFillingElement a owl:ObjectProperty ;
    rdfs:label "adeOfAbstractFillingElement"@en ;
    rdfs:range con:ADEOfAbstractFillingElement ;
    skos:definition "Augments AbstractFillingElement with properties defined in an ADE."@en .

con:adeOfAbstractFillingSurface a owl:ObjectProperty ;
    rdfs:label "adeOfAbstractFillingSurface"@en ;
    rdfs:range con:ADEOfAbstractFillingSurface ;
    skos:definition "Augments AbstractFillingSurface with properties defined in an ADE."@en .

con:adeOfAbstractFurniture a owl:ObjectProperty ;
    rdfs:label "adeOfAbstractFurniture"@en ;
    rdfs:range con:ADEOfAbstractFurniture ;
    skos:definition "Augments AbstractFurniture with properties defined in an ADE."@en .

con:adeOfAbstractInstallation a owl:ObjectProperty ;
    rdfs:label "adeOfAbstractInstallation"@en ;
    rdfs:range con:ADEOfAbstractInstallation ;
    skos:definition "Augments AbstractInstallation with properties defined in an ADE."@en .

con:adeOfCeilingSurface a owl:ObjectProperty ;
    rdfs:label "adeOfCeilingSurface"@en ;
    rdfs:range con:ADEOfCeilingSurface ;
    skos:definition "Augments the CeilingSurface with properties defined in an ADE."@en .

con:adeOfDoor a owl:ObjectProperty ;
    rdfs:label "adeOfDoor"@en ;
    rdfs:range con:ADEOfDoor ;
    skos:definition "Augments the Door with properties defined in an ADE."@en .

con:adeOfDoorSurface a owl:ObjectProperty ;
    rdfs:label "adeOfDoorSurface"@en ;
    rdfs:range con:ADEOfDoorSurface ;
    skos:definition "Augments the DoorSurface with properties defined in an ADE."@en .

con:adeOfFloorSurface a owl:ObjectProperty ;
    rdfs:label "adeOfFloorSurface"@en ;
    rdfs:range con:ADEOfFloorSurface ;
    skos:definition "Augments the FloorSurface with properties defined in an ADE."@en .

con:adeOfGroundSurface a owl:ObjectProperty ;
    rdfs:label "adeOfGroundSurface"@en ;
    rdfs:range con:ADEOfGroundSurface ;
    skos:definition "Augments the GroundSurface with properties defined in an ADE."@en .

con:adeOfInteriorWallSurface a owl:ObjectProperty ;
    rdfs:label "adeOfInteriorWallSurface"@en ;
    rdfs:range con:ADEOfInteriorWallSurface ;
    skos:definition "Augments the InteriorWallSurface with properties defined in an ADE."@en .

con:adeOfOtherConstruction a owl:ObjectProperty ;
    rdfs:label "adeOfOtherConstruction"@en ;
    rdfs:range con:ADEOfOtherConstruction ;
    skos:definition "Augments the OtherConstruction with properties defined in an ADE."@en .

con:adeOfOuterCeilingSurface a owl:ObjectProperty ;
    rdfs:label "adeOfOuterCeilingSurface"@en ;
    rdfs:range con:ADEOfOuterCeilingSurface ;
    skos:definition "Augments the OuterCeilingSurface with properties defined in an ADE."@en .

con:adeOfOuterFloorSurface a owl:ObjectProperty ;
    rdfs:label "adeOfOuterFloorSurface"@en ;
    rdfs:range con:ADEOfOuterFloorSurface ;
    skos:definition "Augments the OuterFloorSurface with properties defined in an ADE."@en .

con:adeOfRoofSurface a owl:ObjectProperty ;
    rdfs:label "adeOfRoofSurface"@en ;
    rdfs:range con:ADEOfRoofSurface ;
    skos:definition "Augments the RoofSurface with properties defined in an ADE."@en .

con:adeOfWallSurface a owl:ObjectProperty ;
    rdfs:label "adeOfWallSurface"@en ;
    rdfs:range con:ADEOfWallSurface ;
    skos:definition "Augments the WallSurface with properties defined in an ADE."@en .

con:adeOfWindow a owl:ObjectProperty ;
    rdfs:label "adeOfWindow"@en ;
    rdfs:range con:ADEOfWindow ;
    skos:definition "Augments the Window with properties defined in an ADE."@en .

con:adeOfWindowSurface a owl:ObjectProperty ;
    rdfs:label "adeOfWindowSurface"@en ;
    rdfs:range con:ADEOfWindowSurface ;
    skos:definition "Augments the WindowSurface with properties defined in an ADE."@en .

con:constructionEvent a owl:ObjectProperty ;
    rdfs:label "constructionEvent"@en ;
    rdfs:range con:ConstructionEvent ;
    skos:definition "Describes specific events in the life-time of the construction."@en .

con:elevation a owl:ObjectProperty ;
    rdfs:label "elevation"@en ;
    rdfs:range con:Elevation ;
    skos:definition "Specifies qualified elevations of the construction in relation to a well-defined surface which is commonly taken as origin (e.g. geoid or water level). [cf. INSPIRE]"@en .

con:height a owl:ObjectProperty ;
    rdfs:label "height"@en ;
    rdfs:range con:Height ;
    skos:definition "Specifies qualified heights of the construction above ground or below ground. [cf. INSPIRE]"@en .

con:occupancy a owl:ObjectProperty ;
    rdfs:label "occupancy"@en ;
    rdfs:range core:Occupancy ;
    skos:definition "Provides qualified information on the residency of persons, animals, or other moveable objects in the construction."@en .

con:ADEOfAbstractConstruction a owl:Class ;
    rdfs:label "ADEOfAbstractConstruction"@en ;
    iso19150-2:isAbstract true ;
    skos:definition "ADEOfAbstractConstruction acts as a hook to define properties within an ADE that are to be added to AbstractConstruction."@en .

con:ADEOfAbstractConstructionSurface a owl:Class ;
    rdfs:label "ADEOfAbstractConstructionSurface"@en ;
    iso19150-2:isAbstract true ;
    skos:definition "ADEOfAbstractConstructionSurface acts as a hook to define properties within an ADE that are to be added to AbstractConstructionSurface."@en .

con:ADEOfAbstractConstructiveElement a owl:Class ;
    rdfs:label "ADEOfAbstractConstructiveElement"@en ;
    iso19150-2:isAbstract true ;
    skos:definition "ADEOfAbstractConstructiveElement acts as a hook to define properties within an ADE that are to be added to AbstractConstructiveElement."@en .

con:ADEOfAbstractFillingElement a owl:Class ;
    rdfs:label "ADEOfAbstractFillingElement"@en ;
    iso19150-2:isAbstract true ;
    skos:definition "ADEOfAbstractFillingElement acts as a hook to define properties within an ADE that are to be added to AbstractFillingElement."@en .

con:ADEOfAbstractFillingSurface a owl:Class ;
    rdfs:label "ADEOfAbstractFillingSurface"@en ;
    iso19150-2:isAbstract true ;
    skos:definition "ADEOfAbstractFillingSurface acts as a hook to define properties within an ADE that are to be added to AbstractFillingSurface."@en .

con:ADEOfAbstractFurniture a owl:Class ;
    rdfs:label "ADEOfAbstractFurniture"@en ;
    iso19150-2:isAbstract true ;
    skos:definition "ADEOfAbstractFurniture acts as a hook to define properties within an ADE that are to be added to AbstractFurniture."@en .

con:ADEOfAbstractInstallation a owl:Class ;
    rdfs:label "ADEOfAbstractInstallation"@en ;
    iso19150-2:isAbstract true ;
    skos:definition "ADEOfAbstractInstallation acts as a hook to define properties within an ADE that are to be added to AbstractInstallation."@en .

con:ADEOfCeilingSurface a owl:Class ;
    rdfs:label "ADEOfCeilingSurface"@en ;
    iso19150-2:isAbstract true ;
    skos:definition "ADEOfCeilingSurface acts as a hook to define properties within an ADE that are to be added to a CeilingSurface."@en .

con:ADEOfDoor a owl:Class ;
    rdfs:label "ADEOfDoor"@en ;
    iso19150-2:isAbstract true ;
    skos:definition "ADEOfDoor acts as a hook to define properties within an ADE that are to be added to a Door."@en .

con:ADEOfDoorSurface a owl:Class ;
    rdfs:label "ADEOfDoorSurface"@en ;
    iso19150-2:isAbstract true ;
    skos:definition "ADEOfDoorSurface acts as a hook to define properties within an ADE that are to be added to a DoorSurface."@en .

con:ADEOfFloorSurface a owl:Class ;
    rdfs:label "ADEOfFloorSurface"@en ;
    iso19150-2:isAbstract true ;
    skos:definition "ADEOfFloorSurface acts as a hook to define properties within an ADE that are to be added to a FloorSurface."@en .

con:ADEOfGroundSurface a owl:Class ;
    rdfs:label "ADEOfGroundSurface"@en ;
    iso19150-2:isAbstract true ;
    skos:definition "ADEOfGroundSurface acts as a hook to define properties within an ADE that are to be added to a GroundSurface."@en .

con:ADEOfInteriorWallSurface a owl:Class ;
    rdfs:label "ADEOfInteriorWallSurface"@en ;
    iso19150-2:isAbstract true ;
    skos:definition "ADEOfInteriorWallSurface acts as a hook to define properties within an ADE that are to be added to an InteriorWallSurface."@en .

con:ADEOfOtherConstruction a owl:Class ;
    rdfs:label "ADEOfOtherConstruction"@en ;
    iso19150-2:isAbstract true ;
    skos:definition "ADEOfOtherConstruction acts as a hook to define properties within an ADE that are to be added to an OtherConstruction."@en .

con:ADEOfOuterCeilingSurface a owl:Class ;
    rdfs:label "ADEOfOuterCeilingSurface"@en ;
    iso19150-2:isAbstract true ;
    skos:definition "ADEOfOuterCeilingSurface acts as a hook to define properties within an ADE that are to be added to an OuterCeilingSurface."@en .

con:ADEOfOuterFloorSurface a owl:Class ;
    rdfs:label "ADEOfOuterFloorSurface"@en ;
    iso19150-2:isAbstract true ;
    skos:definition "ADEOfOuterFloorSurface acts as a hook to define properties within an ADE that are to be added to an OuterFloorSurface."@en .

con:ADEOfRoofSurface a owl:Class ;
    rdfs:label "ADEOfRoofSurface"@en ;
    iso19150-2:isAbstract true ;
    skos:definition "ADEOfRoofSurface acts as a hook to define properties within an ADE that are to be added to a RoofSurface."@en .

con:ADEOfWallSurface a owl:Class ;
    rdfs:label "ADEOfWallSurface"@en ;
    iso19150-2:isAbstract true ;
    skos:definition "ADEOfWallSurface acts as a hook to define properties within an ADE that are to be added to a WallSurface."@en .

con:ADEOfWindow a owl:Class ;
    rdfs:label "ADEOfWindow"@en ;
    iso19150-2:isAbstract true ;
    skos:definition "ADEOfWindow acts as a hook to define properties within an ADE that are to be added to a Window."@en .

con:ADEOfWindowSurface a owl:Class ;
    rdfs:label "ADEOfWindowSurface"@en ;
    iso19150-2:isAbstract true ;
    skos:definition "ADEOfWindowSurface acts as a hook to define properties within an ADE that are to be added to a WindowSurface."@en .

con:AbstractConstruction a owl:Class ;
    rdfs:label "AbstractConstruction"@en ;
    iso19150-2:isAbstract true ;
    rdfs:subClassOf [ a owl:Restriction ;
            owl:allValuesFrom con:Height ;
            owl:onProperty con:height ],
        [ a owl:Restriction ;
            owl:maxQualifiedCardinality "1"^^xsd:nonNegativeInteger ;
            owl:onDataRange xsd:date ;
            owl:onProperty con:dateOfDemolition ],
        [ a owl:Restriction ;
            owl:allValuesFrom con:ConditionOfConstructionValue ;
            owl:onProperty con:conditionOfConstruction ],
        [ a owl:Restriction ;
            owl:maxQualifiedCardinality "1"^^xsd:nonNegativeInteger ;
            owl:onDataRange con:ConditionOfConstructionValue ;
            owl:onProperty con:conditionOfConstruction ],
        [ a owl:Restriction ;
            owl:allValuesFrom con:Elevation ;
            owl:onProperty con:elevation ],
        [ a owl:Restriction ;
            owl:allValuesFrom core:Occupancy ;
            owl:onProperty con:occupancy ],
        [ a owl:Restriction ;
            owl:maxQualifiedCardinality "1"^^xsd:nonNegativeInteger ;
            owl:onDataRange xsd:date ;
            owl:onProperty con:dateOfConstruction ],
        [ a owl:Restriction ;
            owl:allValuesFrom core:AbstractThematicSurface ;
            owl:onProperty con:AbstractConstruction.boundary ],
        [ a owl:Restriction ;
            owl:allValuesFrom xsd:date ;
            owl:onProperty con:dateOfDemolition ],
        [ a owl:Restriction ;
            owl:allValuesFrom con:ADEOfAbstractConstruction ;
            owl:onProperty con:adeOfAbstractConstruction ],
        [ a owl:Restriction ;
            owl:allValuesFrom con:ConstructionEvent ;
            owl:onProperty con:constructionEvent ],
        [ a owl:Restriction ;
            owl:allValuesFrom xsd:date ;
            owl:onProperty con:dateOfConstruction ],
        core:AbstractOccupiedSpace ;
    skos:definition "AbstractConstruction is the abstract superclass for objects that are manufactured by humans from construction materials, are connected to earth, and are intended to be permanent. A connection with the ground also exists when the construction rests by its own weight on the ground or is moveable limited on stationary rails or if the construction  is intended to be used mainly stationary."@en .

con:AbstractConstructiveElement a owl:Class ;
    rdfs:label "AbstractConstructiveElement"@en ;
    iso19150-2:isAbstract true ;
    rdfs:subClassOf [ a owl:Restriction ;
            owl:allValuesFrom con:ADEOfAbstractConstructiveElement ;
            owl:onProperty con:adeOfAbstractConstructiveElement ],
        [ a owl:Restriction ;
            owl:allValuesFrom con:AbstractFillingElement ;
            owl:onProperty con:AbstractConstructiveElement.filling ],
        [ a owl:Restriction ;
            owl:allValuesFrom xsd:boolean ;
            owl:onProperty con:isStructuralElement ],
        [ a owl:Restriction ;
            owl:allValuesFrom core:AbstractThematicSurface ;
            owl:onProperty con:AbstractConstructiveElement.boundary ],
        [ a owl:Restriction ;
            owl:maxQualifiedCardinality "1"^^xsd:nonNegativeInteger ;
            owl:onDataRange xsd:boolean ;
            owl:onProperty con:isStructuralElement ],
        core:AbstractOccupiedSpace ;
    skos:definition "AbstractConstructiveElement is the abstract superclass for the representation of volumetric elements of a construction. Examples are walls, beams, slabs."@en .

con:ConstructionEvent a owl:Class ;
    rdfs:label "ConstructionEvent"@en ;
    rdfs:subClassOf [ a owl:Restriction ;
            owl:allValuesFrom xsd:string ;
            owl:onProperty con:description ],
        [ a owl:Restriction ;
            owl:maxQualifiedCardinality "1"^^xsd:nonNegativeInteger ;
            owl:onDataRange xsd:string ;
            owl:onProperty con:description ],
        [ a owl:Restriction ;
            owl:allValuesFrom xsd:date ;
            owl:onProperty con:dateOfEvent ],
        [ a owl:Restriction ;
            owl:onDataRange xsd:date ;
            owl:onProperty con:dateOfEvent ;
            owl:qualifiedCardinality "1"^^xsd:nonNegativeInteger ],
        [ a owl:Restriction ;
            owl:allValuesFrom con:EventValue ;
            owl:onProperty con:event ],
        [ a owl:Restriction ;
            owl:onClass con:EventValue ;
            owl:onProperty con:event ;
            owl:qualifiedCardinality "1"^^xsd:nonNegativeInteger ] ;
    skos:definition "A ConstructionEvent is a data type used to describe a specific event that is associated with a construction. Examples are the issuing of a building permit or the renovation of a building."@en .

con:Door a owl:Class ;
    rdfs:label "Door"@en ;
    rdfs:subClassOf [ a owl:Restriction ;
            owl:allValuesFrom con:DoorFunctionValue ;
            owl:onProperty con:function ],
        [ a owl:Restriction ;
            owl:allValuesFrom con:DoorSurface ;
            owl:onProperty con:Door.boundary ],
        [ a owl:Restriction ;
            owl:allValuesFrom con:ADEOfDoor ;
            owl:onProperty con:adeOfDoor ],
        [ a owl:Restriction ;
            owl:maxQualifiedCardinality "1"^^xsd:nonNegativeInteger ;
            owl:onClass con:DoorClassValue ;
            owl:onProperty con:class ],
        [ a owl:Restriction ;
            owl:allValuesFrom core:Address ;
            owl:onProperty con:Door.address ],
        [ a owl:Restriction ;
            owl:allValuesFrom con:DoorUsageValue ;
            owl:onProperty con:usage ],
        [ a owl:Restriction ;
            owl:allValuesFrom con:DoorClassValue ;
            owl:onProperty con:class ],
        con:AbstractFillingElement ;
    owl:disjointWith con:Window ;
    skos:definition "A Door is a construction for closing an opening intended primarily for access or egress or both. [cf. ISO 6707-1]"@en .

con:Elevation a owl:Class ;
    rdfs:label "Elevation"@en ;
    rdfs:subClassOf [ a owl:Restriction ;
            owl:allValuesFrom gmlowl:Point ;
            owl:onProperty con:elevationValue ],
        [ a owl:Restriction ;
            owl:onClass gmlowl:Point ;
            owl:onProperty con:elevationValue ;
            owl:qualifiedCardinality "1"^^xsd:nonNegativeInteger ],
        [ a owl:Restriction ;
            owl:allValuesFrom con:ElevationReferenceValue ;
            owl:onProperty con:elevationReference ],
        [ a owl:Restriction ;
            owl:onClass con:ElevationReferenceValue ;
            owl:onProperty con:elevationReference ;
            owl:qualifiedCardinality "1"^^xsd:nonNegativeInteger ] ;
    skos:definition "Elevation is a data type that includes the elevation value itself and information on how this elevation was measured. [cf. INSPIRE]"@en .

con:Height a owl:Class ;
    rdfs:label "Height"@en ;
    rdfs:subClassOf [ a owl:Restriction ;
            owl:allValuesFrom con:HeightStatusValue ;
            owl:onProperty con:status ],
        [ a owl:Restriction ;
            owl:allValuesFrom con:ElevationReferenceValue ;
            owl:onProperty con:lowReference ],
        [ a owl:Restriction ;
            owl:allValuesFrom con:ElevationReferenceValue ;
            owl:onProperty con:highReference ],
        [ a owl:Restriction ;
            owl:onDataRange sc:Measure ;
            owl:onProperty con:value ;
            owl:qualifiedCardinality "1"^^xsd:nonNegativeInteger ],
        [ a owl:Restriction ;
            owl:allValuesFrom sc:Measure ;
            owl:onProperty con:value ],
        [ a owl:Restriction ;
            owl:onClass con:ElevationReferenceValue ;
            owl:onProperty con:lowReference ;
            owl:qualifiedCardinality "1"^^xsd:nonNegativeInteger ],
        [ a owl:Restriction ;
            owl:onClass con:ElevationReferenceValue ;
            owl:onProperty con:highReference ;
            owl:qualifiedCardinality "1"^^xsd:nonNegativeInteger ],
        [ a owl:Restriction ;
            owl:onDataRange con:HeightStatusValue ;
            owl:onProperty con:status ;
            owl:qualifiedCardinality "1"^^xsd:nonNegativeInteger ] ;
    skos:definition "Height represents a vertical distance (measured or estimated) between a low reference and a high reference. [cf. INSPIRE]"@en .

con:Window a owl:Class ;
    rdfs:label "Window"@en ;
    rdfs:subClassOf [ a owl:Restriction ;
            owl:allValuesFrom con:DoorFunctionValue ;
            owl:onProperty con:function ],
        [ a owl:Restriction ;
            owl:allValuesFrom con:DoorClassValue ;
            owl:onProperty con:class ],
        [ a owl:Restriction ;
            owl:maxQualifiedCardinality "1"^^xsd:nonNegativeInteger ;
            owl:onClass con:DoorClassValue ;
            owl:onProperty con:class ],
        [ a owl:Restriction ;
            owl:allValuesFrom con:ADEOfWindow ;
            owl:onProperty con:adeOfWindow ],
        [ a owl:Restriction ;
            owl:allValuesFrom con:WindowSurface ;
            owl:onProperty con:Window.boundary ],
        [ a owl:Restriction ;
            owl:allValuesFrom con:DoorUsageValue ;
            owl:onProperty con:usage ],
        con:AbstractFillingElement ;
    skos:definition "A Window is a construction for closing an opening in a wall  or roof, primarily intended to admit light and/or provide ventilation. [cf. ISO  6707-1]"@en .

con:conditionOfConstruction a owl:DatatypeProperty ;
    rdfs:label "conditionOfConstruction"@en ;
    rdfs:range con:ConditionOfConstructionValue ;
    skos:definition "Indicates the life-cycle status of the construction. [cf. INSPIRE]"@en .

con:dateOfConstruction a owl:DatatypeProperty ;
    rdfs:label "dateOfConstruction"@en ;
    rdfs:range xsd:date ;
    skos:definition "Indicates the date at which the construction was completed."@en .

con:dateOfDemolition a owl:DatatypeProperty ;
    rdfs:label "dateOfDemolition"@en ;
    rdfs:range xsd:date ;
    skos:definition "Indicates the date at which the construction was demolished."@en .

con:dateOfEvent a owl:DatatypeProperty ;
    rdfs:label "dateOfEvent"@en ;
    rdfs:range xsd:date ;
    skos:definition "Specifies the date at which the event took or will take place."@en .

con:description a owl:DatatypeProperty ;
    rdfs:label "description"@en ;
    rdfs:range xsd:string ;
    skos:definition "Provides additional information on the event."@en .

con:elevationReference a owl:ObjectProperty ;
    rdfs:label "elevationReference"@en ;
    rdfs:range con:ElevationReferenceValue ;
    skos:definition "Specifies the level from which the elevation was measured. [cf. INSPIRE]"@en .

con:elevationValue a owl:ObjectProperty ;
    rdfs:label "elevationValue"@en ;
    rdfs:range gmlowl:Point ;
    skos:definition "Specifies the value of the elevation. [cf. INSPIRE]"@en .

con:event a owl:ObjectProperty ;
    rdfs:label "event"@en ;
    rdfs:range con:EventValue ;
    skos:definition "Indicates the specific event type."@en .

con:highReference a owl:ObjectProperty ;
    rdfs:label "highReference"@en ;
    rdfs:range con:ElevationReferenceValue ;
    skos:definition "Indicates the high point used to calculate the value of the height. [cf. INSPIRE]"@en .

con:isStructuralElement a owl:DatatypeProperty ;
    rdfs:label "isStructuralElement"@en ;
    rdfs:range xsd:boolean ;
    skos:definition "Indicates whether the constructive element is essential from a structural point of view. A structural element cannot be omitted without collapsing of the construction. Examples are pylons and anchorages of bridges."@en .

con:lowReference a owl:ObjectProperty ;
    rdfs:label "lowReference"@en ;
    rdfs:range con:ElevationReferenceValue ;
    skos:definition "Indicates the low point used to calculate the value of the height. [cf. INSPIRE]"@en .

con:relationToConstruction a owl:DatatypeProperty ;
    rdfs:label "relationToConstruction"@en ;
    rdfs:range con:RelationToConstruction ;
    skos:definition "Indicates whether the installation is located inside and/or outside of the construction."@en .

con:status a owl:DatatypeProperty ;
    rdfs:label "status"@en ;
    rdfs:range con:HeightStatusValue ;
    skos:definition "Indicates the way the height has been captured. [cf. INSPIRE]"@en .

con:value a owl:DatatypeProperty ;
    rdfs:label "value"@en ;
    rdfs:range sc:Measure ;
    skos:definition "Specifies the value of the height above or below ground. [cf. INSPIRE]"@en .

con:ConditionOfConstructionValue a rdfs:Datatype ;
    rdfs:label "ConditionOfConstructionValue"@en ;
    owl:equivalentClass [ a rdfs:Datatype ;
            owl:oneOf ( "declined" "demolished" "functional" "projected" "ruin" "underConstruction" ) ] ;
    skos:definition "ConditionOfConstructionValue enumerates different conditions of a construction. [cf. INSPIRE]"@en .

con:DoorSurface a owl:Class ;
    rdfs:label "DoorSurface"@en ;
    rdfs:subClassOf [ a owl:Restriction ;
            owl:allValuesFrom con:ADEOfDoorSurface ;
            owl:onProperty con:adeOfDoorSurface ],
        [ a owl:Restriction ;
            owl:allValuesFrom core:Address ;
            owl:onProperty con:DoorSurface.address ],
        con:AbstractFillingSurface ;
    owl:disjointWith con:WindowSurface ;
    skos:definition "A DoorSurface is either a boundary surface of a Door feature or a surface that seals an opening filled by a door."@en .

con:HeightStatusValue a rdfs:Datatype ;
    rdfs:label "HeightStatusValue"@en ;
    owl:equivalentClass [ a rdfs:Datatype ;
            owl:oneOf ( "estimated" "measured" ) ] ;
    skos:definition "HeightStatusValue enumerates the different methods used to capture a height. [cf. INSPIRE]"@en .

con:RelationToConstruction a rdfs:Datatype ;
    rdfs:label "RelationToConstruction"@en ;
    owl:equivalentClass [ a rdfs:Datatype ;
            owl:oneOf ( "inside" "outside" "bothInsideAndOutside" ) ] ;
    skos:definition "RelationToConstruction is an enumeration used to describe whether an installation is positioned inside and/or outside of a construction."@en .

con:WindowSurface a owl:Class ;
    rdfs:label "WindowSurface"@en ;
    rdfs:subClassOf [ a owl:Restriction ;
            owl:allValuesFrom con:ADEOfWindowSurface ;
            owl:onProperty con:adeOfWindowSurface ],
        con:AbstractFillingSurface ;
    skos:definition "A WindowSurface is either a boundary surface of a Window feature or a surface that seals an opening filled by a window."@en .

con:function a owl:ObjectProperty ;
    rdfs:label "function"@en ;
    rdfs:range con:DoorFunctionValue ;
    skos:definition "Specifies the intended purposes of the Door."@en .

con:usage a owl:ObjectProperty ;
    rdfs:label "usage"@en ;
    rdfs:range con:DoorUsageValue ;
    skos:definition "Specifies the actual uses of the Door."@en .

con:AbstractFillingElement a owl:Class ;
    rdfs:label "AbstractFillingElement"@en ;
    iso19150-2:isAbstract true ;
    rdfs:subClassOf [ a owl:Restriction ;
            owl:allValuesFrom con:ADEOfAbstractFillingElement ;
            owl:onProperty con:adeOfAbstractFillingElement ],
        core:AbstractOccupiedSpace ;
    skos:definition "AbstractFillingElement is the abstract superclass for different kinds of elements that fill the openings of a construction."@en .

con:AbstractFillingSurface a owl:Class ;
    rdfs:label "AbstractFillingSurface"@en ;
    iso19150-2:isAbstract true ;
    rdfs:subClassOf [ a owl:Restriction ;
            owl:allValuesFrom con:ADEOfAbstractFillingSurface ;
            owl:onProperty con:adeOfAbstractFillingSurface ],
        core:AbstractThematicSurface ;
    skos:definition "AbstractFillingSurface is the abstract superclass for different kinds of surfaces that seal openings filled by filling elements."@en .

con:EventValue a owl:Class ;
    rdfs:label "EventValue"@en ;
    rdfs:subClassOf skos:Concept ;
    skos:definition "EventValue is a code list that enumerates the different events of a construction."@en .

con:DoorFunctionValue a owl:Class ;
    rdfs:label "DoorFunctionValue"@en ;
    rdfs:subClassOf skos:Concept ;
    skos:definition "DoorFunctionValue is a code list that enumerates the different purposes of a Door."@en .

con:DoorUsageValue a owl:Class ;
    rdfs:label "DoorUsageValue"@en ;
    rdfs:subClassOf skos:Concept ;
    skos:definition "DoorUsageValue is a code list that enumerates the different uses of a Door."@en .

con:class a owl:ObjectProperty ;
    rdfs:label "class"@en ;
    rdfs:range con:DoorClassValue ;
    skos:definition "Indicates the specific type of the Door."@en .

con:DoorClassValue a owl:Class ;
    rdfs:label "DoorClassValue"@en ;
    rdfs:subClassOf skos:Concept ;
    skos:definition "DoorClassValue is a code list used to further classify a Door."@en .

con:AbstractConstructionSurface a owl:Class ;
    rdfs:label "AbstractConstructionSurface"@en ;
    iso19150-2:isAbstract true ;
    rdfs:subClassOf [ a owl:Restriction ;
            owl:allValuesFrom con:ADEOfAbstractConstructionSurface ;
            owl:onProperty con:adeOfAbstractConstructionSurface ],
        [ a owl:Restriction ;
            owl:allValuesFrom con:AbstractFillingSurface ;
            owl:onProperty con:AbstractConstructionSurface.fillingSurface ],
        core:AbstractThematicSurface ;
    skos:definition "AbstractConstructionSurface is the abstract superclass for different kinds of surfaces that bound a construction."@en .

con:ElevationReferenceValue a owl:Class ;
    rdfs:label "ElevationReferenceValue"@en ;
    rdfs:subClassOf skos:Concept ;
    skos:definition "ElevationReferenceValue is a code list that enumerates the different elevation reference levels used to measure construction heights."@en .

[] a owl:AllDisjointClasses ;
    owl:members ( brid:BridgeFurniture bldg:BuildingFurniture tun:TunnelFurniture ) .

[] a owl:AllDisjointClasses ;
    owl:members ( brid:BridgeInstallation bldg:BuildingInstallation tun:TunnelInstallation ) .

[] a owl:AllDisjointClasses ;
    owl:members ( brid:AbstractBridge bldg:AbstractBuilding con:OtherConstruction tun:AbstractTunnel ) .

[] a owl:AllDisjointClasses ;
    owl:members ( con:CeilingSurface con:FloorSurface con:GroundSurface con:InteriorWallSurface con:OuterCeilingSurface con:OuterFloorSurface con:RoofSurface con:WallSurface ) .

[] a owl:AllDisjointClasses ;
    owl:members ( brid:BridgeConstructiveElement bldg:BuildingConstructiveElement tun:TunnelConstructiveElement ) .

