@prefix con:        <https://www.opengis.net/ont/citygml/construction/> .
@prefix core:       <https://www.opengis.net/ont/citygml/core/> .
@prefix iso19150-2: <http://def.isotc211.org/iso19150/-2/2012/base#> .
@prefix owl:        <http://www.w3.org/2002/07/owl#> .
@prefix rdf:        <http://www.w3.org/1999/02/22-rdf-syntax-ns#> .
@prefix rdfs:       <http://www.w3.org/2000/01/rdf-schema#> .
@prefix skos:       <http://www.w3.org/2004/02/skos/core#> .
@prefix tun:        <https://www.opengis.net/ont/citygml/tunnel/> .
@prefix xsd:        <http://www.w3.org/2001/XMLSchema#> .

tun:ADEOfTunnelPart  rdf:type  owl:Class;
        rdfs:label             "ADEOfTunnelPart"@en;
        iso19150-2:isAbstract  true;
        skos:definition        "ADEOfTunnelPart acts as a hook to define properties within an ADE that are to be added to a TunnelPart."@en .

tun:TunnelUsageValue  rdf:type  owl:Class;
        rdfs:label       "TunnelUsageValue"@en;
        rdfs:subClassOf  skos:Concept;
        skos:definition  "TunnelUsageValue is a code list that enumerates the different uses of a Tunnel."@en .

tun:HollowSpace  rdf:type  owl:Class;
        rdfs:label       "HollowSpace"@en;
        rdfs:subClassOf  core:AbstractUnoccupiedSpace;
        rdfs:subClassOf  [ rdf:type           owl:Restriction;
                           owl:allValuesFrom  tun:HollowSpaceFunctionValue;
                           owl:onProperty     tun:HollowSpace.function
                         ];
        rdfs:subClassOf  [ rdf:type                     owl:Restriction;
                           owl:maxQualifiedCardinality  "1"^^xsd:nonNegativeInteger;
                           owl:onClass                  tun:HollowSpaceClassValue;
                           owl:onProperty               tun:HollowSpace.class
                         ];
        rdfs:subClassOf  [ rdf:type           owl:Restriction;
                           owl:allValuesFrom  tun:TunnelInstallation;
                           owl:onProperty     tun:HollowSpace.tunnelInstallation
                         ];
        rdfs:subClassOf  [ rdf:type           owl:Restriction;
                           owl:allValuesFrom  tun:ADEOfHollowSpace;
                           owl:onProperty     tun:adeOfHollowSpace
                         ];
        rdfs:subClassOf  [ rdf:type           owl:Restriction;
                           owl:allValuesFrom  tun:HollowSpaceUsageValue;
                           owl:onProperty     tun:HollowSpace.usage
                         ];
        rdfs:subClassOf  [ rdf:type           owl:Restriction;
                           owl:allValuesFrom  core:AbstractThematicSurface;
                           owl:onProperty     tun:boundary
                         ];
        rdfs:subClassOf  [ rdf:type           owl:Restriction;
                           owl:allValuesFrom  tun:TunnelFurniture;
                           owl:onProperty     tun:HollowSpace.tunnelFurniture
                         ];
        rdfs:subClassOf  [ rdf:type           owl:Restriction;
                           owl:allValuesFrom  tun:HollowSpaceClassValue;
                           owl:onProperty     tun:HollowSpace.class
                         ];
        skos:definition  "A HollowSpace is a space within a Tunnel or TunnelPart intended for certain functions (e.g. transport or passage ways, service rooms, emergency shelters). A HollowSpace is bounded physically and/or virtually (e.g. by ClosureSurfaces or GenericSurfaces)."@en .

tun:ADEOfTunnelConstructiveElement
        rdf:type               owl:Class;
        rdfs:label             "ADEOfTunnelConstructiveElement"@en;
        iso19150-2:isAbstract  true;
        skos:definition        "ADEOfTunnelConstructiveElement acts as a hook to define properties within an ADE that are to be added to a TunnelConstructiveElement."@en .

tun:TunnelFurniture.class
        rdf:type         owl:ObjectProperty;
        rdfs:domain      tun:TunnelFurniture;
        rdfs:label       "class"@en;
        rdfs:range       tun:TunnelFurnitureClassValue;
        skos:definition  "Indicates the specific type of the TunnelFurniture."@en .

tun:AbstractTunnel.class
        rdf:type         owl:ObjectProperty;
        rdfs:domain      tun:AbstractTunnel;
        rdfs:label       "class"@en;
        rdfs:range       tun:TunnelClassValue;
        skos:definition  "Indicates the specific type of the Tunnel or TunnelPart."@en .

tun:HollowSpace.tunnelFurniture
        rdf:type         owl:ObjectProperty;
        rdfs:domain      tun:HollowSpace;
        rdfs:label       "tunnelFurniture"@en;
        rdfs:range       tun:TunnelFurniture;
        skos:definition  "Relates the furniture objects to the HollowSpace."@en .

tun:TunnelInstallationFunctionValue
        rdf:type         owl:Class;
        rdfs:label       "TunnelInstallationFunctionValue"@en;
        rdfs:subClassOf  skos:Concept;
        skos:definition  "TunnelInstallationFunctionValue is a code list that enumerates the different purposes of a TunnelInstallation."@en .

tun:HollowSpace.class
        rdf:type         owl:ObjectProperty;
        rdfs:domain      tun:HollowSpace;
        rdfs:label       "class"@en;
        rdfs:range       tun:HollowSpaceClassValue;
        skos:definition  "Indicates the specific type of the HollowSpace."@en .

tun:TunnelClassValue  rdf:type  owl:Class;
        rdfs:label       "TunnelClassValue"@en;
        rdfs:subClassOf  skos:Concept;
        skos:definition  "TunnelClassValue is a code list used to further classify a Tunnel."@en .

tun:HollowSpaceFunctionValue
        rdf:type         owl:Class;
        rdfs:label       "HollowSpaceFunctionValue"@en;
        rdfs:subClassOf  skos:Concept;
        skos:definition  "HollowSpaceFunctionValue is a code list that enumerates the different purposes of a HollowSpace."@en .

tun:HollowSpace.function
        rdf:type         owl:ObjectProperty;
        rdfs:domain      tun:HollowSpace;
        rdfs:label       "function"@en;
        rdfs:range       tun:HollowSpaceFunctionValue;
        skos:definition  "Specifies the intended purposes of the HollowSpace."@en .

tun:TunnelInstallation.class
        rdf:type         owl:ObjectProperty;
        rdfs:domain      tun:TunnelInstallation;
        rdfs:label       "class"@en;
        rdfs:range       tun:TunnelInstallationClassValue;
        skos:definition  "Indicates the specific type of the TunnelInstallation."@en .

tun:ADEOfTunnelInstallation
        rdf:type               owl:Class;
        rdfs:label             "ADEOfTunnelInstallation"@en;
        iso19150-2:isAbstract  true;
        skos:definition        "ADEOfTunnelInstallation acts as a hook to define properties within an ADE that are to be added to a TunnelInstallation."@en .

tun:ADEOfAbstractTunnel
        rdf:type               owl:Class;
        rdfs:label             "ADEOfAbstractTunnel"@en;
        iso19150-2:isAbstract  true;
        skos:definition        "ADEOfAbstractTunnel acts as a hook to define properties within an ADE that are to be added to AbstractTunnel."@en .

tun:tunnelConstructiveElement
        rdf:type         owl:ObjectProperty;
        rdfs:label       "tunnelConstructiveElement"@en;
        rdfs:range       tun:TunnelConstructiveElement;
        skos:definition  "Relates the constructive elements to the Tunnel or TunnelPart."@en .

tun:boundary  rdf:type   owl:ObjectProperty;
        rdfs:label       "boundary"@en;
        rdfs:range       core:AbstractThematicSurface;
        skos:definition  "Relates to the surfaces that bound the HollowSpace. This relation is inherited from the Core module."@en .

tun:ADEOfHollowSpace  rdf:type  owl:Class;
        rdfs:label             "ADEOfHollowSpace"@en;
        iso19150-2:isAbstract  true;
        skos:definition        "ADEOfHollowSpace acts as a hook to define properties within an ADE that are to be added to a HollowSpace."@en .

tun:HollowSpaceUsageValue
        rdf:type         owl:Class;
        rdfs:label       "HollowSpaceUsageValue"@en;
        rdfs:subClassOf  skos:Concept;
        skos:definition  "HollowSpaceUsageValue is a code list that enumerates the different uses of a HollowSpace."@en .

tun:TunnelFunctionValue
        rdf:type         owl:Class;
        rdfs:label       "TunnelFunctionValue"@en;
        rdfs:subClassOf  skos:Concept;
        skos:definition  "TunnelFunctionValue is a code list that enumerates the different purposes of a Tunnel."@en .

tun:AbstractTunnel.tunnelInstallation
        rdf:type         owl:ObjectProperty;
        rdfs:domain      tun:AbstractTunnel;
        rdfs:label       "tunnelInstallation"@en;
        rdfs:range       tun:TunnelInstallation;
        skos:definition  "Relates the installation objects to the Tunnel or TunnelPart."@en .

tun:TunnelConstructiveElement.usage
        rdf:type         owl:ObjectProperty;
        rdfs:domain      tun:TunnelConstructiveElement;
        rdfs:label       "usage"@en;
        rdfs:range       tun:TunnelConstructiveElementUsageValue;
        skos:definition  "Specifies the actual uses of the TunnelConstructiveElement."@en .

tun:adeOfTunnelFurniture
        rdf:type         owl:ObjectProperty;
        rdfs:label       "adeOfTunnelFurniture"@en;
        rdfs:range       tun:ADEOfTunnelFurniture;
        skos:definition  "Augments the TunnelFurniture with properties defined in an ADE."@en .

tun:TunnelPart  rdf:type  owl:Class;
        rdfs:label       "TunnelPart"@en;
        rdfs:subClassOf  tun:AbstractTunnel;
        rdfs:subClassOf  [ rdf:type           owl:Restriction;
                           owl:allValuesFrom  tun:ADEOfTunnelPart;
                           owl:onProperty     tun:adeOfTunnelPart
                         ];
        skos:definition  "A TunnelPart is a physical or functional subdivision of a Tunnel. It would be considered a Tunnel, if it were not part of a collection of other TunnelParts."@en .

tun:adeOfTunnel  rdf:type  owl:ObjectProperty;
        rdfs:label       "adeOfTunnel"@en;
        rdfs:range       tun:ADEOfTunnel;
        skos:definition  "Augments the Tunnel with properties defined in an ADE."@en .

tun:hollowSpace  rdf:type  owl:ObjectProperty;
        rdfs:label       "hollowSpace"@en;
        rdfs:range       tun:HollowSpace;
        skos:definition  "Relates the hollow spaces to the Tunnel or TunnelPart."@en .

tun:Tunnel  rdf:type      owl:Class;
        rdfs:label        "Tunnel"@en;
        rdfs:subClassOf   tun:AbstractTunnel;
        rdfs:subClassOf   [ rdf:type           owl:Restriction;
                            owl:allValuesFrom  tun:ADEOfTunnel;
                            owl:onProperty     tun:adeOfTunnel
                          ];
        rdfs:subClassOf   [ rdf:type           owl:Restriction;
                            owl:allValuesFrom  tun:TunnelPart;
                            owl:onProperty     tun:tunnelPart
                          ];
        owl:disjointWith  tun:TunnelPart;
        skos:definition   "A Tunnel represents a horizontal or sloping enclosed passage way of a certain length, mainly underground or underwater. [cf. ISO 6707-1]"@en .

tun:adeOfHollowSpace  rdf:type  owl:ObjectProperty;
        rdfs:label       "adeOfHollowSpace"@en;
        rdfs:range       tun:ADEOfHollowSpace;
        skos:definition  "Augments the HollowSpace with properties defined in an ADE."@en .

tun:TunnelInstallationUsageValue
        rdf:type         owl:Class;
        rdfs:label       "TunnelInstallationUsageValue"@en;
        rdfs:subClassOf  skos:Concept;
        skos:definition  "TunnelInstallationUsageValue is a code list that enumerates the different uses of a TunnelInstallation."@en .

tun:AbstractTunnel  rdf:type   owl:Class;
        rdfs:label             "AbstractTunnel"@en;
        rdfs:subClassOf        con:AbstractConstruction;
        rdfs:subClassOf        [ rdf:type           owl:Restriction;
                                 owl:allValuesFrom  tun:TunnelInstallation;
                                 owl:onProperty     tun:AbstractTunnel.tunnelInstallation
                               ];
        rdfs:subClassOf        [ rdf:type           owl:Restriction;
                                 owl:allValuesFrom  tun:TunnelConstructiveElement;
                                 owl:onProperty     tun:tunnelConstructiveElement
                               ];
        rdfs:subClassOf        [ rdf:type           owl:Restriction;
                                 owl:allValuesFrom  tun:TunnelUsageValue;
                                 owl:onProperty     tun:AbstractTunnel.usage
                               ];
        rdfs:subClassOf        [ rdf:type                     owl:Restriction;
                                 owl:maxQualifiedCardinality  "1"^^xsd:nonNegativeInteger;
                                 owl:onClass                  tun:TunnelClassValue;
                                 owl:onProperty               tun:AbstractTunnel.class
                               ];
        rdfs:subClassOf        [ rdf:type           owl:Restriction;
                                 owl:allValuesFrom  tun:ADEOfAbstractTunnel;
                                 owl:onProperty     tun:adeOfAbstractTunnel
                               ];
        rdfs:subClassOf        [ rdf:type           owl:Restriction;
                                 owl:allValuesFrom  tun:TunnelClassValue;
                                 owl:onProperty     tun:AbstractTunnel.class
                               ];
        rdfs:subClassOf        [ rdf:type           owl:Restriction;
                                 owl:allValuesFrom  tun:TunnelFunctionValue;
                                 owl:onProperty     tun:AbstractTunnel.function
                               ];
        rdfs:subClassOf        [ rdf:type           owl:Restriction;
                                 owl:allValuesFrom  tun:HollowSpace;
                                 owl:onProperty     tun:hollowSpace
                               ];
        rdfs:subClassOf        [ rdf:type           owl:Restriction;
                                 owl:allValuesFrom  tun:TunnelFurniture;
                                 owl:onProperty     tun:AbstractTunnel.tunnelFurniture
                               ];
        iso19150-2:isAbstract  true;
        skos:definition        "AbstractTunnel is an abstract superclass representing the common attributes and associations of the classes Tunnel and TunnelPart."@en .

tun:TunnelFurniture.function
        rdf:type         owl:ObjectProperty;
        rdfs:domain      tun:TunnelFurniture;
        rdfs:label       "function"@en;
        rdfs:range       tun:TunnelFurnitureFunctionValue;
        skos:definition  "Specifies the intended purposes of the TunnelFurniture."@en .

tun:adeOfTunnelInstallation
        rdf:type         owl:ObjectProperty;
        rdfs:label       "adeOfTunnelInstallation"@en;
        rdfs:range       tun:ADEOfTunnelInstallation;
        skos:definition  "Augments the TunnelInstallation with properties defined in an ADE."@en .

tun:adeOfAbstractTunnel
        rdf:type         owl:ObjectProperty;
        rdfs:label       "adeOfAbstractTunnel"@en;
        rdfs:range       tun:ADEOfAbstractTunnel;
        skos:definition  "Augments AbstractTunnel with properties defined in an ADE."@en .

tun:HollowSpaceClassValue
        rdf:type         owl:Class;
        rdfs:label       "HollowSpaceClassValue"@en;
        rdfs:subClassOf  skos:Concept;
        skos:definition  "HollowSpaceClassValue is a code list used to further classify a HollowSpace."@en .

tun:TunnelInstallation.function
        rdf:type         owl:ObjectProperty;
        rdfs:domain      tun:TunnelInstallation;
        rdfs:label       "function"@en;
        rdfs:range       tun:TunnelInstallationFunctionValue;
        skos:definition  "Specifies the intended purposes of the TunnelInstallation."@en .

tun:TunnelFurnitureUsageValue
        rdf:type         owl:Class;
        rdfs:label       "TunnelFurnitureUsageValue"@en;
        rdfs:subClassOf  skos:Concept;
        skos:definition  "TunnelFurnitureUsageValue is a code list that enumerates the different uses of a TunnelFurniture."@en .

tun:ADEOfTunnel  rdf:type      owl:Class;
        rdfs:label             "ADEOfTunnel"@en;
        iso19150-2:isAbstract  true;
        skos:definition        "ADEOfTunnel acts as a hook to define properties within an ADE that are to be added to a Tunnel."@en .

tun:TunnelConstructiveElementUsageValue
        rdf:type         owl:Class;
        rdfs:label       "TunnelConstructiveElementUsageValue"@en;
        rdfs:subClassOf  skos:Concept;
        skos:definition  "TunnelConstructiveElementUsageValue is a code list that enumerates the different uses of a TunnelConstructiveElement."@en .

tun:TunnelConstructiveElementFunctionValue
        rdf:type         owl:Class;
        rdfs:label       "TunnelConstructiveElementFunctionValue"@en;
        rdfs:subClassOf  skos:Concept;
        skos:definition  "TunnelConstructiveElementFunctionValue is a code list that enumerates the different purposes of a TunnelConstructiveElement."@en .

tun:adeOfTunnelConstructiveElement
        rdf:type         owl:ObjectProperty;
        rdfs:label       "adeOfTunnelConstructiveElement"@en;
        rdfs:range       tun:ADEOfTunnelConstructiveElement;
        skos:definition  "Augments the TunnelConstructiveElement with properties defined in an ADE."@en .

tun:ADEOfTunnelFurniture
        rdf:type               owl:Class;
        rdfs:label             "ADEOfTunnelFurniture"@en;
        iso19150-2:isAbstract  true;
        skos:definition        "ADEOfTunnelFurniture acts as a hook to define properties within an ADE that are to be added to a TunnelFurniture."@en .

tun:adeOfTunnelPart  rdf:type  owl:ObjectProperty;
        rdfs:label       "adeOfTunnelPart"@en;
        rdfs:range       tun:ADEOfTunnelPart;
        skos:definition  "Augments the TunnelPart with properties defined in an ADE."@en .

<https://www.opengis.net/ont/citygml/tunnel>
        rdf:type         owl:Ontology;
        rdfs:label       "Tunnel"@en;
        owl:imports      <https://www.opengis.net/ont/citygml/construction> , <https://www.opengis.net/ont/citygml/core> , <http://def.isotc211.org/iso19150/-2/2012/base>;
        skos:definition  "The Tunnel module supports representation of thematic and spatial aspects of tunnels, tunnel parts, tunnel installations, and interior tunnel structures."@en .

tun:AbstractTunnel.function
        rdf:type         owl:ObjectProperty;
        rdfs:domain      tun:AbstractTunnel;
        rdfs:label       "function"@en;
        rdfs:range       tun:TunnelFunctionValue;
        skos:definition  "Specifies the intended purposes of the Tunnel or TunnelPart."@en .

tun:HollowSpace.tunnelInstallation
        rdf:type         owl:ObjectProperty;
        rdfs:domain      tun:HollowSpace;
        rdfs:label       "tunnelInstallation"@en;
        rdfs:range       tun:TunnelInstallation;
        skos:definition  "Relates the installation objects to the HollowSpace."@en .

tun:TunnelConstructiveElement.class
        rdf:type         owl:ObjectProperty;
        rdfs:domain      tun:TunnelConstructiveElement;
        rdfs:label       "class"@en;
        rdfs:range       tun:TunnelConstructiveElementClassValue;
        skos:definition  "Indicates the specific type of the TunnelConstructiveElement."@en .

tun:TunnelFurniture.usage
        rdf:type         owl:ObjectProperty;
        rdfs:domain      tun:TunnelFurniture;
        rdfs:label       "usage"@en;
        rdfs:range       tun:TunnelFurnitureUsageValue;
        skos:definition  "Specifies the actual uses of the TunnelFurniture."@en .

tun:AbstractTunnel.usage
        rdf:type         owl:ObjectProperty;
        rdfs:domain      tun:AbstractTunnel;
        rdfs:label       "usage"@en;
        rdfs:range       tun:TunnelUsageValue;
        skos:definition  "Specifies the actual uses of the Tunnel or TunnelPart."@en .

tun:TunnelInstallation
        rdf:type         owl:Class;
        rdfs:label       "TunnelInstallation"@en;
        rdfs:subClassOf  con:AbstractInstallation;
        rdfs:subClassOf  [ rdf:type           owl:Restriction;
                           owl:allValuesFrom  tun:ADEOfTunnelInstallation;
                           owl:onProperty     tun:adeOfTunnelInstallation
                         ];
        rdfs:subClassOf  [ rdf:type           owl:Restriction;
                           owl:allValuesFrom  tun:TunnelInstallationUsageValue;
                           owl:onProperty     tun:TunnelInstallation.usage
                         ];
        rdfs:subClassOf  [ rdf:type           owl:Restriction;
                           owl:allValuesFrom  tun:TunnelInstallationFunctionValue;
                           owl:onProperty     tun:TunnelInstallation.function
                         ];
        rdfs:subClassOf  [ rdf:type           owl:Restriction;
                           owl:allValuesFrom  tun:TunnelInstallationClassValue;
                           owl:onProperty     tun:TunnelInstallation.class
                         ];
        rdfs:subClassOf  [ rdf:type                     owl:Restriction;
                           owl:maxQualifiedCardinality  "1"^^xsd:nonNegativeInteger;
                           owl:onClass                  tun:TunnelInstallationClassValue;
                           owl:onProperty               tun:TunnelInstallation.class
                         ];
        skos:definition  "A TunnelInstallation is a permanent part of a Tunnel (inside and/or outside) which does not have the significance of a TunnelPart. In contrast to TunnelConstructiveElement, a TunnelInstallation is not essential from a structural point of view. Examples are stairs, antennas or railings."@en .

tun:TunnelInstallationClassValue
        rdf:type         owl:Class;
        rdfs:label       "TunnelInstallationClassValue"@en;
        rdfs:subClassOf  skos:Concept;
        skos:definition  "TunnelInstallationClassValue is a code list used to further classify a TunnelInstallation."@en .

tun:TunnelConstructiveElement
        rdf:type         owl:Class;
        rdfs:label       "TunnelConstructiveElement"@en;
        rdfs:subClassOf  con:AbstractConstructiveElement;
        rdfs:subClassOf  [ rdf:type           owl:Restriction;
                           owl:allValuesFrom  tun:ADEOfTunnelConstructiveElement;
                           owl:onProperty     tun:adeOfTunnelConstructiveElement
                         ];
        rdfs:subClassOf  [ rdf:type           owl:Restriction;
                           owl:allValuesFrom  tun:TunnelConstructiveElementUsageValue;
                           owl:onProperty     tun:TunnelConstructiveElement.usage
                         ];
        rdfs:subClassOf  [ rdf:type           owl:Restriction;
                           owl:allValuesFrom  tun:TunnelConstructiveElementFunctionValue;
                           owl:onProperty     tun:TunnelConstructiveElement.function
                         ];
        rdfs:subClassOf  [ rdf:type           owl:Restriction;
                           owl:allValuesFrom  tun:TunnelConstructiveElementClassValue;
                           owl:onProperty     tun:TunnelConstructiveElement.class
                         ];
        rdfs:subClassOf  [ rdf:type                     owl:Restriction;
                           owl:maxQualifiedCardinality  "1"^^xsd:nonNegativeInteger;
                           owl:onClass                  tun:TunnelConstructiveElementClassValue;
                           owl:onProperty               tun:TunnelConstructiveElement.class
                         ];
        skos:definition  "A TunnelConstructiveElement is an element of a Tunnel which is essential from a structural point of view. Examples are walls, slabs, beams."@en .

tun:tunnelPart  rdf:type  owl:ObjectProperty;
        rdfs:label       "tunnelPart"@en;
        rdfs:range       tun:TunnelPart;
        skos:definition  "Relates the tunnel parts to the Tunnel."@en .

tun:TunnelFurnitureFunctionValue
        rdf:type         owl:Class;
        rdfs:label       "TunnelFurnitureFunctionValue"@en;
        rdfs:subClassOf  skos:Concept;
        skos:definition  "TunnelFurnitureFunctionValue is a code list that enumerates the different purposes of a TunnelFurniture."@en .

tun:HollowSpace.usage
        rdf:type         owl:ObjectProperty;
        rdfs:domain      tun:HollowSpace;
        rdfs:label       "usage"@en;
        rdfs:range       tun:HollowSpaceUsageValue;
        skos:definition  "Specifies the actual uses of the HollowSpace."@en .

tun:TunnelFurnitureClassValue
        rdf:type         owl:Class;
        rdfs:label       "TunnelFurnitureClassValue"@en;
        rdfs:subClassOf  skos:Concept;
        skos:definition  "TunnelFurnitureClassValue is a code list used to further classify a TunnelFurniture."@en .

tun:TunnelConstructiveElementClassValue
        rdf:type         owl:Class;
        rdfs:label       "TunnelConstructiveElementClassValue"@en;
        rdfs:subClassOf  skos:Concept;
        skos:definition  "TunnelConstructiveElementClassValue is a code list used to further classify a TunnelConstructiveElement."@en .

tun:TunnelFurniture  rdf:type  owl:Class;
        rdfs:label       "TunnelFurniture"@en;
        rdfs:subClassOf  con:AbstractFurniture;
        rdfs:subClassOf  [ rdf:type           owl:Restriction;
                           owl:allValuesFrom  tun:ADEOfTunnelFurniture;
                           owl:onProperty     tun:adeOfTunnelFurniture
                         ];
        rdfs:subClassOf  [ rdf:type           owl:Restriction;
                           owl:allValuesFrom  tun:TunnelFurnitureUsageValue;
                           owl:onProperty     tun:TunnelFurniture.usage
                         ];
        rdfs:subClassOf  [ rdf:type           owl:Restriction;
                           owl:allValuesFrom  tun:TunnelFurnitureFunctionValue;
                           owl:onProperty     tun:TunnelFurniture.function
                         ];
        rdfs:subClassOf  [ rdf:type           owl:Restriction;
                           owl:allValuesFrom  tun:TunnelFurnitureClassValue;
                           owl:onProperty     tun:TunnelFurniture.class
                         ];
        rdfs:subClassOf  [ rdf:type                     owl:Restriction;
                           owl:maxQualifiedCardinality  "1"^^xsd:nonNegativeInteger;
                           owl:onClass                  tun:TunnelFurnitureClassValue;
                           owl:onProperty               tun:TunnelFurniture.class
                         ];
        skos:definition  "A TunnelFurniture is an equipment for occupant use, usually not fixed to the tunnel. [cf. ISO 6707-1]"@en .

tun:TunnelConstructiveElement.function
        rdf:type         owl:ObjectProperty;
        rdfs:domain      tun:TunnelConstructiveElement;
        rdfs:label       "function"@en;
        rdfs:range       tun:TunnelConstructiveElementFunctionValue;
        skos:definition  "Specifies the intended purposes of the TunnelConstructiveElement."@en .

tun:TunnelInstallation.usage
        rdf:type         owl:ObjectProperty;
        rdfs:domain      tun:TunnelInstallation;
        rdfs:label       "usage"@en;
        rdfs:range       tun:TunnelInstallationUsageValue;
        skos:definition  "Specifies the actual uses of the TunnelInstallation."@en .

tun:AbstractTunnel.tunnelFurniture
        rdf:type         owl:ObjectProperty;
        rdfs:domain      tun:AbstractTunnel;
        rdfs:label       "tunnelFurniture"@en;
        rdfs:range       tun:TunnelFurniture;
        skos:definition  "Relates the furniture objects to the Tunnel or TunnelPart."@en .
