@prefix core: <https://www.opengis.net/ont/citygml/core/> .
@prefix iso19150-2: <http://def.isotc211.org/iso19150/-2/2012/base#> .
@prefix owl: <http://www.w3.org/2002/07/owl#> .
@prefix rdf: <http://www.w3.org/1999/02/22-rdf-syntax-ns#> .
@prefix rdfs: <http://www.w3.org/2000/01/rdf-schema#> .
@prefix skos: <http://www.w3.org/2004/02/skos/core#> .
@prefix tran: <https://www.opengis.net/ont/citygml/transportation/> .
@prefix xsd: <http://www.w3.org/2001/XMLSchema#> .

<https://www.opengis.net/ont/citygml/transportation> a owl:Ontology ;
    rdfs:label "Transportation"@en ;
    owl:imports <http://def.isotc211.org/iso19150/-2/2012/base>,
        <https://www.opengis.net/ont/citygml/core> ;
    skos:definition "The Transportation module supports representation of the transportation infrastructure. Transportation features include roads, tracks, waterways, railways, and squares. Transportation features may be represented as a network and/or as a collection of spaces or surface elements embedded in a three-dimensional space."@en .

tran:HoleSurface a owl:Class ;
    rdfs:label "HoleSurface"@en ;
    rdfs:subClassOf [ a owl:Restriction ;
            owl:allValuesFrom tran:ADEOfHoleSurface ;
            owl:onProperty tran:adeOfHoleSurface ],
        core:AbstractThematicSurface ;
    skos:definition "A HoleSurface is a representation of the ground surface of a hole."@en .

tran:AbstractTransportationSpace.occupancy a owl:ObjectProperty ;
    rdfs:label "occupancy"@en ;
    rdfs:domain tran:AbstractTransportationSpace ;
    rdfs:range core:Occupancy ;
    skos:definition "Provides information on the residency of persons, vehicles, or other moving features in the transportation space."@en .

tran:AuxiliaryTrafficArea.function a owl:ObjectProperty ;
    rdfs:label "function"@en ;
    rdfs:domain tran:AuxiliaryTrafficArea ;
    rdfs:range tran:AuxiliaryTrafficAreaFunctionValue ;
    skos:definition "Specifies the intended purposes of the AuxiliaryTrafficArea."@en .

tran:AuxiliaryTrafficArea.usage a owl:ObjectProperty ;
    rdfs:label "usage"@en ;
    rdfs:domain tran:AuxiliaryTrafficArea ;
    rdfs:range tran:AuxiliaryTrafficAreaUsageValue ;
    skos:definition "Specifies the actual uses of the AuxiliaryTrafficArea."@en .

tran:AuxiliaryTrafficSpace.boundary a owl:ObjectProperty ;
    rdfs:label "boundary"@en ;
    rdfs:domain tran:AuxiliaryTrafficSpace ;
    rdfs:range tran:AuxiliaryTrafficArea ;
    skos:definition "Relates to the auxiliary traffic areas that bound the AuxiliaryTrafficSpace. This relation is inherited from the Core module."@en .

tran:AuxiliaryTrafficSpace.function a owl:ObjectProperty ;
    rdfs:label "function"@en ;
    rdfs:domain tran:AuxiliaryTrafficSpace ;
    rdfs:range tran:AuxiliaryTrafficSpaceFunctionValue ;
    skos:definition "Specifies the intended purposes of the AuxiliaryTrafficSpace."@en .

tran:AuxiliaryTrafficSpace.usage a owl:ObjectProperty ;
    rdfs:label "usage"@en ;
    rdfs:domain tran:AuxiliaryTrafficSpace ;
    rdfs:range tran:AuxiliaryTrafficSpaceUsageValue ;
    skos:definition "Specifies the actual uses of the AuxiliaryTrafficSpace."@en .

tran:ClearanceSpace.class a owl:ObjectProperty ;
    rdfs:label "class"@en ;
    rdfs:domain tran:ClearanceSpace ;
    rdfs:range tran:ClearanceSpaceClassValue ;
    skos:definition "Indicates the specific type of the ClearanceSpace."@en .

tran:Railway.function a owl:ObjectProperty ;
    rdfs:label "function"@en ;
    rdfs:domain tran:Railway ;
    rdfs:range tran:RailwayFunctionValue ;
    skos:definition "Specifies the intended purposes of the Railway."@en .

tran:Railway.intersection a owl:ObjectProperty ;
    rdfs:label "intersection"@en ;
    rdfs:domain tran:Railway ;
    rdfs:range tran:Intersection ;
    skos:definition "Relates to the intersections that are part of the Railway."@en .

tran:Railway.section a owl:ObjectProperty ;
    rdfs:label "section"@en ;
    rdfs:domain tran:Railway ;
    rdfs:range tran:Section ;
    skos:definition "Relates to the sections that are part of the Railway."@en .

tran:Railway.usage a owl:ObjectProperty ;
    rdfs:label "usage"@en ;
    rdfs:domain tran:Railway ;
    rdfs:range tran:RailwayUsageValue ;
    skos:definition "Specifies the actual uses of the Railway."@en .

tran:Road.function a owl:ObjectProperty ;
    rdfs:label "function"@en ;
    rdfs:domain tran:Road ;
    rdfs:range tran:RoadFunctionValue ;
    skos:definition "Specifies the intended purposes of the Road."@en .

tran:Road.intersection a owl:ObjectProperty ;
    rdfs:label "intersection"@en ;
    rdfs:domain tran:Road ;
    rdfs:range tran:Intersection ;
    skos:definition "Relates to the intersections that are part of the Road."@en .

tran:Road.section a owl:ObjectProperty ;
    rdfs:label "section"@en ;
    rdfs:domain tran:Road ;
    rdfs:range tran:Section ;
    skos:definition "Relates to the sections that are part of the Road."@en .

tran:Road.usage a owl:ObjectProperty ;
    rdfs:label "usage"@en ;
    rdfs:domain tran:Road ;
    rdfs:range tran:RoadUsageValue ;
    skos:definition "Specifies the actual uses of the Road."@en .

tran:Square.function a owl:ObjectProperty ;
    rdfs:label "function"@en ;
    rdfs:domain tran:Square ;
    rdfs:range tran:SquareFunctionValue ;
    skos:definition "Specifies the intended purposes of the Square."@en .

tran:Square.usage a owl:ObjectProperty ;
    rdfs:label "usage"@en ;
    rdfs:domain tran:Square ;
    rdfs:range tran:SquareUsageValue ;
    skos:definition "Specifies the actual uses of the Square."@en .

tran:Track.function a owl:ObjectProperty ;
    rdfs:label "function"@en ;
    rdfs:domain tran:Track ;
    rdfs:range tran:TrackFunctionValue ;
    skos:definition "Specifies the intended purposes of the Track."@en .

tran:Track.intersection a owl:ObjectProperty ;
    rdfs:label "intersection"@en ;
    rdfs:domain tran:Track ;
    rdfs:range tran:Intersection ;
    skos:definition "Relates to the intersections that are part of the Track."@en .

tran:Track.section a owl:ObjectProperty ;
    rdfs:label "section"@en ;
    rdfs:domain tran:Track ;
    rdfs:range tran:Section ;
    skos:definition "Relates to the sections that are part of the Track."@en .

tran:Track.usage a owl:ObjectProperty ;
    rdfs:label "usage"@en ;
    rdfs:domain tran:Track ;
    rdfs:range tran:TrackUsageValue ;
    skos:definition "Specifies the actual uses of the Track."@en .

tran:TrafficArea.function a owl:ObjectProperty ;
    rdfs:label "function"@en ;
    rdfs:domain tran:TrafficArea ;
    rdfs:range tran:TrafficAreaFunctionValue ;
    skos:definition "Specifies the intended purposes of the TrafficArea."@en .

tran:TrafficArea.usage a owl:ObjectProperty ;
    rdfs:label "usage"@en ;
    rdfs:domain tran:TrafficArea ;
    rdfs:range tran:TrafficAreaUsageValue ;
    skos:definition "Specifies the actual uses of the TrafficArea."@en .

tran:TrafficSpace.boundary a owl:ObjectProperty ;
    rdfs:label "boundary"@en ;
    rdfs:domain tran:TrafficSpace ;
    rdfs:range tran:TrafficArea ;
    skos:definition "Relates to the traffic areas that bound the TrafficSpace. This relation is inherited from the Core module."@en .

tran:TrafficSpace.function a owl:ObjectProperty ;
    rdfs:label "function"@en ;
    rdfs:domain tran:TrafficSpace ;
    rdfs:range tran:TrafficSpaceFunctionValue ;
    skos:definition "Specifies the intended purposes of the TrafficSpace."@en .

tran:TrafficSpace.occupancy a owl:ObjectProperty ;
    rdfs:label "occupancy"@en ;
    rdfs:domain tran:TrafficSpace ;
    rdfs:range core:Occupancy ;
    skos:definition "Provides information on the residency of persons, vehicles, or other moving features in the TrafficSpace."@en .

tran:TrafficSpace.usage a owl:ObjectProperty ;
    rdfs:label "usage"@en ;
    rdfs:domain tran:TrafficSpace ;
    rdfs:range tran:TrafficSpaceUsageValue ;
    skos:definition "Specifies the actual uses of the TrafficSpace."@en .

tran:Waterway.function a owl:ObjectProperty ;
    rdfs:label "function"@en ;
    rdfs:domain tran:Waterway ;
    rdfs:range tran:WaterwayFunctionValue ;
    skos:definition "Specifies the intended purposes of the Waterway."@en .

tran:Waterway.intersection a owl:ObjectProperty ;
    rdfs:label "intersection"@en ;
    rdfs:domain tran:Waterway ;
    rdfs:range tran:Intersection ;
    skos:definition "Relates to the intersections that are part of the Waterway."@en .

tran:Waterway.section a owl:ObjectProperty ;
    rdfs:label "section"@en ;
    rdfs:domain tran:Waterway ;
    rdfs:range tran:Section ;
    skos:definition "Relates to the sections that are part of the Waterway."@en .

tran:Waterway.usage a owl:ObjectProperty ;
    rdfs:label "usage"@en ;
    rdfs:domain tran:Waterway ;
    rdfs:range tran:WaterwayUsageValue ;
    skos:definition "Specifies the actual uses of the Waterway."@en .

tran:adeOfAbstractTransportationSpace a owl:ObjectProperty ;
    rdfs:label "adeOfAbstractTransportationSpace"@en ;
    rdfs:range tran:ADEOfAbstractTransportationSpace ;
    skos:definition "Augments AbstractTransportationSpace with properties defined in an ADE."@en .

tran:adeOfAuxiliaryTrafficArea a owl:ObjectProperty ;
    rdfs:label "adeOfAuxiliaryTrafficArea"@en ;
    rdfs:range tran:ADEOfAuxiliaryTrafficArea ;
    skos:definition "Augments the AuxiliaryTrafficArea with properties defined in an ADE."@en .

tran:adeOfAuxiliaryTrafficSpace a owl:ObjectProperty ;
    rdfs:label "adeOfAuxiliaryTrafficSpace"@en ;
    rdfs:range tran:ADEOfAuxiliaryTrafficSpace ;
    skos:definition "Augments the AuxiliaryTrafficSpace with properties defined in an ADE."@en .

tran:adeOfClearanceSpace a owl:ObjectProperty ;
    rdfs:label "adeOfClearanceSpace"@en ;
    rdfs:range tran:ADEOfClearanceSpace ;
    skos:definition "Augments the ClearanceSpace with properties defined in an ADE."@en .

tran:adeOfHole a owl:ObjectProperty ;
    rdfs:label "adeOfHole"@en ;
    rdfs:range tran:ADEOfHole ;
    skos:definition "Augments the Hole with properties defined in an ADE."@en .

tran:adeOfHoleSurface a owl:ObjectProperty ;
    rdfs:label "adeOfHoleSurface"@en ;
    rdfs:range tran:ADEOfHoleSurface ;
    skos:definition "Augments the HoleSurface with properties defined in an ADE."@en .

tran:adeOfIntersection a owl:ObjectProperty ;
    rdfs:label "adeOfIntersection"@en ;
    rdfs:range tran:ADEOfIntersection ;
    skos:definition "Augments the Intersection with properties defined in an ADE."@en .

tran:adeOfMarking a owl:ObjectProperty ;
    rdfs:label "adeOfMarking"@en ;
    rdfs:range tran:ADEOfMarking ;
    skos:definition "Augments the Marking with properties defined in an ADE."@en .

tran:adeOfRailway a owl:ObjectProperty ;
    rdfs:label "adeOfRailway"@en ;
    rdfs:range tran:ADEOfRailway ;
    skos:definition "Augments the Railway with properties defined in an ADE."@en .

tran:adeOfRoad a owl:ObjectProperty ;
    rdfs:label "adeOfRoad"@en ;
    rdfs:range tran:ADEOfRoad ;
    skos:definition "Augments the Road with properties defined in an ADE."@en .

tran:adeOfSection a owl:ObjectProperty ;
    rdfs:label "adeOfSection"@en ;
    rdfs:range tran:ADEOfSection ;
    skos:definition "Augments the Section with properties defined in an ADE."@en .

tran:adeOfSquare a owl:ObjectProperty ;
    rdfs:label "adeOfSquare"@en ;
    rdfs:range tran:ADEOfSquare ;
    skos:definition "Augments the Square with properties defined in an ADE."@en .

tran:adeOfTrack a owl:ObjectProperty ;
    rdfs:label "adeOfTrack"@en ;
    rdfs:range tran:ADEOfTrack ;
    skos:definition "Augments the Track with properties defined in an ADE."@en .

tran:adeOfTrafficArea a owl:ObjectProperty ;
    rdfs:label "adeOfTrafficArea"@en ;
    rdfs:range tran:ADEOfTrafficArea ;
    skos:definition "Augments the TrafficArea with properties defined in an ADE."@en .

tran:adeOfTrafficSpace a owl:ObjectProperty ;
    rdfs:label "adeOfTrafficSpace"@en ;
    rdfs:range tran:ADEOfTrafficSpace ;
    skos:definition "Augments the TrafficSpace with properties defined in an ADE."@en .

tran:adeOfWaterway a owl:ObjectProperty ;
    rdfs:label "adeOfWaterway"@en ;
    rdfs:range tran:ADEOfWaterway ;
    skos:definition "Augments the Waterway with properties defined in an ADE."@en .

tran:auxiliaryTrafficSpace a owl:ObjectProperty ;
    rdfs:label "auxiliaryTrafficSpace"@en ;
    rdfs:range tran:AuxiliaryTrafficSpace ;
    skos:definition "Relates to the auxiliary traffic spaces that are part of the transportation space."@en .

tran:clearanceSpace a owl:ObjectProperty ;
    rdfs:label "clearanceSpace"@en ;
    rdfs:range tran:ClearanceSpace ;
    skos:definition "Relates to the clearance spaces that are part of the TrafficSpace."@en .

tran:hole a owl:ObjectProperty ;
    rdfs:label "hole"@en ;
    rdfs:range tran:Hole ;
    skos:definition "Relates to the holes that are part of the transportation space."@en .

tran:marking a owl:ObjectProperty ;
    rdfs:label "marking"@en ;
    rdfs:range tran:Marking ;
    skos:definition "Relates to the markings that are part of the transportation space."@en .

tran:predecessor a owl:ObjectProperty ;
    rdfs:label "predecessor"@en ;
    rdfs:range tran:TrafficSpace ;
    skos:definition "Indicates the predecessor(s) of the TrafficSpace."@en .

tran:successor a owl:ObjectProperty ;
    rdfs:label "successor"@en ;
    rdfs:range tran:TrafficSpace ;
    skos:definition "Indicates the successor(s) of the TrafficSpace."@en .

tran:trafficSpace a owl:ObjectProperty ;
    rdfs:label "trafficSpace"@en ;
    rdfs:range tran:TrafficSpace ;
    skos:definition "Relates to the traffic spaces that are part of the transportation space."@en .

tran:ADEOfAbstractTransportationSpace a owl:Class ;
    rdfs:label "ADEOfAbstractTransportationSpace"@en ;
    iso19150-2:isAbstract true ;
    skos:definition "ADEOfAbstractTransportationSpace acts as a hook to define properties within an ADE that are to be added to AbstractTransportationSpace."@en .

tran:ADEOfAuxiliaryTrafficArea a owl:Class ;
    rdfs:label "ADEOfAuxiliaryTrafficArea"@en ;
    iso19150-2:isAbstract true ;
    skos:definition "ADEOfAuxiliaryTrafficArea acts as a hook to define properties within an ADE that are to be added to an AuxiliaryTrafficArea."@en .

tran:ADEOfAuxiliaryTrafficSpace a owl:Class ;
    rdfs:label "ADEOfAuxiliaryTrafficSpace"@en ;
    iso19150-2:isAbstract true ;
    skos:definition "ADEOfAuxiliaryTrafficSpace acts as a hook to define properties within an ADE that are to be added to an AuxiliaryTrafficSpace."@en .

tran:ADEOfClearanceSpace a owl:Class ;
    rdfs:label "ADEOfClearanceSpace"@en ;
    iso19150-2:isAbstract true ;
    skos:definition "ADEOfClearanceSpace acts as a hook to define properties within an ADE that are to be added to a ClearanceSpace."@en .

tran:ADEOfHole a owl:Class ;
    rdfs:label "ADEOfHole"@en ;
    iso19150-2:isAbstract true ;
    skos:definition "ADEOfHole acts as a hook to define properties within an ADE that are to be added to a Hole."@en .

tran:ADEOfHoleSurface a owl:Class ;
    rdfs:label "ADEOfHoleSurface"@en ;
    iso19150-2:isAbstract true ;
    skos:definition "ADEOfHoleSurface acts as a hook to define properties within an ADE that are to be added to a HoleSurface."@en .

tran:ADEOfIntersection a owl:Class ;
    rdfs:label "ADEOfIntersection"@en ;
    iso19150-2:isAbstract true ;
    skos:definition "ADEOfIntersection acts as a hook to define properties within an ADE that are to be added to an Intersection."@en .

tran:ADEOfMarking a owl:Class ;
    rdfs:label "ADEOfMarking"@en ;
    iso19150-2:isAbstract true ;
    skos:definition "ADEOfMarking acts as a hook to define properties within an ADE that are to be added to a Marking."@en .

tran:ADEOfRailway a owl:Class ;
    rdfs:label "ADEOfRailway"@en ;
    iso19150-2:isAbstract true ;
    skos:definition "ADEOfRailway acts as a hook to define properties within an ADE that are to be added to a Railway."@en .

tran:ADEOfRoad a owl:Class ;
    rdfs:label "ADEOfRoad"@en ;
    iso19150-2:isAbstract true ;
    skos:definition "ADEOfRoad acts as a hook to define properties within an ADE that are to be added to a Road."@en .

tran:ADEOfSection a owl:Class ;
    rdfs:label "ADEOfSection"@en ;
    iso19150-2:isAbstract true ;
    skos:definition "ADEOfSection acts as a hook to define properties within an ADE that are to be added to a Section."@en .

tran:ADEOfSquare a owl:Class ;
    rdfs:label "ADEOfSquare"@en ;
    iso19150-2:isAbstract true ;
    skos:definition "ADEOfSquare acts as a hook to define properties within an ADE that are to be added to a Square."@en .

tran:ADEOfTrack a owl:Class ;
    rdfs:label "ADEOfTrack"@en ;
    iso19150-2:isAbstract true ;
    skos:definition "ADEOfTrack acts as a hook to define properties within an ADE that are to be added to a Track."@en .

tran:ADEOfTrafficArea a owl:Class ;
    rdfs:label "ADEOfTrafficArea"@en ;
    iso19150-2:isAbstract true ;
    skos:definition "ADEOfTrafficArea acts as a hook to define properties within an ADE that are to be added to a TrafficArea."@en .

tran:ADEOfTrafficSpace a owl:Class ;
    rdfs:label "ADEOfTrafficSpace"@en ;
    iso19150-2:isAbstract true ;
    skos:definition "ADEOfTrafficSpace acts as a hook to define properties within an ADE that are to be added to a TrafficSpace."@en .

tran:ADEOfWaterway a owl:Class ;
    rdfs:label "ADEOfWaterway"@en ;
    iso19150-2:isAbstract true ;
    skos:definition "ADEOfWaterway acts as a hook to define properties within an ADE that are to be added to a Waterway."@en .

tran:AbstractTransportationSpace.trafficDirection a owl:DatatypeProperty ;
    rdfs:label "trafficDirection"@en ;
    rdfs:domain tran:AbstractTransportationSpace ;
    rdfs:range tran:TrafficDirectionValue ;
    skos:definition "Indicates the direction of traffic flow relative to the corresponding linear geometry representation."@en .

tran:AuxiliaryTrafficArea.class a owl:ObjectProperty ;
    rdfs:label "class"@en ;
    rdfs:domain tran:AuxiliaryTrafficArea ;
    rdfs:range tran:AuxiliaryTrafficAreaClassValue ;
    skos:definition "Indicates the specific type of the AuxiliaryTrafficArea."@en .

tran:AuxiliaryTrafficArea.surfaceMaterial a owl:ObjectProperty ;
    rdfs:label "surfaceMaterial"@en ;
    rdfs:domain tran:AuxiliaryTrafficArea ;
    rdfs:range tran:SurfaceMaterialValue ;
    skos:definition "Specifies the type of pavement of the AuxiliaryTrafficArea."@en .

tran:AuxiliaryTrafficAreaFunctionValue a owl:Class ;
    rdfs:label "AuxiliaryTrafficAreaFunctionValue"@en ;
    rdfs:subClassOf skos:Concept ;
    skos:definition "AuxiliaryTrafficAreaFunctionValue is a code list that enumerates the different purposes of an AuxiliaryTrafficArea."@en .

tran:AuxiliaryTrafficAreaUsageValue a owl:Class ;
    rdfs:label "AuxiliaryTrafficAreaUsageValue"@en ;
    rdfs:subClassOf skos:Concept ;
    skos:definition "AuxiliaryTrafficAreaUsageValue is a code list that enumerates the different uses of an AuxiliaryTrafficArea."@en .

tran:AuxiliaryTrafficSpace.class a owl:ObjectProperty ;
    rdfs:label "class"@en ;
    rdfs:domain tran:AuxiliaryTrafficSpace ;
    rdfs:range tran:AuxiliaryTrafficSpaceClassValue ;
    skos:definition "Indicates the specific type of the AuxiliaryTrafficSpace."@en .

tran:AuxiliaryTrafficSpace.granularity a owl:DatatypeProperty ;
    rdfs:label "granularity"@en ;
    rdfs:domain tran:AuxiliaryTrafficSpace ;
    rdfs:range tran:GranularityValue ;
    skos:definition "Defines whether auxiliary traffic spaces are represented by individual ways or by individual lanes, depending on the desired level of spatial and semantic decomposition."@en .

tran:AuxiliaryTrafficSpaceFunctionValue a owl:Class ;
    rdfs:label "AuxiliaryTrafficSpaceFunctionValue"@en ;
    rdfs:subClassOf skos:Concept ;
    skos:definition "AuxiliaryTrafficSpaceFunctionValue is a code list that enumerates the different purposes of an AuxiliaryTrafficSpace."@en .

tran:AuxiliaryTrafficSpaceUsageValue a owl:Class ;
    rdfs:label "AuxiliaryTrafficSpaceUsageValue"@en ;
    rdfs:subClassOf skos:Concept ;
    skos:definition "AuxiliaryTrafficSpaceUsageValue is a code list that enumerates the different uses of an AuxiliaryTrafficSpace."@en .

tran:ClearanceSpaceClassValue a owl:Class ;
    rdfs:label "ClearanceSpaceClassValue"@en ;
    rdfs:subClassOf skos:Concept ;
    skos:definition "ClearanceSpaceClassValue is a code list used to further classify a ClearanceSpace."@en .

tran:Hole.class a owl:ObjectProperty ;
    rdfs:label "class"@en ;
    rdfs:domain tran:Hole ;
    rdfs:range tran:HoleClassValue ;
    skos:definition "Indicates the specific type of the Hole."@en .

tran:Intersection.class a owl:ObjectProperty ;
    rdfs:label "class"@en ;
    rdfs:domain tran:Intersection ;
    rdfs:range tran:IntersectionClassValue ;
    skos:definition "Indicates the specific type of the Intersection."@en .

tran:Marking.class a owl:ObjectProperty ;
    rdfs:label "class"@en ;
    rdfs:domain tran:Marking ;
    rdfs:range tran:MarkingClassValue ;
    skos:definition "Indicates the specific type of the Marking."@en .

tran:Railway.class a owl:ObjectProperty ;
    rdfs:label "class"@en ;
    rdfs:domain tran:Railway ;
    rdfs:range tran:RailwayClassValue ;
    skos:definition "Indicates the specific type of the Railway."@en .

tran:RailwayFunctionValue a owl:Class ;
    rdfs:label "RailwayFunctionValue"@en ;
    rdfs:subClassOf skos:Concept ;
    skos:definition "RailwayFunctionValue is a code list that enumerates the different purposes of a Railway."@en .

tran:RailwayUsageValue a owl:Class ;
    rdfs:label "RailwayUsageValue"@en ;
    rdfs:subClassOf skos:Concept ;
    skos:definition "RailwayUsageValue is a code list that enumerates the different uses of a Railway."@en .

tran:Road.class a owl:ObjectProperty ;
    rdfs:label "class"@en ;
    rdfs:domain tran:Road ;
    rdfs:range tran:RoadClassValue ;
    skos:definition "Indicates the specific type of the Road."@en .

tran:RoadFunctionValue a owl:Class ;
    rdfs:label "RoadFunctionValue"@en ;
    rdfs:subClassOf skos:Concept ;
    skos:definition "RoadFunctionValue is a code list that enumerates the different purposes of a Road."@en .

tran:RoadUsageValue a owl:Class ;
    rdfs:label "RoadUsageValue"@en ;
    rdfs:subClassOf skos:Concept ;
    skos:definition "RoadUsageValue is a code list that enumerates the different uses of a Road."@en .

tran:Section.class a owl:ObjectProperty ;
    rdfs:label "class"@en ;
    rdfs:domain tran:Section ;
    rdfs:range tran:SectionClassValue ;
    skos:definition "Indicates the specific type of the Section."@en .

tran:Square.class a owl:ObjectProperty ;
    rdfs:label "class"@en ;
    rdfs:domain tran:Square ;
    rdfs:range tran:SquareClassValue ;
    skos:definition "Indicates the specific type of the Square."@en .

tran:SquareFunctionValue a owl:Class ;
    rdfs:label "SquareFunctionValue"@en ;
    rdfs:subClassOf skos:Concept ;
    skos:definition "SquareFunctionValue is a code list that enumerates the different purposes of a Square."@en .

tran:SquareUsageValue a owl:Class ;
    rdfs:label "SquareUsageValue"@en ;
    rdfs:subClassOf skos:Concept ;
    skos:definition "SquareUsageValue is a code list that enumerates the different uses of a Square."@en .

tran:Track.class a owl:ObjectProperty ;
    rdfs:label "class"@en ;
    rdfs:domain tran:Track ;
    rdfs:range tran:TrackClassValue ;
    skos:definition "Indicates the specific type of the Track."@en .

tran:TrackFunctionValue a owl:Class ;
    rdfs:label "TrackFunctionValue"@en ;
    rdfs:subClassOf skos:Concept ;
    skos:definition "TrackFunctionValue is a code list that enumerates the different purposes of a Track."@en .

tran:TrackUsageValue a owl:Class ;
    rdfs:label "TrackUsageValue"@en ;
    rdfs:subClassOf skos:Concept ;
    skos:definition "TrackUsageValue is a code list that enumerates the different uses of a Track."@en .

tran:TrafficArea.class a owl:ObjectProperty ;
    rdfs:label "class"@en ;
    rdfs:domain tran:TrafficArea ;
    rdfs:range tran:TrafficAreaClassValue ;
    skos:definition "Indicates the specific type of the TrafficArea."@en .

tran:TrafficArea.surfaceMaterial a owl:ObjectProperty ;
    rdfs:label "surfaceMaterial"@en ;
    rdfs:domain tran:TrafficArea ;
    rdfs:range tran:SurfaceMaterialValue ;
    skos:definition "Specifies the type of pavement of the TrafficArea."@en .

tran:TrafficAreaFunctionValue a owl:Class ;
    rdfs:label "TrafficAreaFunctionValue"@en ;
    rdfs:subClassOf skos:Concept ;
    skos:definition "TrafficAreaFunctionValue is a code list that enumerates the different purposes of a TrafficArea."@en .

tran:TrafficAreaUsageValue a owl:Class ;
    rdfs:label "TrafficAreaUsageValue"@en ;
    rdfs:subClassOf skos:Concept ;
    skos:definition "TrafficAreaUsageValue is a code list that enumerates the different uses of a TrafficArea."@en .

tran:TrafficSpace.class a owl:ObjectProperty ;
    rdfs:label "class"@en ;
    rdfs:domain tran:TrafficSpace ;
    rdfs:range tran:TrafficSpaceClassValue ;
    skos:definition "Indicates the specific type of the TrafficSpace."@en .

tran:TrafficSpace.granularity a owl:DatatypeProperty ;
    rdfs:label "granularity"@en ;
    rdfs:domain tran:TrafficSpace ;
    rdfs:range tran:GranularityValue ;
    skos:definition "Defines whether traffic spaces are represented by individual ways or by individual lanes, depending on the desired level of spatial and semantic decomposition."@en .

tran:TrafficSpace.trafficDirection a owl:DatatypeProperty ;
    rdfs:label "trafficDirection"@en ;
    rdfs:domain tran:TrafficSpace ;
    rdfs:range tran:TrafficDirectionValue ;
    skos:definition "Indicates the direction of traffic flow relative to the corresponding linear geometry representation."@en .

tran:TrafficSpaceFunctionValue a owl:Class ;
    rdfs:label "TrafficSpaceFunctionValue"@en ;
    rdfs:subClassOf skos:Concept ;
    skos:definition "TrafficSpaceFunctionValue is a code list that enumerates the different purposes of a TrafficSpace."@en .

tran:TrafficSpaceUsageValue a owl:Class ;
    rdfs:label "TrafficSpaceUsageValue"@en ;
    rdfs:subClassOf skos:Concept ;
    skos:definition "TrafficSpaceUsageValue is a code list that enumerates the different uses of a TrafficSpace."@en .

tran:Waterway.class a owl:ObjectProperty ;
    rdfs:label "class"@en ;
    rdfs:domain tran:Waterway ;
    rdfs:range tran:WaterwayClassValue ;
    skos:definition "Indicates the specific type of the Waterway."@en .

tran:WaterwayFunctionValue a owl:Class ;
    rdfs:label "WaterwayFunctionValue"@en ;
    rdfs:subClassOf skos:Concept ;
    skos:definition "WaterwayFunctionValue is a code list that enumerates the different purposes of a Waterway."@en .

tran:WaterwayUsageValue a owl:Class ;
    rdfs:label "WaterwayUsageValue"@en ;
    rdfs:subClassOf skos:Concept ;
    skos:definition "WaterwayUsageValue is a code list that enumerates the different uses of a Waterway."@en .

tran:AuxiliaryTrafficAreaClassValue a owl:Class ;
    rdfs:label "AuxiliaryTrafficAreaClassValue"@en ;
    rdfs:subClassOf skos:Concept ;
    skos:definition "AuxiliaryTrafficAreaClassValue is a code list used to further classify an AuxiliaryTrafficArea."@en .

tran:AuxiliaryTrafficSpaceClassValue a owl:Class ;
    rdfs:label "AuxiliaryTrafficSpaceClassValue"@en ;
    rdfs:subClassOf skos:Concept ;
    skos:definition "AuxiliaryTrafficSpaceClassValue is a code list used to further classify an AuxiliaryTrafficSpace."@en .

tran:ClearanceSpace a owl:Class ;
    rdfs:label "ClearanceSpace"@en ;
    rdfs:subClassOf [ a owl:Restriction ;
            owl:allValuesFrom tran:ADEOfClearanceSpace ;
            owl:onProperty tran:adeOfClearanceSpace ],
        [ a owl:Restriction ;
            owl:allValuesFrom tran:ClearanceSpaceClassValue ;
            owl:onProperty tran:ClearanceSpace.class ],
        core:AbstractUnoccupiedSpace ;
    skos:definition "A ClearanceSpace represents the actual free space above a TrafficArea within which a mobile object can move without contacting an obstruction."@en .

tran:Hole a owl:Class ;
    rdfs:label "Hole"@en ;
    rdfs:subClassOf [ a owl:Restriction ;
            owl:allValuesFrom tran:ADEOfHole ;
            owl:onProperty tran:adeOfHole ],
        [ a owl:Restriction ;
            owl:allValuesFrom tran:HoleClassValue ;
            owl:onProperty tran:Hole.class ],
        [ a owl:Restriction ;
            owl:maxQualifiedCardinality "1"^^xsd:nonNegativeInteger ;
            owl:onClass tran:HoleClassValue ;
            owl:onProperty tran:Hole.class ],
        core:AbstractUnoccupiedSpace ;
    skos:definition "A Hole is an opening in the surface of a Road, Track or Square such as road damages, manholes or drains. Holes can span multiple transportation objects."@en .

tran:HoleClassValue a owl:Class ;
    rdfs:label "HoleClassValue"@en ;
    rdfs:subClassOf skos:Concept ;
    skos:definition "HoleClassValue is a code list used to further classify a Hole."@en .

tran:IntersectionClassValue a owl:Class ;
    rdfs:label "IntersectionClassValue"@en ;
    rdfs:subClassOf skos:Concept ;
    skos:definition "IntersectionClassValue is a code list used to further classify an Intersection."@en .

tran:Marking a owl:Class ;
    rdfs:label "Marking"@en ;
    rdfs:subClassOf [ a owl:Restriction ;
            owl:allValuesFrom tran:ADEOfMarking ;
            owl:onProperty tran:adeOfMarking ],
        [ a owl:Restriction ;
            owl:allValuesFrom tran:MarkingClassValue ;
            owl:onProperty tran:Marking.class ],
        [ a owl:Restriction ;
            owl:maxQualifiedCardinality "1"^^xsd:nonNegativeInteger ;
            owl:onClass tran:MarkingClassValue ;
            owl:onProperty tran:Marking.class ],
        core:AbstractThematicSurface ;
    skos:definition "A Marking is a visible pattern on a transportation area relevant to the structuring or restriction of traffic. Examples are road markings and markings related to railway or waterway traffic."@en .

tran:MarkingClassValue a owl:Class ;
    rdfs:label "MarkingClassValue"@en ;
    rdfs:subClassOf skos:Concept ;
    skos:definition "MarkingClassValue is a code list used to further classify a Marking."@en .

tran:RailwayClassValue a owl:Class ;
    rdfs:label "RailwayClassValue"@en ;
    rdfs:subClassOf skos:Concept ;
    skos:definition "RailwayClassValue is a code list used to further classify a Railway."@en .

tran:RoadClassValue a owl:Class ;
    rdfs:label "RoadClassValue"@en ;
    rdfs:subClassOf skos:Concept ;
    skos:definition "RoadClassValue is a code list used to further classify a Road."@en .

tran:SectionClassValue a owl:Class ;
    rdfs:label "SectionClassValue"@en ;
    rdfs:subClassOf skos:Concept ;
    skos:definition "SectionClassValue is a code list used to further classify a Section."@en .

tran:SquareClassValue a owl:Class ;
    rdfs:label "SquareClassValue"@en ;
    rdfs:subClassOf skos:Concept ;
    skos:definition "SquareClassValue is a code list used to further classify a Square."@en .

tran:TrackClassValue a owl:Class ;
    rdfs:label "TrackClassValue"@en ;
    rdfs:subClassOf skos:Concept ;
    skos:definition "TrackClassValue is a code list used to further classify a Track."@en .

tran:TrafficAreaClassValue a owl:Class ;
    rdfs:label "TrafficAreaClassValue"@en ;
    rdfs:subClassOf skos:Concept ;
    skos:definition "TrafficAreaClassValue is a code list used to further classify a TrafficArea."@en .

tran:TrafficSpaceClassValue a owl:Class ;
    rdfs:label "TrafficSpaceClassValue"@en ;
    rdfs:subClassOf skos:Concept ;
    skos:definition "TrafficSpaceClassValue is a code list used to further classify a TrafficSpace."@en .

tran:WaterwayClassValue a owl:Class ;
    rdfs:label "WaterwayClassValue"@en ;
    rdfs:subClassOf skos:Concept ;
    skos:definition "WaterwayClassValue is a code list used to further classify a Waterway."@en .

tran:Square a owl:Class ;
    rdfs:label "Square"@en ;
    rdfs:subClassOf [ a owl:Restriction ;
            owl:allValuesFrom tran:SquareUsageValue ;
            owl:onProperty tran:Square.usage ],
        [ a owl:Restriction ;
            owl:allValuesFrom tran:SquareFunctionValue ;
            owl:onProperty tran:Square.function ],
        [ a owl:Restriction ;
            owl:allValuesFrom tran:SquareClassValue ;
            owl:onProperty tran:Square.class ],
        [ a owl:Restriction ;
            owl:maxQualifiedCardinality "1"^^xsd:nonNegativeInteger ;
            owl:onClass tran:SquareClassValue ;
            owl:onProperty tran:Square.class ],
        [ a owl:Restriction ;
            owl:allValuesFrom tran:ADEOfSquare ;
            owl:onProperty tran:adeOfSquare ],
        tran:AbstractTransportationSpace ;
    skos:definition "A Square is a transportation space for unrestricted movement for vehicles, bicycles and/or pedestrians. This includes plazas as well as large sealed surfaces such as parking lots."@en .

tran:AuxiliaryTrafficArea a owl:Class ;
    rdfs:label "AuxiliaryTrafficArea"@en ;
    rdfs:subClassOf [ a owl:Restriction ;
            owl:allValuesFrom tran:AuxiliaryTrafficAreaUsageValue ;
            owl:onProperty tran:AuxiliaryTrafficArea.usage ],
        [ a owl:Restriction ;
            owl:allValuesFrom tran:ADEOfAuxiliaryTrafficArea ;
            owl:onProperty tran:adeOfAuxiliaryTrafficArea ],
        [ a owl:Restriction ;
            owl:allValuesFrom tran:AuxiliaryTrafficAreaFunctionValue ;
            owl:onProperty tran:AuxiliaryTrafficArea.function ],
        [ a owl:Restriction ;
            owl:allValuesFrom tran:AuxiliaryTrafficAreaClassValue ;
            owl:onProperty tran:AuxiliaryTrafficArea.class ],
        [ a owl:Restriction ;
            owl:allValuesFrom tran:SurfaceMaterialValue ;
            owl:onProperty tran:AuxiliaryTrafficArea.surfaceMaterial ],
        [ a owl:Restriction ;
            owl:maxQualifiedCardinality "1"^^xsd:nonNegativeInteger ;
            owl:onClass tran:SurfaceMaterialValue ;
            owl:onProperty tran:AuxiliaryTrafficArea.surfaceMaterial ],
        [ a owl:Restriction ;
            owl:maxQualifiedCardinality "1"^^xsd:nonNegativeInteger ;
            owl:onClass tran:AuxiliaryTrafficAreaClassValue ;
            owl:onProperty tran:AuxiliaryTrafficArea.class ],
        core:AbstractThematicSurface ;
    skos:definition "An AuxiliaryTrafficArea is the ground surface of an AuxiliaryTrafficSpace."@en .

tran:GranularityValue a rdfs:Datatype ;
    rdfs:label "GranularityValue"@en ;
    owl:equivalentClass [ a rdfs:Datatype ;
            owl:oneOf ( "lane" "way" ) ] ;
    skos:definition "GranularityValue enumerates the different levels of granularity in which transportation objects are represented."@en .

tran:Railway a owl:Class ;
    rdfs:label "Railway"@en ;
    rdfs:subClassOf [ a owl:Restriction ;
            owl:allValuesFrom tran:RailwayFunctionValue ;
            owl:onProperty tran:Railway.function ],
        [ a owl:Restriction ;
            owl:allValuesFrom tran:ADEOfRailway ;
            owl:onProperty tran:adeOfRailway ],
        [ a owl:Restriction ;
            owl:allValuesFrom tran:RailwayClassValue ;
            owl:onProperty tran:Railway.class ],
        [ a owl:Restriction ;
            owl:allValuesFrom tran:Intersection ;
            owl:onProperty tran:Railway.intersection ],
        [ a owl:Restriction ;
            owl:allValuesFrom tran:RailwayUsageValue ;
            owl:onProperty tran:Railway.usage ],
        [ a owl:Restriction ;
            owl:allValuesFrom tran:Section ;
            owl:onProperty tran:Railway.section ],
        [ a owl:Restriction ;
            owl:maxQualifiedCardinality "1"^^xsd:nonNegativeInteger ;
            owl:onClass tran:RailwayClassValue ;
            owl:onProperty tran:Railway.class ],
        tran:AbstractTransportationSpace ;
    skos:definition "A Railway is a transportation space used by wheeled vehicles on rails."@en .

tran:Road a owl:Class ;
    rdfs:label "Road"@en ;
    rdfs:subClassOf [ a owl:Restriction ;
            owl:allValuesFrom tran:RoadUsageValue ;
            owl:onProperty tran:Road.usage ],
        [ a owl:Restriction ;
            owl:allValuesFrom tran:ADEOfRoad ;
            owl:onProperty tran:adeOfRoad ],
        [ a owl:Restriction ;
            owl:allValuesFrom tran:RoadFunctionValue ;
            owl:onProperty tran:Road.function ],
        [ a owl:Restriction ;
            owl:allValuesFrom tran:Intersection ;
            owl:onProperty tran:Road.intersection ],
        [ a owl:Restriction ;
            owl:allValuesFrom tran:RoadClassValue ;
            owl:onProperty tran:Road.class ],
        [ a owl:Restriction ;
            owl:maxQualifiedCardinality "1"^^xsd:nonNegativeInteger ;
            owl:onClass tran:RoadClassValue ;
            owl:onProperty tran:Road.class ],
        [ a owl:Restriction ;
            owl:allValuesFrom tran:Section ;
            owl:onProperty tran:Road.section ],
        tran:AbstractTransportationSpace ;
    skos:definition "A Road is a transportation space used by vehicles, bicycles and/or pedestrians."@en .

tran:SurfaceMaterialValue a owl:Class ;
    rdfs:label "SurfaceMaterialValue"@en ;
    rdfs:subClassOf skos:Concept ;
    skos:definition "SurfaceMaterialValue is a code list that enumerates the different surface materials."@en .

tran:Track a owl:Class ;
    rdfs:label "Track"@en ;
    rdfs:subClassOf [ a owl:Restriction ;
            owl:allValuesFrom tran:ADEOfTrack ;
            owl:onProperty tran:adeOfTrack ],
        [ a owl:Restriction ;
            owl:maxQualifiedCardinality "1"^^xsd:nonNegativeInteger ;
            owl:onClass tran:TrackClassValue ;
            owl:onProperty tran:Track.class ],
        [ a owl:Restriction ;
            owl:allValuesFrom tran:TrackClassValue ;
            owl:onProperty tran:Track.class ],
        [ a owl:Restriction ;
            owl:allValuesFrom tran:Section ;
            owl:onProperty tran:Track.section ],
        [ a owl:Restriction ;
            owl:allValuesFrom tran:TrackUsageValue ;
            owl:onProperty tran:Track.usage ],
        [ a owl:Restriction ;
            owl:allValuesFrom tran:Intersection ;
            owl:onProperty tran:Track.intersection ],
        [ a owl:Restriction ;
            owl:allValuesFrom tran:TrackFunctionValue ;
            owl:onProperty tran:Track.function ],
        tran:AbstractTransportationSpace ;
    skos:definition "A Track is a small path mainly used by pedestrians. Tracks can be segmented into Sections and Intersections."@en .

tran:TrafficArea a owl:Class ;
    rdfs:label "TrafficArea"@en ;
    rdfs:subClassOf [ a owl:Restriction ;
            owl:allValuesFrom tran:ADEOfTrafficArea ;
            owl:onProperty tran:adeOfTrafficArea ],
        [ a owl:Restriction ;
            owl:maxQualifiedCardinality "1"^^xsd:nonNegativeInteger ;
            owl:onClass tran:SurfaceMaterialValue ;
            owl:onProperty tran:TrafficArea.surfaceMaterial ],
        [ a owl:Restriction ;
            owl:allValuesFrom tran:TrafficAreaClassValue ;
            owl:onProperty tran:TrafficArea.class ],
        [ a owl:Restriction ;
            owl:allValuesFrom tran:SurfaceMaterialValue ;
            owl:onProperty tran:TrafficArea.surfaceMaterial ],
        [ a owl:Restriction ;
            owl:maxQualifiedCardinality "1"^^xsd:nonNegativeInteger ;
            owl:onClass tran:TrafficAreaClassValue ;
            owl:onProperty tran:TrafficArea.class ],
        [ a owl:Restriction ;
            owl:allValuesFrom tran:TrafficAreaUsageValue ;
            owl:onProperty tran:TrafficArea.usage ],
        [ a owl:Restriction ;
            owl:allValuesFrom tran:TrafficAreaFunctionValue ;
            owl:onProperty tran:TrafficArea.function ],
        core:AbstractThematicSurface ;
    skos:definition "A TrafficArea is the ground surface of a TrafficSpace. Traffic areas are the surfaces upon which traffic actually takes place."@en .

tran:TrafficDirectionValue a rdfs:Datatype ;
    rdfs:label "TrafficDirectionValue"@en ;
    owl:equivalentClass [ a rdfs:Datatype ;
            owl:oneOf ( "forwards" "backwards" "both" ) ] ;
    skos:definition "TrafficDirectionValue enumerates the allowed directions of travel of a mobile object."@en .

tran:Waterway a owl:Class ;
    rdfs:label "Waterway"@en ;
    rdfs:subClassOf [ a owl:Restriction ;
            owl:allValuesFrom tran:ADEOfWaterway ;
            owl:onProperty tran:adeOfWaterway ],
        [ a owl:Restriction ;
            owl:maxQualifiedCardinality "1"^^xsd:nonNegativeInteger ;
            owl:onClass tran:WaterwayClassValue ;
            owl:onProperty tran:Waterway.class ],
        [ a owl:Restriction ;
            owl:allValuesFrom tran:Section ;
            owl:onProperty tran:Waterway.section ],
        [ a owl:Restriction ;
            owl:allValuesFrom tran:WaterwayClassValue ;
            owl:onProperty tran:Waterway.class ],
        [ a owl:Restriction ;
            owl:allValuesFrom tran:WaterwayFunctionValue ;
            owl:onProperty tran:Waterway.function ],
        [ a owl:Restriction ;
            owl:allValuesFrom tran:Intersection ;
            owl:onProperty tran:Waterway.intersection ],
        [ a owl:Restriction ;
            owl:allValuesFrom tran:WaterwayUsageValue ;
            owl:onProperty tran:Waterway.usage ],
        tran:AbstractTransportationSpace ;
    skos:definition "A Waterway is a transportation space used for the movement of vessels upon or within a water body."@en .

tran:AuxiliaryTrafficSpace a owl:Class ;
    rdfs:label "AuxiliaryTrafficSpace"@en ;
    rdfs:subClassOf [ a owl:Restriction ;
            owl:allValuesFrom tran:ADEOfAuxiliaryTrafficSpace ;
            owl:onProperty tran:adeOfAuxiliaryTrafficSpace ],
        [ a owl:Restriction ;
            owl:maxQualifiedCardinality "1"^^xsd:nonNegativeInteger ;
            owl:onClass tran:AuxiliaryTrafficSpaceClassValue ;
            owl:onProperty tran:AuxiliaryTrafficSpace.class ],
        [ a owl:Restriction ;
            owl:allValuesFrom tran:GranularityValue ;
            owl:onProperty tran:AuxiliaryTrafficSpace.granularity ],
        [ a owl:Restriction ;
            owl:allValuesFrom tran:AuxiliaryTrafficArea ;
            owl:onProperty tran:AuxiliaryTrafficSpace.boundary ],
        [ a owl:Restriction ;
            owl:allValuesFrom tran:AuxiliaryTrafficSpaceFunctionValue ;
            owl:onProperty tran:AuxiliaryTrafficSpace.function ],
        [ a owl:Restriction ;
            owl:allValuesFrom tran:AuxiliaryTrafficSpaceUsageValue ;
            owl:onProperty tran:AuxiliaryTrafficSpace.usage ],
        [ a owl:Restriction ;
            owl:onDataRange tran:GranularityValue ;
            owl:onProperty tran:AuxiliaryTrafficSpace.granularity ;
            owl:qualifiedCardinality "1"^^xsd:nonNegativeInteger ],
        [ a owl:Restriction ;
            owl:allValuesFrom tran:AuxiliaryTrafficSpaceClassValue ;
            owl:onProperty tran:AuxiliaryTrafficSpace.class ],
        core:AbstractUnoccupiedSpace ;
    skos:definition "An AuxiliaryTrafficSpace is a space within the transportation space not intended for traffic purposes."@en .

tran:AbstractTransportationSpace a owl:Class ;
    rdfs:label "AbstractTransportationSpace"@en ;
    iso19150-2:isAbstract true ;
    rdfs:subClassOf [ a owl:Restriction ;
            owl:allValuesFrom tran:TrafficDirectionValue ;
            owl:onProperty tran:AbstractTransportationSpace.trafficDirection ],
        [ a owl:Restriction ;
            owl:allValuesFrom tran:Hole ;
            owl:onProperty tran:hole ],
        [ a owl:Restriction ;
            owl:allValuesFrom tran:ADEOfAbstractTransportationSpace ;
            owl:onProperty tran:adeOfAbstractTransportationSpace ],
        [ a owl:Restriction ;
            owl:allValuesFrom core:Occupancy ;
            owl:onProperty tran:AbstractTransportationSpace.occupancy ],
        [ a owl:Restriction ;
            owl:allValuesFrom tran:Marking ;
            owl:onProperty tran:marking ],
        [ a owl:Restriction ;
            owl:maxQualifiedCardinality "1"^^xsd:nonNegativeInteger ;
            owl:onDataRange tran:TrafficDirectionValue ;
            owl:onProperty tran:AbstractTransportationSpace.trafficDirection ],
        [ a owl:Restriction ;
            owl:allValuesFrom tran:TrafficSpace ;
            owl:onProperty tran:trafficSpace ],
        [ a owl:Restriction ;
            owl:allValuesFrom tran:AuxiliaryTrafficSpace ;
            owl:onProperty tran:auxiliaryTrafficSpace ],
        core:AbstractUnoccupiedSpace ;
    skos:definition "AbstractTransportationSpace is the abstract superclass of transportation objects such as Roads, Tracks, Railways, Waterways or Squares."@en .

tran:Intersection a owl:Class ;
    rdfs:label "Intersection"@en ;
    rdfs:subClassOf [ a owl:Restriction ;
            owl:allValuesFrom tran:ADEOfIntersection ;
            owl:onProperty tran:adeOfIntersection ],
        [ a owl:Restriction ;
            owl:allValuesFrom tran:IntersectionClassValue ;
            owl:onProperty tran:Intersection.class ],
        [ a owl:Restriction ;
            owl:maxQualifiedCardinality "1"^^xsd:nonNegativeInteger ;
            owl:onClass tran:IntersectionClassValue ;
            owl:onProperty tran:Intersection.class ],
        tran:AbstractTransportationSpace ;
    skos:definition "An Intersection is a transportation space that is a shared segment of multiple Road, Track, Railway, or Waterway objects (e.g. a crossing of two roads or a level crossing of a road and a railway)."@en .

tran:Section a owl:Class ;
    rdfs:label "Section"@en ;
    rdfs:subClassOf [ a owl:Restriction ;
            owl:allValuesFrom tran:ADEOfSection ;
            owl:onProperty tran:adeOfSection ],
        [ a owl:Restriction ;
            owl:allValuesFrom tran:SectionClassValue ;
            owl:onProperty tran:Section.class ],
        [ a owl:Restriction ;
            owl:maxQualifiedCardinality "1"^^xsd:nonNegativeInteger ;
            owl:onClass tran:SectionClassValue ;
            owl:onProperty tran:Section.class ],
        tran:AbstractTransportationSpace ;
    skos:definition "A Section is a transportation space that is a segment of a Road, Railway, Track, or Waterway."@en .

tran:TrafficSpace a owl:Class ;
    rdfs:label "TrafficSpace"@en ;
    rdfs:subClassOf [ a owl:Restriction ;
            owl:allValuesFrom tran:ADEOfTrafficSpace ;
            owl:onProperty tran:adeOfTrafficSpace ],
        [ a owl:Restriction ;
            owl:allValuesFrom tran:GranularityValue ;
            owl:onProperty tran:TrafficSpace.granularity ],
        [ a owl:Restriction ;
            owl:allValuesFrom tran:TrafficSpace ;
            owl:onProperty tran:predecessor ],
        [ a owl:Restriction ;
            owl:maxQualifiedCardinality "1"^^xsd:nonNegativeInteger ;
            owl:onClass tran:TrafficSpaceClassValue ;
            owl:onProperty tran:TrafficSpace.class ],
        [ a owl:Restriction ;
            owl:allValuesFrom tran:TrafficSpaceFunctionValue ;
            owl:onProperty tran:TrafficSpace.function ],
        [ a owl:Restriction ;
            owl:allValuesFrom core:Occupancy ;
            owl:onProperty tran:TrafficSpace.occupancy ],
        [ a owl:Restriction ;
            owl:maxQualifiedCardinality "1"^^xsd:nonNegativeInteger ;
            owl:onDataRange tran:TrafficDirectionValue ;
            owl:onProperty tran:TrafficSpace.trafficDirection ],
        [ a owl:Restriction ;
            owl:allValuesFrom tran:ClearanceSpace ;
            owl:onProperty tran:clearanceSpace ],
        [ a owl:Restriction ;
            owl:allValuesFrom tran:TrafficSpaceUsageValue ;
            owl:onProperty tran:TrafficSpace.usage ],
        [ a owl:Restriction ;
            owl:allValuesFrom tran:TrafficSpaceClassValue ;
            owl:onProperty tran:TrafficSpace.class ],
        [ a owl:Restriction ;
            owl:allValuesFrom tran:TrafficSpace ;
            owl:onProperty tran:successor ],
        [ a owl:Restriction ;
            owl:allValuesFrom tran:TrafficDirectionValue ;
            owl:onProperty tran:TrafficSpace.trafficDirection ],
        [ a owl:Restriction ;
            owl:onDataRange tran:GranularityValue ;
            owl:onProperty tran:TrafficSpace.granularity ;
            owl:qualifiedCardinality "1"^^xsd:nonNegativeInteger ],
        [ a owl:Restriction ;
            owl:allValuesFrom tran:TrafficArea ;
            owl:onProperty tran:TrafficSpace.boundary ],
        core:AbstractUnoccupiedSpace ;
    skos:definition "A TrafficSpace is a space in which traffic takes place. Traffic includes the movement of entities such as trains, vehicles, pedestrians, ships, or other transportation types."@en .

[] a owl:AllDisjointClasses ;
    owl:members ( tran:Intersection tran:Railway tran:Road tran:Section tran:Square tran:Track tran:Waterway ) .

