@prefix core: <https://www.opengis.net/ont/citygml/core#> .
@prefix iso19150-2: <http://def.isotc211.org/iso19150/-2/2012/base#> .
@prefix owl: <http://www.w3.org/2002/07/owl#> .
@prefix rdfs: <http://www.w3.org/2000/01/rdf-schema#> .
@prefix skos: <http://www.w3.org/2004/02/skos/core#> .
@prefix wtr: <https://www.opengis.net/ont/citygml/waterbody#> .
@prefix xsd: <http://www.w3.org/2001/XMLSchema#> .

<https://www.opengis.net/ont/citygml/waterbody> a owl:Ontology ;
    rdfs:label "WaterBody"@en ;
    owl:imports <http://def.isotc211.org/iso19150/-2/2012/base>,
        <https://www.opengis.net/ont/citygml/core> ;
    skos:definition "The WaterBody module supports representation of the thematic aspects and 3D geometry of rivers, canals, lakes, and basins. It does, however, not inherit any hydrological or other dynamic aspects of fluid flow."@en .

wtr:WaterGroundSurface a owl:Class ;
    rdfs:label "WaterGroundSurface"@en ;
    rdfs:subClassOf [ a owl:Restriction ;
            owl:allValuesFrom wtr:ADEOfWaterGroundSurface ;
            owl:onProperty wtr:adeOfWaterGroundSurface ],
        wtr:AbstractWaterBoundarySurface ;
    owl:disjointWith wtr:WaterSurface ;
    skos:definition "A WaterGroundSurface represents the exterior boundary surface of the submerged bottom of a water body."@en .

wtr:WaterBody a owl:Class ;
    rdfs:label "WaterBody"@en ;
    rdfs:subClassOf [ a owl:Restriction ;
            owl:allValuesFrom wtr:ADEOfWaterBody ;
            owl:onProperty wtr:adeOfWaterBody ],
        [ a owl:Restriction ;
            owl:allValuesFrom wtr:AbstractWaterBoundarySurface ;
            owl:onProperty wtr:WaterBody.boundary ],
        [ a owl:Restriction ;
            owl:allValuesFrom wtr:WaterBodyFunctionValue ;
            owl:onProperty wtr:function ],
        [ a owl:Restriction ;
            owl:allValuesFrom wtr:WaterBodyClassValue ;
            owl:onProperty wtr:class ],
        [ a owl:Restriction ;
            owl:maxQualifiedCardinality "1"^^xsd:nonNegativeInteger ;
            owl:onClass wtr:WaterBodyClassValue ;
            owl:onProperty wtr:class ],
        [ a owl:Restriction ;
            owl:allValuesFrom wtr:WaterBodyUsageValue ;
            owl:onProperty wtr:usage ],
        core:AbstractOccupiedSpace ;
    skos:definition "A WaterBody represents significant and permanent or semi-permanent accumulations of surface water, usually covering a part of the Earth."@en .

wtr:WaterBody.boundary a owl:ObjectProperty ;
    rdfs:label "boundary"@en ;
    rdfs:domain wtr:WaterBody ;
    rdfs:range wtr:AbstractWaterBoundarySurface .

wtr:WaterSurface a owl:Class ;
    rdfs:label "WaterSurface"@en ;
    rdfs:subClassOf [ a owl:Restriction ;
            owl:allValuesFrom wtr:ADEOfWaterSurface ;
            owl:onProperty wtr:adeOfWaterSurface ],
        [ a owl:Restriction ;
            owl:allValuesFrom wtr:WaterLevelValue ;
            owl:onProperty wtr:waterLevel ],
        [ a owl:Restriction ;
            owl:maxQualifiedCardinality "1"^^xsd:nonNegativeInteger ;
            owl:onClass wtr:WaterLevelValue ;
            owl:onProperty wtr:waterLevel ],
        wtr:AbstractWaterBoundarySurface ;
    skos:definition "A WaterSurface represents the upper exterior interface between a water body and the atmosphere."@en .

wtr:adeOfAbstractWaterBoundarySurface a owl:ObjectProperty ;
    rdfs:label "adeOfAbstractWaterBoundarySurface"@en ;
    rdfs:range wtr:ADEOfAbstractWaterBoundarySurface ;
    skos:definition "Augments AbstractWaterBoundarySurface with properties defined in an ADE."@en .

wtr:adeOfWaterBody a owl:ObjectProperty ;
    rdfs:label "adeOfWaterBody"@en ;
    rdfs:range wtr:ADEOfWaterBody ;
    skos:definition "Augments the WaterBody with properties defined in an ADE."@en .

wtr:adeOfWaterGroundSurface a owl:ObjectProperty ;
    rdfs:label "adeOfWaterGroundSurface"@en ;
    rdfs:range wtr:ADEOfWaterGroundSurface ;
    skos:definition "Augments the WaterGroundSurface with properties defined in an ADE."@en .

wtr:adeOfWaterSurface a owl:ObjectProperty ;
    rdfs:label "adeOfWaterSurface"@en ;
    rdfs:range wtr:ADEOfWaterSurface ;
    skos:definition "Augments the WaterSurface with properties defined in an ADE."@en .

wtr:function a owl:ObjectProperty ;
    rdfs:label "function"@en ;
    rdfs:range wtr:WaterBodyFunctionValue ;
    skos:definition "Specifies the intended purposes of the WaterBody."@en .

wtr:usage a owl:ObjectProperty ;
    rdfs:label "usage"@en ;
    rdfs:range wtr:WaterBodyUsageValue ;
    skos:definition "Specifies the actual uses of the WaterBody."@en .

wtr:ADEOfAbstractWaterBoundarySurface a owl:Class ;
    rdfs:label "ADEOfAbstractWaterBoundarySurface"@en ;
    iso19150-2:isAbstract true ;
    skos:definition "ADEOfAbstractWaterBoundarySurface acts as a hook to define properties within an ADE that are to be added to AbstractWaterBoundarySurface."@en .

wtr:ADEOfWaterBody a owl:Class ;
    rdfs:label "ADEOfWaterBody"@en ;
    iso19150-2:isAbstract true ;
    skos:definition "ADEOfWaterBody acts as a hook to define properties within an ADE that are to be added to a WaterBody."@en .

wtr:ADEOfWaterGroundSurface a owl:Class ;
    rdfs:label "ADEOfWaterGroundSurface"@en ;
    iso19150-2:isAbstract true ;
    skos:definition "ADEOfWaterGroundSurface acts as a hook to define properties within an ADE that are to be added to a WaterGroundSurface."@en .

wtr:ADEOfWaterSurface a owl:Class ;
    rdfs:label "ADEOfWaterSurface"@en ;
    iso19150-2:isAbstract true ;
    skos:definition "ADEOfWaterSurface acts as a hook to define properties within an ADE that are to be added to a WaterSurface."@en .

wtr:WaterBodyFunctionValue a owl:Class ;
    rdfs:label "WaterBodyFunctionValue"@en ;
    rdfs:subClassOf skos:Concept ;
    skos:definition "WaterBodyFunctionValue is a code list that enumerates the different purposes of a WaterBody."@en .

wtr:WaterBodyUsageValue a owl:Class ;
    rdfs:label "WaterBodyUsageValue"@en ;
    rdfs:subClassOf skos:Concept ;
    skos:definition "WaterBodyUsageValue is a code list that enumerates the different uses of a WaterBody."@en .

wtr:class a owl:ObjectProperty ;
    rdfs:label "class"@en ;
    rdfs:range wtr:WaterBodyClassValue ;
    skos:definition "Indicates the specific type of the WaterBody."@en .

wtr:waterLevel a owl:ObjectProperty ;
    rdfs:label "waterLevel"@en ;
    rdfs:range wtr:WaterLevelValue ;
    skos:definition "Specifies the level of the WaterSurface."@en .

wtr:WaterBodyClassValue a owl:Class ;
    rdfs:label "WaterBodyClassValue"@en ;
    rdfs:subClassOf skos:Concept ;
    skos:definition "WaterBodyClassValue is a code list used to further classify a WaterBody."@en .

wtr:WaterLevelValue a owl:Class ;
    rdfs:label "WaterLevelValue"@en ;
    rdfs:subClassOf skos:Concept ;
    skos:definition "WaterLevelValue is a code list that enumerates the different levels of a water surface."@en .

wtr:AbstractWaterBoundarySurface a owl:Class ;
    rdfs:label "AbstractWaterBoundarySurface"@en ;
    iso19150-2:isAbstract true ;
    rdfs:subClassOf [ a owl:Restriction ;
            owl:allValuesFrom wtr:ADEOfAbstractWaterBoundarySurface ;
            owl:onProperty wtr:adeOfAbstractWaterBoundarySurface ],
        core:AbstractThematicSurface ;
    skos:definition "AbstractWaterBoundarySurface is the abstract superclass for all kinds of thematic surfaces bounding a water body."@en .

