@prefix bldg:        <https://www.opengis.net/ont/citygml/building/> .
@prefix con:         <https://www.opengis.net/ont/citygml/construction/> .
@prefix core:        <https://www.opengis.net/ont/citygml/core/> .
@prefix iso19136-bt: <http://def.isotc211.org/iso19136/2007/BasicTypes#> .
@prefix iso19150-2:  <http://def.isotc211.org/iso19150/-2/2012/base#> .
@prefix owl:         <http://www.w3.org/2002/07/owl#> .
@prefix rdf:         <http://www.w3.org/1999/02/22-rdf-syntax-ns#> .
@prefix rdfs:        <http://www.w3.org/2000/01/rdf-schema#> .
@prefix sc:          <http://shapechange.net/resources/ont/base#> .
@prefix skos:        <http://www.w3.org/2004/02/skos/core#> .
@prefix xsd:         <http://www.w3.org/2001/XMLSchema#> .

bldg:storeysAboveGround
        rdf:type         owl:DatatypeProperty;
        rdfs:label       "storeysAboveGround"@en;
        rdfs:range       xsd:integer;
        skos:definition  "Indicates the number of storeys positioned above ground level."@en .

bldg:buildingPart  rdf:type  owl:ObjectProperty;
        rdfs:label       "buildingPart"@en;
        rdfs:range       bldg:BuildingPart;
        skos:definition  "Relates the building parts to the Building."@en .

bldg:BuildingInstallationFunctionValue
        rdf:type         owl:Class;
        rdfs:label       "BuildingInstallationFunctionValue"@en;
        rdfs:subClassOf  skos:Concept;
        skos:definition  "BuildingInstallationFunctionValue is a code list that enumerates the different purposes of a BuildingInstallation."@en .

bldg:AbstractBuildingSubdivision.function
        rdf:type         owl:ObjectProperty;
        rdfs:domain      bldg:AbstractBuildingSubdivision;
        rdfs:label       "function"@en;
        rdfs:range       bldg:BuildingSubdivisionFunctionValue;
        skos:definition  "Specifies the intended purposes of the building subdivision."@en .

bldg:BuildingSubdivisionClassValue
        rdf:type         owl:Class;
        rdfs:label       "BuildingSubdivisionClassValue"@en;
        rdfs:subClassOf  skos:Concept;
        skos:definition  "BuildingSubdivisionClassValue is a code list used to further classify a BuildingSubdivision."@en .

bldg:Storey  rdf:type    owl:Class;
        rdfs:label       "Storey"@en;
        rdfs:subClassOf  bldg:AbstractBuildingSubdivision;
        rdfs:subClassOf  [ rdf:type           owl:Restriction;
                           owl:allValuesFrom  bldg:ADEOfStorey;
                           owl:onProperty     bldg:adeOfStorey
                         ];
        rdfs:subClassOf  [ rdf:type           owl:Restriction;
                           owl:allValuesFrom  core:AbstractThematicSurface;
                           owl:onProperty     bldg:Storey.boundary
                         ];
        rdfs:subClassOf  [ rdf:type           owl:Restriction;
                           owl:allValuesFrom  bldg:BuildingUnit;
                           owl:onProperty     bldg:buildingUnit
                         ];
        skos:definition  "A Storey is typically a horizontal section of a Building. Storeys are not always defined according to the building structure, but can also be defined according to logical considerations."@en .

bldg:ADEOfBuildingFurniture
        rdf:type               owl:Class;
        rdfs:label             "ADEOfBuildingFurniture"@en;
        iso19150-2:isAbstract  true;
        skos:definition        "ADEOfBuildingFurniture acts as a hook to define properties within an ADE that are to be added to a BuildingFurniture."@en .

bldg:buildingSubdivision
        rdf:type         owl:ObjectProperty;
        rdfs:label       "buildingSubdivision"@en;
        rdfs:range       bldg:AbstractBuildingSubdivision;
        skos:definition  "Relates the logical subdivisions to the Building or BuildingPart."@en .

bldg:ADEOfBuildingUnit
        rdf:type               owl:Class;
        rdfs:label             "ADEOfBuildingUnit"@en;
        iso19150-2:isAbstract  true;
        skos:definition        "ADEOfBuildingUnit acts as a hook to define properties within an ADE that are to be added to a BuildingUnit."@en .

bldg:BuildingConstructiveElement.class
        rdf:type         owl:ObjectProperty;
        rdfs:domain      bldg:BuildingConstructiveElement;
        rdfs:label       "class"@en;
        rdfs:range       bldg:BuildingConstructiveElementClassValue;
        skos:definition  "Indicates the specific type of the BuildingConstructiveElement."@en .

bldg:AbstractBuilding.buildingRoom
        rdf:type         owl:ObjectProperty;
        rdfs:domain      bldg:AbstractBuilding;
        rdfs:label       "buildingRoom"@en;
        rdfs:range       bldg:BuildingRoom;
        skos:definition  "Relates the rooms to the Building or BuildingPart."@en .

bldg:BuildingSubdivisionFunctionValue
        rdf:type         owl:Class;
        rdfs:label       "BuildingSubdivisionFunctionValue"@en;
        rdfs:subClassOf  skos:Concept;
        skos:definition  "BuildingSubdivisionFunctionValue is a code list that enumerates the different purposes of a BuildingSubdivision."@en .

bldg:AbstractBuilding.buildingInstallation
        rdf:type         owl:ObjectProperty;
        rdfs:domain      bldg:AbstractBuilding;
        rdfs:label       "buildingInstallation"@en;
        rdfs:range       bldg:BuildingInstallation;
        skos:definition  "Relates the installation objects to the Building or BuildingPart."@en .

bldg:BuildingConstructiveElement.usage
        rdf:type         owl:ObjectProperty;
        rdfs:domain      bldg:BuildingConstructiveElement;
        rdfs:label       "usage"@en;
        rdfs:range       bldg:BuildingConstructiveElementUsageValue;
        skos:definition  "Specifies the actual uses of the BuildingConstructiveElement."@en .

bldg:AbstractBuilding.class
        rdf:type         owl:ObjectProperty;
        rdfs:domain      bldg:AbstractBuilding;
        rdfs:label       "class"@en;
        rdfs:range       bldg:BuildingClassValue;
        skos:definition  "Indicates the specific type of the Building or BuildingPart."@en .

bldg:storeysBelowGround
        rdf:type         owl:DatatypeProperty;
        rdfs:label       "storeysBelowGround"@en;
        rdfs:range       xsd:integer;
        skos:definition  "Indicates the number of storeys positioned below ground level."@en .

bldg:BuildingConstructiveElementClassValue
        rdf:type         owl:Class;
        rdfs:label       "BuildingConstructiveElementClassValue"@en;
        rdfs:subClassOf  skos:Concept;
        skos:definition  "BuildingConstructiveElementClassValue is a code list used to further classify a BuildingConstructiveElement."@en .

bldg:BuildingFurniture.class
        rdf:type         owl:ObjectProperty;
        rdfs:domain      bldg:BuildingFurniture;
        rdfs:label       "class"@en;
        rdfs:range       bldg:BuildingFurnitureClassValue;
        skos:definition  "Indicates the specific type of the BuildingFurniture."@en .

bldg:RoomHeight  rdf:type  owl:Class;
        rdfs:label       "RoomHeight"@en;
        rdfs:subClassOf  [ rdf:type                  owl:Restriction;
                           owl:onClass               bldg:RoomElevationReferenceValue;
                           owl:onProperty            bldg:lowReference;
                           owl:qualifiedCardinality  "1"^^xsd:nonNegativeInteger
                         ];
        rdfs:subClassOf  [ rdf:type                  owl:Restriction;
                           owl:onClass               bldg:RoomElevationReferenceValue;
                           owl:onProperty            bldg:highReference;
                           owl:qualifiedCardinality  "1"^^xsd:nonNegativeInteger
                         ];
        rdfs:subClassOf  [ rdf:type           owl:Restriction;
                           owl:allValuesFrom  con:HeightStatusValue;
                           owl:onProperty     bldg:status
                         ];
        rdfs:subClassOf  [ rdf:type           owl:Restriction;
                           owl:allValuesFrom  bldg:RoomElevationReferenceValue;
                           owl:onProperty     bldg:highReference
                         ];
        rdfs:subClassOf  [ rdf:type                  owl:Restriction;
                           owl:onClass               con:HeightStatusValue;
                           owl:onProperty            bldg:status;
                           owl:qualifiedCardinality  "1"^^xsd:nonNegativeInteger
                         ];
        rdfs:subClassOf  [ rdf:type                  owl:Restriction;
                           owl:onClass               sc:Measure;
                           owl:onProperty            bldg:value;
                           owl:qualifiedCardinality  "1"^^xsd:nonNegativeInteger
                         ];
        rdfs:subClassOf  [ rdf:type           owl:Restriction;
                           owl:allValuesFrom  sc:Measure;
                           owl:onProperty     bldg:value
                         ];
        rdfs:subClassOf  [ rdf:type           owl:Restriction;
                           owl:allValuesFrom  bldg:RoomElevationReferenceValue;
                           owl:onProperty     bldg:lowReference
                         ];
        skos:definition  "The RoomHeight represents a vertical distance (measured or estimated) between a low reference and a high reference. [cf. INSPIRE]"@en .

bldg:AbstractBuilding.usage
        rdf:type         owl:ObjectProperty;
        rdfs:domain      bldg:AbstractBuilding;
        rdfs:label       "usage"@en;
        rdfs:range       bldg:BuildingUsageValue;
        skos:definition  "Specifies the actual uses of the Building or BuildingPart."@en .

bldg:ADEOfBuildingConstructiveElement
        rdf:type               owl:Class;
        rdfs:label             "ADEOfBuildingConstructiveElement"@en;
        iso19150-2:isAbstract  true;
        skos:definition        "ADEOfBuildingConstructiveElement acts as a hook to define properties within an ADE that are to be added to a BuildingConstructiveElement."@en .

bldg:ADEOfAbstractBuilding
        rdf:type               owl:Class;
        rdfs:label             "ADEOfAbstractBuilding"@en;
        iso19150-2:isAbstract  true;
        skos:definition        "ADEOfAbstractBuilding acts as a hook to define properties within an ADE that are to be added to AbstractBuilding."@en .

bldg:BuildingFurnitureUsageValue
        rdf:type         owl:Class;
        rdfs:label       "BuildingFurnitureUsageValue"@en;
        rdfs:subClassOf  skos:Concept;
        skos:definition  "BuildingFurnitureUsageValue is a code list that enumerates the different uses of a BuildingFurniture."@en .

bldg:BuildingConstructiveElement.function
        rdf:type         owl:ObjectProperty;
        rdfs:domain      bldg:BuildingConstructiveElement;
        rdfs:label       "function"@en;
        rdfs:range       bldg:BuildingConstructiveElementFunctionValue;
        skos:definition  "Specifies the intended purposes of the BuildingConstructiveElement."@en .

bldg:storeyHeightsAboveGround
        rdf:type         owl:ObjectProperty;
        rdfs:label       "storeyHeightsAboveGround"@en;
        rdfs:range       iso19136-bt:MeasureOrNilReasonList;
        skos:definition  "Lists the heights of each storey above ground. The first value in the list denotes the height of the storey closest to the ground level, the last value denotes the height furthest away."@en .

bldg:AbstractBuildingSubdivision.buildingInstallation
        rdf:type         owl:ObjectProperty;
        rdfs:domain      bldg:AbstractBuildingSubdivision;
        rdfs:label       "buildingInstallation"@en;
        rdfs:range       bldg:BuildingInstallation;
        skos:definition  "Relates the installation objects to the building subdivision."@en .

bldg:adeOfBuildingRoom
        rdf:type         owl:ObjectProperty;
        rdfs:label       "adeOfBuildingRoom"@en;
        rdfs:range       bldg:ADEOfBuildingRoom;
        skos:definition  "Augments the BuildingRoom with properties defined in an ADE."@en .

bldg:adeOfAbstractBuilding
        rdf:type         owl:ObjectProperty;
        rdfs:label       "adeOfAbstractBuilding"@en;
        rdfs:range       bldg:ADEOfAbstractBuilding;
        skos:definition  "Augments AbstractBuilding with properties defined in an ADE."@en .

bldg:BuildingRoom.usage
        rdf:type         owl:ObjectProperty;
        rdfs:domain      bldg:BuildingRoom;
        rdfs:label       "usage"@en;
        rdfs:range       bldg:BuildingRoomUsageValue;
        skos:definition  "Specifies the actual uses of the BuildingRoom."@en .

bldg:elevation  rdf:type  owl:ObjectProperty;
        rdfs:label       "elevation"@en;
        rdfs:range       con:Elevation;
        skos:definition  "Specifies qualified elevations of the building subdivision in relation to a well-defined surface which is commonly taken as origin (e.g. geoid or water level). [cf. INSPIRE]"@en .

bldg:adeOfBuildingConstructiveElement
        rdf:type         owl:ObjectProperty;
        rdfs:label       "adeOfBuildingConstructiveElement"@en;
        rdfs:range       bldg:ADEOfBuildingConstructiveElement;
        skos:definition  "Augments the BuildingConstructiveElement with properties defined in an ADE."@en .

bldg:ADEOfBuilding  rdf:type   owl:Class;
        rdfs:label             "ADEOfBuilding"@en;
        iso19150-2:isAbstract  true;
        skos:definition        "ADEOfBuilding acts as a hook to define properties within an ADE that are to be added to a Building."@en .

bldg:AbstractBuilding.buildingFurniture
        rdf:type         owl:ObjectProperty;
        rdfs:domain      bldg:AbstractBuilding;
        rdfs:label       "buildingFurniture"@en;
        rdfs:range       bldg:BuildingFurniture;
        skos:definition  "Relates the furniture objects to the Building or BuildingPart."@en .

bldg:ADEOfBuildingPart
        rdf:type               owl:Class;
        rdfs:label             "ADEOfBuildingPart"@en;
        iso19150-2:isAbstract  true;
        skos:definition        "ADEOfBuildingPart acts as a hook to define properties within an ADE that are to be added to a BuildingPart."@en .

bldg:AbstractBuilding.buildingConstructiveElement
        rdf:type         owl:ObjectProperty;
        rdfs:domain      bldg:AbstractBuilding;
        rdfs:label       "buildingConstructiveElement"@en;
        rdfs:range       bldg:BuildingConstructiveElement;
        skos:definition  "Relates the constructive elements to the Building or BuildingPart."@en .

bldg:AbstractBuilding
        rdf:type               owl:Class;
        rdfs:label             "AbstractBuilding"@en;
        rdfs:subClassOf        con:AbstractConstruction;
        rdfs:subClassOf        [ rdf:type           owl:Restriction;
                                 owl:allValuesFrom  xsd:integer;
                                 owl:onProperty     bldg:storeysBelowGround
                               ];
        rdfs:subClassOf        [ rdf:type           owl:Restriction;
                                 owl:allValuesFrom  iso19136-bt:MeasureOrNilReasonList;
                                 owl:onProperty     bldg:storeyHeightsAboveGround
                               ];
        rdfs:subClassOf        [ rdf:type           owl:Restriction;
                                 owl:allValuesFrom  bldg:BuildingClassValue;
                                 owl:onProperty     bldg:AbstractBuilding.class
                               ];
        rdfs:subClassOf        [ rdf:type           owl:Restriction;
                                 owl:allValuesFrom  bldg:BuildingFunctionValue;
                                 owl:onProperty     bldg:AbstractBuilding.function
                               ];
        rdfs:subClassOf        [ rdf:type           owl:Restriction;
                                 owl:allValuesFrom  xsd:integer;
                                 owl:onProperty     bldg:storeysAboveGround
                               ];
        rdfs:subClassOf        [ rdf:type           owl:Restriction;
                                 owl:allValuesFrom  bldg:BuildingConstructiveElement;
                                 owl:onProperty     bldg:AbstractBuilding.buildingConstructiveElement
                               ];
        rdfs:subClassOf        [ rdf:type           owl:Restriction;
                                 owl:allValuesFrom  bldg:BuildingInstallation;
                                 owl:onProperty     bldg:AbstractBuilding.buildingInstallation
                               ];
        rdfs:subClassOf        [ rdf:type           owl:Restriction;
                                 owl:allValuesFrom  bldg:BuildingFurniture;
                                 owl:onProperty     bldg:AbstractBuilding.buildingFurniture
                               ];
        rdfs:subClassOf        [ rdf:type                     owl:Restriction;
                                 owl:maxQualifiedCardinality  "1"^^xsd:nonNegativeInteger;
                                 owl:onClass                  bldg:RoofTypeValue;
                                 owl:onProperty               bldg:roofType
                               ];
        rdfs:subClassOf        [ rdf:type           owl:Restriction;
                                 owl:allValuesFrom  iso19136-bt:MeasureOrNilReasonList;
                                 owl:onProperty     bldg:storeyHeightsBelowGround
                               ];
        rdfs:subClassOf        [ rdf:type                     owl:Restriction;
                                 owl:maxQualifiedCardinality  "1"^^xsd:nonNegativeInteger;
                                 owl:onClass                  iso19136-bt:MeasureOrNilReasonList;
                                 owl:onProperty               bldg:storeyHeightsAboveGround
                               ];
        rdfs:subClassOf        [ rdf:type           owl:Restriction;
                                 owl:allValuesFrom  bldg:AbstractBuildingSubdivision;
                                 owl:onProperty     bldg:buildingSubdivision
                               ];
        rdfs:subClassOf        [ rdf:type                     owl:Restriction;
                                 owl:maxQualifiedCardinality  "1"^^xsd:nonNegativeInteger;
                                 owl:onClass                  bldg:BuildingClassValue;
                                 owl:onProperty               bldg:AbstractBuilding.class
                               ];
        rdfs:subClassOf        [ rdf:type           owl:Restriction;
                                 owl:allValuesFrom  bldg:RoofTypeValue;
                                 owl:onProperty     bldg:roofType
                               ];
        rdfs:subClassOf        [ rdf:type                     owl:Restriction;
                                 owl:maxQualifiedCardinality  "1"^^xsd:nonNegativeInteger;
                                 owl:onClass                  xsd:integer;
                                 owl:onProperty               bldg:storeysAboveGround
                               ];
        rdfs:subClassOf        [ rdf:type           owl:Restriction;
                                 owl:allValuesFrom  bldg:BuildingRoom;
                                 owl:onProperty     bldg:AbstractBuilding.buildingRoom
                               ];
        rdfs:subClassOf        [ rdf:type                     owl:Restriction;
                                 owl:maxQualifiedCardinality  "1"^^xsd:nonNegativeInteger;
                                 owl:onClass                  iso19136-bt:MeasureOrNilReasonList;
                                 owl:onProperty               bldg:storeyHeightsBelowGround
                               ];
        rdfs:subClassOf        [ rdf:type           owl:Restriction;
                                 owl:allValuesFrom  core:Address;
                                 owl:onProperty     bldg:AbstractBuilding.address
                               ];
        rdfs:subClassOf        [ rdf:type                     owl:Restriction;
                                 owl:maxQualifiedCardinality  "1"^^xsd:nonNegativeInteger;
                                 owl:onClass                  xsd:integer;
                                 owl:onProperty               bldg:storeysBelowGround
                               ];
        rdfs:subClassOf        [ rdf:type           owl:Restriction;
                                 owl:allValuesFrom  bldg:BuildingUsageValue;
                                 owl:onProperty     bldg:AbstractBuilding.usage
                               ];
        rdfs:subClassOf        [ rdf:type           owl:Restriction;
                                 owl:allValuesFrom  bldg:ADEOfAbstractBuilding;
                                 owl:onProperty     bldg:adeOfAbstractBuilding
                               ];
        iso19150-2:isAbstract  true;
        skos:definition        "AbstractBuilding is an abstract superclass representing the common attributes and associations of the classes Building and BuildingPart."@en .

bldg:AbstractBuildingSubdivision.class
        rdf:type         owl:ObjectProperty;
        rdfs:domain      bldg:AbstractBuildingSubdivision;
        rdfs:label       "class"@en;
        rdfs:range       bldg:BuildingSubdivisionClassValue;
        skos:definition  "Indicates the specific type of the building subdivision."@en .

bldg:BuildingRoom  rdf:type  owl:Class;
        rdfs:label       "BuildingRoom"@en;
        rdfs:subClassOf  core:AbstractUnoccupiedSpace;
        rdfs:subClassOf  [ rdf:type                     owl:Restriction;
                           owl:maxQualifiedCardinality  "1"^^xsd:nonNegativeInteger;
                           owl:onClass                  bldg:BuildingRoomClassValue;
                           owl:onProperty               bldg:BuildingRoom.class
                         ];
        rdfs:subClassOf  [ rdf:type           owl:Restriction;
                           owl:allValuesFrom  bldg:ADEOfBuildingRoom;
                           owl:onProperty     bldg:adeOfBuildingRoom
                         ];
        rdfs:subClassOf  [ rdf:type           owl:Restriction;
                           owl:allValuesFrom  bldg:BuildingFurniture;
                           owl:onProperty     bldg:BuildingRoom.buildingFurniture
                         ];
        rdfs:subClassOf  [ rdf:type           owl:Restriction;
                           owl:allValuesFrom  bldg:BuildingRoomFunctionValue;
                           owl:onProperty     bldg:BuildingRoom.function
                         ];
        rdfs:subClassOf  [ rdf:type           owl:Restriction;
                           owl:allValuesFrom  core:AbstractThematicSurface;
                           owl:onProperty     bldg:BuildingRoom.boundary
                         ];
        rdfs:subClassOf  [ rdf:type           owl:Restriction;
                           owl:allValuesFrom  bldg:RoomHeight;
                           owl:onProperty     bldg:roomHeight
                         ];
        rdfs:subClassOf  [ rdf:type           owl:Restriction;
                           owl:allValuesFrom  bldg:BuildingRoomClassValue;
                           owl:onProperty     bldg:BuildingRoom.class
                         ];
        rdfs:subClassOf  [ rdf:type           owl:Restriction;
                           owl:allValuesFrom  bldg:BuildingInstallation;
                           owl:onProperty     bldg:BuildingRoom.buildingInstallation
                         ];
        rdfs:subClassOf  [ rdf:type           owl:Restriction;
                           owl:allValuesFrom  bldg:BuildingRoomUsageValue;
                           owl:onProperty     bldg:BuildingRoom.usage
                         ];
        skos:definition  "A BuildingRoom is a space within a Building or BuildingPart intended for human occupancy (e.g. a place of work or recreation) and/or containment of animals or things. A BuildingRoom is bounded physically and/or virtually (e.g. by ClosureSurfaces or GenericSurfaces)."@en .

bldg:highReference  rdf:type  owl:ObjectProperty;
        rdfs:label       "highReference"@en;
        rdfs:range       bldg:RoomElevationReferenceValue;
        skos:definition  "Indicates the high point used to calculate the value of the room height."@en .

bldg:roofType  rdf:type  owl:ObjectProperty;
        rdfs:label       "roofType"@en;
        rdfs:range       bldg:RoofTypeValue;
        skos:definition  "Indicates the shape of the roof of the Building or BuildingPart."@en .

bldg:value  rdf:type     owl:DatatypeProperty;
        rdfs:label       "value"@en;
        rdfs:range       sc:Measure;
        skos:definition  "Specifies the value of the room height."@en .

bldg:AbstractBuildingSubdivision.buildingFurniture
        rdf:type         owl:ObjectProperty;
        rdfs:domain      bldg:AbstractBuildingSubdivision;
        rdfs:label       "buildingFurniture"@en;
        rdfs:range       bldg:BuildingFurniture;
        skos:definition  "Relates the furniture objects to the building subdivision."@en .

bldg:BuildingConstructiveElementFunctionValue
        rdf:type         owl:Class;
        rdfs:label       "BuildingConstructiveElementFunctionValue"@en;
        rdfs:subClassOf  skos:Concept;
        skos:definition  "BuildingConstructiveElementFunctionValue is a code list that enumerates the different purposes of a BuildingConstructiveElement."@en .

bldg:AbstractBuildingSubdivision.usage
        rdf:type         owl:ObjectProperty;
        rdfs:domain      bldg:AbstractBuildingSubdivision;
        rdfs:label       "usage"@en;
        rdfs:range       bldg:BuildingSubdivisionUsageValue;
        skos:definition  "Specifies the actual uses of the building subdivision."@en .

bldg:BuildingInstallationUsageValue
        rdf:type         owl:Class;
        rdfs:label       "BuildingInstallationUsageValue"@en;
        rdfs:subClassOf  skos:Concept;
        skos:definition  "BuildingInstallationUsageValue is a code list that enumerates the different uses of a BuildingInstallation."@en .

bldg:adeOfAbstractBuildingSubdivision
        rdf:type         owl:ObjectProperty;
        rdfs:label       "adeOfAbstractBuildingSubdivision"@en;
        rdfs:range       bldg:ADEOfAbstractBuildingSubdivision;
        skos:definition  "Augments AbstractBuildingSubdivision with properties defined in an ADE."@en .

bldg:BuildingRoomClassValue
        rdf:type         owl:Class;
        rdfs:label       "BuildingRoomClassValue"@en;
        rdfs:subClassOf  skos:Concept;
        skos:definition  "BuildingRoomClassValue is a code list used to further classify a BuildingRoom."@en .

bldg:BuildingClassValue
        rdf:type         owl:Class;
        rdfs:label       "BuildingClassValue"@en;
        rdfs:subClassOf  skos:Concept;
        skos:definition  "BuildingClassValue is a code list used to further classify a Building."@en .

bldg:storeyHeightsBelowGround
        rdf:type         owl:ObjectProperty;
        rdfs:label       "storeyHeightsBelowGround"@en;
        rdfs:range       iso19136-bt:MeasureOrNilReasonList;
        skos:definition  "Lists the height of each storey below ground. The first value in the list denotes the height of the storey closest to the ground level, the last value denotes the height furthest away."@en .

bldg:adeOfStorey  rdf:type  owl:ObjectProperty;
        rdfs:label       "adeOfStorey"@en;
        rdfs:range       bldg:ADEOfStorey;
        skos:definition  "Augments the Storey with properties defined in an ADE."@en .

bldg:BuildingRoom.function
        rdf:type         owl:ObjectProperty;
        rdfs:domain      bldg:BuildingRoom;
        rdfs:label       "function"@en;
        rdfs:range       bldg:BuildingRoomFunctionValue;
        skos:definition  "Specifies the intended purposes of the BuildingRoom."@en .

bldg:BuildingFurniture.function
        rdf:type         owl:ObjectProperty;
        rdfs:domain      bldg:BuildingFurniture;
        rdfs:label       "function"@en;
        rdfs:range       bldg:BuildingFurnitureFunctionValue;
        skos:definition  "Specifies the intended purposes of the BuildingFurniture."@en .

bldg:adeOfBuildingUnit
        rdf:type         owl:ObjectProperty;
        rdfs:label       "adeOfBuildingUnit"@en;
        rdfs:range       bldg:ADEOfBuildingUnit;
        skos:definition  "Augments the BuildingUnit with properties defined in an ADE."@en .

<https://www.opengis.net/ont/citygml/building>
        rdf:type         owl:Ontology;
        rdfs:label       "Building"@en;
        owl:imports      <http://shapechange.net/resources/ont/base> , <https://www.opengis.net/ont/citygml/construction> , <https://www.opengis.net/ont/citygml/core> , <http://def.isotc211.org/iso19150/-2/2012/base>;
        skos:definition  "The Building module supports representation of thematic and spatial aspects of buildings, building parts, building installations, building subdivisions, and interior building structures."@en .

bldg:AbstractBuilding.address
        rdf:type         owl:ObjectProperty;
        rdfs:domain      bldg:AbstractBuilding;
        rdfs:label       "address"@en;
        rdfs:range       core:Address;
        skos:definition  "Relates the addresses to the Building or BuildingPart."@en .

bldg:BuildingRoomUsageValue
        rdf:type         owl:Class;
        rdfs:label       "BuildingRoomUsageValue"@en;
        rdfs:subClassOf  skos:Concept;
        skos:definition  "BuildingRoomUsageValue is a code list that enumerates the different uses of a BuildingRoom."@en .

bldg:BuildingUsageValue
        rdf:type         owl:Class;
        rdfs:label       "BuildingUsageValue"@en;
        rdfs:subClassOf  skos:Concept;
        skos:definition  "BuildingUsageValue is a code list that enumerates the different uses of a Building."@en .

bldg:BuildingUnit  rdf:type  owl:Class;
        rdfs:label        "BuildingUnit"@en;
        rdfs:subClassOf   bldg:AbstractBuildingSubdivision;
        rdfs:subClassOf   [ rdf:type           owl:Restriction;
                            owl:allValuesFrom  bldg:ADEOfBuildingUnit;
                            owl:onProperty     bldg:adeOfBuildingUnit
                          ];
        rdfs:subClassOf   [ rdf:type           owl:Restriction;
                            owl:allValuesFrom  core:Address;
                            owl:onProperty     bldg:BuildingUnit.address
                          ];
        rdfs:subClassOf   [ rdf:type           owl:Restriction;
                            owl:allValuesFrom  bldg:Storey;
                            owl:onProperty     bldg:storey
                          ];
        owl:disjointWith  bldg:Storey;
        skos:definition   "A BuildingUnit is a logical subdivision of a Building. BuildingUnits are formed according to some homogeneous property like function, ownership, management, or accessibility. They may be separately sold, rented out, inherited, managed, etc."@en .

bldg:BuildingSubdivisionUsageValue
        rdf:type         owl:Class;
        rdfs:label       "BuildingSubdivisionUsageValue"@en;
        rdfs:subClassOf  skos:Concept;
        skos:definition  "BuildingSubdivisionUsageValue is a code list that enumerates the different uses of a BuildingSubdivision."@en .

bldg:BuildingConstructiveElement
        rdf:type         owl:Class;
        rdfs:label       "BuildingConstructiveElement"@en;
        rdfs:subClassOf  con:AbstractConstructiveElement;
        rdfs:subClassOf  [ rdf:type           owl:Restriction;
                           owl:allValuesFrom  bldg:ADEOfBuildingConstructiveElement;
                           owl:onProperty     bldg:adeOfBuildingConstructiveElement
                         ];
        rdfs:subClassOf  [ rdf:type           owl:Restriction;
                           owl:allValuesFrom  bldg:BuildingConstructiveElementUsageValue;
                           owl:onProperty     bldg:BuildingConstructiveElement.usage
                         ];
        rdfs:subClassOf  [ rdf:type           owl:Restriction;
                           owl:allValuesFrom  bldg:BuildingConstructiveElementFunctionValue;
                           owl:onProperty     bldg:BuildingConstructiveElement.function
                         ];
        rdfs:subClassOf  [ rdf:type           owl:Restriction;
                           owl:allValuesFrom  bldg:BuildingConstructiveElementClassValue;
                           owl:onProperty     bldg:BuildingConstructiveElement.class
                         ];
        rdfs:subClassOf  [ rdf:type                     owl:Restriction;
                           owl:maxQualifiedCardinality  "1"^^xsd:nonNegativeInteger;
                           owl:onClass                  bldg:BuildingConstructiveElementClassValue;
                           owl:onProperty               bldg:BuildingConstructiveElement.class
                         ];
        skos:definition  "A BuildingConstructiveElement is an element of a Building which is essential from a structural point of view. Examples are walls, slabs, staircases, beams."@en .

bldg:roomHeight  rdf:type  owl:ObjectProperty;
        rdfs:label       "roomHeight"@en;
        rdfs:range       bldg:RoomHeight;
        skos:definition  "Specifies qualified heights of the BuildingRoom."@en .

bldg:BuildingInstallation.function
        rdf:type         owl:ObjectProperty;
        rdfs:domain      bldg:BuildingInstallation;
        rdfs:label       "function"@en;
        rdfs:range       bldg:BuildingInstallationFunctionValue;
        skos:definition  "Specifies the intended purposes of the BuildingInstallation."@en .

bldg:AbstractBuildingSubdivision.buildingConstructiveElement
        rdf:type         owl:ObjectProperty;
        rdfs:domain      bldg:AbstractBuildingSubdivision;
        rdfs:label       "buildingConstructiveElement"@en;
        rdfs:range       bldg:BuildingConstructiveElement;
        skos:definition  "Relates the constructive elements to the building subdivision."@en .

bldg:BuildingUnit.address
        rdf:type         owl:ObjectProperty;
        rdfs:domain      bldg:BuildingUnit;
        rdfs:label       "address"@en;
        rdfs:range       core:Address;
        skos:definition  "Relates to the addresses that are assigned to the BuildingUnit."@en .

bldg:BuildingRoomFunctionValue
        rdf:type         owl:Class;
        rdfs:label       "BuildingRoomFunctionValue"@en;
        rdfs:subClassOf  skos:Concept;
        skos:definition  "BuildingRoomFunctionValue is a code list that enumerates the different purposes of a BuildingRoom."@en .

bldg:BuildingInstallation
        rdf:type         owl:Class;
        rdfs:label       "BuildingInstallation"@en;
        rdfs:subClassOf  con:AbstractInstallation;
        rdfs:subClassOf  [ rdf:type           owl:Restriction;
                           owl:allValuesFrom  bldg:ADEOfBuildingInstallation;
                           owl:onProperty     bldg:adeOfBuildingInstallation
                         ];
        rdfs:subClassOf  [ rdf:type           owl:Restriction;
                           owl:allValuesFrom  bldg:BuildingInstallationUsageValue;
                           owl:onProperty     bldg:BuildingInstallation.usage
                         ];
        rdfs:subClassOf  [ rdf:type           owl:Restriction;
                           owl:allValuesFrom  bldg:BuildingInstallationFunctionValue;
                           owl:onProperty     bldg:BuildingInstallation.function
                         ];
        rdfs:subClassOf  [ rdf:type           owl:Restriction;
                           owl:allValuesFrom  bldg:BuildingInstallationClassValue;
                           owl:onProperty     bldg:BuildingInstallation.class
                         ];
        rdfs:subClassOf  [ rdf:type                     owl:Restriction;
                           owl:maxQualifiedCardinality  "1"^^xsd:nonNegativeInteger;
                           owl:onClass                  bldg:BuildingInstallationClassValue;
                           owl:onProperty               bldg:BuildingInstallation.class
                         ];
        skos:definition  "A BuildingInstallation is a permanent part of a Building (inside and/or outside) which has not the significance of a BuildingPart. Examples are stairs, antennas, balconies or small roofs."@en .

bldg:adeOfBuilding  rdf:type  owl:ObjectProperty;
        rdfs:label       "adeOfBuilding"@en;
        rdfs:range       bldg:ADEOfBuilding;
        skos:definition  "Augments the Building with properties defined in an ADE."@en .

bldg:ADEOfBuildingInstallation
        rdf:type               owl:Class;
        rdfs:label             "ADEOfBuildingInstallation"@en;
        iso19150-2:isAbstract  true;
        skos:definition        "ADEOfBuildingInstallation acts as a hook to define properties within an ADE that are to be added to a BuildingInstallation."@en .

bldg:BuildingFurnitureClassValue
        rdf:type         owl:Class;
        rdfs:label       "BuildingFurnitureClassValue"@en;
        rdfs:subClassOf  skos:Concept;
        skos:definition  "BuildingFurnitureClassValue is a code list used to further classify a BuildingFurniture."@en .

bldg:BuildingRoom.buildingFurniture
        rdf:type         owl:ObjectProperty;
        rdfs:domain      bldg:BuildingRoom;
        rdfs:label       "buildingFurniture"@en;
        rdfs:range       bldg:BuildingFurniture;
        skos:definition  "Relates the furniture objects to the BuildingRoom."@en .

bldg:buildingUnit  rdf:type  owl:ObjectProperty;
        rdfs:label       "buildingUnit"@en;
        rdfs:range       bldg:BuildingUnit;
        skos:definition  "Relates to the building units that belong to the Storey."@en .

bldg:AbstractBuildingSubdivision
        rdf:type               owl:Class;
        rdfs:label             "AbstractBuildingSubdivision"@en;
        rdfs:subClassOf        core:AbstractLogicalSpace;
        rdfs:subClassOf        [ rdf:type           owl:Restriction;
                                 owl:allValuesFrom  bldg:ADEOfAbstractBuildingSubdivision;
                                 owl:onProperty     bldg:adeOfAbstractBuildingSubdivision
                               ];
        rdfs:subClassOf        [ rdf:type                     owl:Restriction;
                                 owl:maxQualifiedCardinality  "1"^^xsd:nonNegativeInteger;
                                 owl:onClass                  bldg:BuildingSubdivisionClassValue;
                                 owl:onProperty               bldg:AbstractBuildingSubdivision.class
                               ];
        rdfs:subClassOf        [ rdf:type           owl:Restriction;
                                 owl:allValuesFrom  con:Elevation;
                                 owl:onProperty     bldg:elevation
                               ];
        rdfs:subClassOf        [ rdf:type           owl:Restriction;
                                 owl:allValuesFrom  bldg:BuildingFurniture;
                                 owl:onProperty     bldg:AbstractBuildingSubdivision.buildingFurniture
                               ];
        rdfs:subClassOf        [ rdf:type           owl:Restriction;
                                 owl:allValuesFrom  bldg:BuildingInstallation;
                                 owl:onProperty     bldg:AbstractBuildingSubdivision.buildingInstallation
                               ];
        rdfs:subClassOf        [ rdf:type                     owl:Restriction;
                                 owl:maxQualifiedCardinality  "1"^^xsd:nonNegativeInteger;
                                 owl:onClass                  xsd:double;
                                 owl:onProperty               bldg:sortKey
                               ];
        rdfs:subClassOf        [ rdf:type           owl:Restriction;
                                 owl:allValuesFrom  bldg:BuildingSubdivisionUsageValue;
                                 owl:onProperty     bldg:AbstractBuildingSubdivision.usage
                               ];
        rdfs:subClassOf        [ rdf:type           owl:Restriction;
                                 owl:allValuesFrom  xsd:double;
                                 owl:onProperty     bldg:sortKey
                               ];
        rdfs:subClassOf        [ rdf:type           owl:Restriction;
                                 owl:allValuesFrom  bldg:BuildingConstructiveElement;
                                 owl:onProperty     bldg:AbstractBuildingSubdivision.buildingConstructiveElement
                               ];
        rdfs:subClassOf        [ rdf:type           owl:Restriction;
                                 owl:allValuesFrom  bldg:BuildingSubdivisionFunctionValue;
                                 owl:onProperty     bldg:AbstractBuildingSubdivision.function
                               ];
        rdfs:subClassOf        [ rdf:type           owl:Restriction;
                                 owl:allValuesFrom  bldg:BuildingSubdivisionClassValue;
                                 owl:onProperty     bldg:AbstractBuildingSubdivision.class
                               ];
        rdfs:subClassOf        [ rdf:type           owl:Restriction;
                                 owl:allValuesFrom  bldg:BuildingRoom;
                                 owl:onProperty     bldg:AbstractBuildingSubdivision.buildingRoom
                               ];
        iso19150-2:isAbstract  true;
        skos:definition        "AbstractBuildingSubdivision is the abstract superclass for different kinds of logical building subdivisions."@en .

bldg:status  rdf:type    owl:ObjectProperty;
        rdfs:label       "status"@en;
        rdfs:range       con:HeightStatusValue;
        skos:definition  "Indicates the way the room height has been captured."@en .

bldg:BuildingFurniture.usage
        rdf:type         owl:ObjectProperty;
        rdfs:domain      bldg:BuildingFurniture;
        rdfs:label       "usage"@en;
        rdfs:range       bldg:BuildingFurnitureUsageValue;
        skos:definition  "Specifies the actual uses of the BuildingFurniture."@en .

bldg:BuildingFunctionValue
        rdf:type         owl:Class;
        rdfs:label       "BuildingFunctionValue"@en;
        rdfs:subClassOf  skos:Concept;
        skos:definition  "BuildingFunctionValue is a code list that enumerates the different purposes of a Building."@en .

bldg:BuildingConstructiveElementUsageValue
        rdf:type         owl:Class;
        rdfs:label       "BuildingConstructiveElementUsageValue"@en;
        rdfs:subClassOf  skos:Concept;
        skos:definition  "BuildingConstructiveElementUsageValue is a code list that enumerates the different uses of a BuildingConstructiveElement."@en .

bldg:Storey.boundary  rdf:type  owl:ObjectProperty;
        rdfs:domain      bldg:Storey;
        rdfs:label       "boundary"@en;
        rdfs:range       core:AbstractThematicSurface;
        skos:definition  "Relates to the surfaces that bound the Storey. This relation is inherited from the Core module."@en .

bldg:adeOfBuildingFurniture
        rdf:type         owl:ObjectProperty;
        rdfs:label       "adeOfBuildingFurniture"@en;
        rdfs:range       bldg:ADEOfBuildingFurniture;
        skos:definition  "Augments the BuildingFurniture with properties defined in an ADE."@en .

bldg:BuildingFurniture
        rdf:type         owl:Class;
        rdfs:label       "BuildingFurniture"@en;
        rdfs:subClassOf  con:AbstractFurniture;
        rdfs:subClassOf  [ rdf:type           owl:Restriction;
                           owl:allValuesFrom  bldg:ADEOfBuildingFurniture;
                           owl:onProperty     bldg:adeOfBuildingFurniture
                         ];
        rdfs:subClassOf  [ rdf:type           owl:Restriction;
                           owl:allValuesFrom  bldg:BuildingFurnitureUsageValue;
                           owl:onProperty     bldg:BuildingFurniture.usage
                         ];
        rdfs:subClassOf  [ rdf:type           owl:Restriction;
                           owl:allValuesFrom  bldg:BuildingFurnitureFunctionValue;
                           owl:onProperty     bldg:BuildingFurniture.function
                         ];
        rdfs:subClassOf  [ rdf:type           owl:Restriction;
                           owl:allValuesFrom  bldg:BuildingFurnitureClassValue;
                           owl:onProperty     bldg:BuildingFurniture.class
                         ];
        rdfs:subClassOf  [ rdf:type                     owl:Restriction;
                           owl:maxQualifiedCardinality  "1"^^xsd:nonNegativeInteger;
                           owl:onClass                  bldg:BuildingFurnitureClassValue;
                           owl:onProperty               bldg:BuildingFurniture.class
                         ];
        skos:definition  "A BuildingFurniture is an equipment for occupant use, usually not fixed to the building. [cf. ISO 6707-1]"@en .

bldg:BuildingInstallation.class
        rdf:type         owl:ObjectProperty;
        rdfs:domain      bldg:BuildingInstallation;
        rdfs:label       "class"@en;
        rdfs:range       bldg:BuildingInstallationClassValue;
        skos:definition  "Indicates the specific type of the BuildingInstallation."@en .

bldg:BuildingRoom.class
        rdf:type         owl:ObjectProperty;
        rdfs:domain      bldg:BuildingRoom;
        rdfs:label       "class"@en;
        rdfs:range       bldg:BuildingRoomClassValue;
        skos:definition  "Indicates the specific type of the BuildingRoom."@en .

bldg:storey  rdf:type    owl:ObjectProperty;
        rdfs:label       "storey"@en;
        rdfs:range       bldg:Storey;
        skos:definition  "Relates to the storeys on which the BuildingUnit is located."@en .

bldg:AbstractBuilding.function
        rdf:type         owl:ObjectProperty;
        rdfs:domain      bldg:AbstractBuilding;
        rdfs:label       "function"@en;
        rdfs:range       bldg:BuildingFunctionValue;
        skos:definition  "Specifies the intended purposes of the Building or BuildingPart."@en .

bldg:RoofTypeValue  rdf:type  owl:Class;
        rdfs:label       "RoofTypeValue"@en;
        rdfs:subClassOf  skos:Concept;
        skos:definition  "RoofTypeValue is a code list that enumerates different roof types."@en .

bldg:lowReference  rdf:type  owl:ObjectProperty;
        rdfs:label       "lowReference"@en;
        rdfs:range       bldg:RoomElevationReferenceValue;
        skos:definition  "Indicates the low point used to calculate the value of the room height."@en .

bldg:adeOfBuildingPart
        rdf:type         owl:ObjectProperty;
        rdfs:label       "adeOfBuildingPart"@en;
        rdfs:range       bldg:ADEOfBuildingPart;
        skos:definition  "Augments the BuildingPart with properties defined in an ADE."@en .

bldg:ADEOfStorey  rdf:type     owl:Class;
        rdfs:label             "ADEOfStorey"@en;
        iso19150-2:isAbstract  true;
        skos:definition        "ADEOfStorey acts as a hook to define properties within an ADE that are to be added to a Storey."@en .

bldg:BuildingRoom.buildingInstallation
        rdf:type         owl:ObjectProperty;
        rdfs:domain      bldg:BuildingRoom;
        rdfs:label       "buildingInstallation"@en;
        rdfs:range       bldg:BuildingInstallation;
        skos:definition  "Relates the installation objects to the BuildingRoom."@en .

bldg:ADEOfBuildingRoom
        rdf:type               owl:Class;
        rdfs:label             "ADEOfBuildingRoom"@en;
        iso19150-2:isAbstract  true;
        skos:definition        "ADEOfBuildingRoom acts as a hook to define properties within an ADE that are to be added to a BuildingRoom."@en .

bldg:BuildingRoom.boundary
        rdf:type         owl:ObjectProperty;
        rdfs:domain      bldg:BuildingRoom;
        rdfs:label       "boundary"@en;
        rdfs:range       core:AbstractThematicSurface;
        skos:definition  "Relates to the surfaces that bound the BuildingRoom. This relation is inherited from the Core module."@en .

bldg:RoomElevationReferenceValue
        rdf:type         owl:Class;
        rdfs:label       "RoomElevationReferenceValue"@en;
        rdfs:subClassOf  skos:Concept;
        skos:definition  "RoomElevationReferenceValue is a code list that enumerates the different elevation reference levels used to measure room heights."@en .

bldg:BuildingInstallationClassValue
        rdf:type         owl:Class;
        rdfs:label       "BuildingInstallationClassValue"@en;
        rdfs:subClassOf  skos:Concept;
        skos:definition  "BuildingInstallationClassValue is a code list used to further classify a BuildingInstallation."@en .

bldg:BuildingFurnitureFunctionValue
        rdf:type         owl:Class;
        rdfs:label       "BuildingFurnitureFunctionValue"@en;
        rdfs:subClassOf  skos:Concept;
        skos:definition  "BuildingFurnitureFunctionValue is a code list that enumerates the different purposes of a BuildingFurniture."@en .

bldg:BuildingInstallation.usage
        rdf:type         owl:ObjectProperty;
        rdfs:domain      bldg:BuildingInstallation;
        rdfs:label       "usage"@en;
        rdfs:range       bldg:BuildingInstallationUsageValue;
        skos:definition  "Specifies the actual uses of the BuildingInstallation."@en .

bldg:BuildingPart  rdf:type  owl:Class;
        rdfs:label       "BuildingPart"@en;
        rdfs:subClassOf  bldg:AbstractBuilding;
        rdfs:subClassOf  [ rdf:type           owl:Restriction;
                           owl:allValuesFrom  bldg:ADEOfBuildingPart;
                           owl:onProperty     bldg:adeOfBuildingPart
                         ];
        skos:definition  "A BuildingPart is a physical or functional subdivision of a Building. It would be considered a Building, if it were not part of a collection of other BuildingParts."@en .

bldg:ADEOfAbstractBuildingSubdivision
        rdf:type               owl:Class;
        rdfs:label             "ADEOfAbstractBuildingSubdivision"@en;
        iso19150-2:isAbstract  true;
        skos:definition        "ADEOfAbstractBuildingSubdivision acts as a hook to define properties within an ADE that are to be added to AbstractBuildingSubdivision."@en .

bldg:AbstractBuildingSubdivision.buildingRoom
        rdf:type         owl:ObjectProperty;
        rdfs:domain      bldg:AbstractBuildingSubdivision;
        rdfs:label       "buildingRoom"@en;
        rdfs:range       bldg:BuildingRoom;
        skos:definition  "Relates the rooms to the building subdivision."@en .

bldg:Building  rdf:type   owl:Class;
        rdfs:label        "Building"@en;
        rdfs:subClassOf   bldg:AbstractBuilding;
        rdfs:subClassOf   [ rdf:type           owl:Restriction;
                            owl:allValuesFrom  bldg:ADEOfBuilding;
                            owl:onProperty     bldg:adeOfBuilding
                          ];
        rdfs:subClassOf   [ rdf:type           owl:Restriction;
                            owl:allValuesFrom  bldg:BuildingPart;
                            owl:onProperty     bldg:buildingPart
                          ];
        owl:disjointWith  bldg:BuildingPart;
        skos:definition   "A Building is a free-standing, self-supporting construction that is roofed, usually walled, and can be entered by humans and is normally designed to stand permanently in one place. It is intended for human occupancy (e.g. a place of work or recreation), habitation and/or shelter of humans, animals or things."@en .

bldg:sortKey  rdf:type   owl:DatatypeProperty;
        rdfs:label       "sortKey"@en;
        rdfs:range       xsd:double;
        skos:definition  "Defines an order among the objects that belong to the building subdivision. An example is the sorting of storeys."@en .

bldg:adeOfBuildingInstallation
        rdf:type         owl:ObjectProperty;
        rdfs:label       "adeOfBuildingInstallation"@en;
        rdfs:range       bldg:ADEOfBuildingInstallation;
        skos:definition  "Augments the BuildingInstallation with properties defined in an ADE."@en .
